<?xml version="1.0"?>
<rdf:RDF xmlns="http://www.semanticweb.org/qihan/ontologies/2023/6/untitled-ontology-12/"
     xml:base="http://www.semanticweb.org/qihan/ontologies/2023/6/untitled-ontology-12/"
     xmlns:owl="http://www.w3.org/2002/07/owl#"
     xmlns:rdf="http://www.w3.org/1999/02/22-rdf-syntax-ns#"
     xmlns:xml="http://www.w3.org/XML/1998/namespace"
     xmlns:xsd="http://www.w3.org/2001/XMLSchema#"
     xmlns:rdfs="http://www.w3.org/2000/01/rdf-schema#">
    <owl:Ontology rdf:about="http://www.semanticweb.org/qihan/ontologies/2023/6/untitled-ontology-12"/>
    


    <!-- 
    ///////////////////////////////////////////////////////////////////////////////////////
    //
    // Object Properties
    //
    ///////////////////////////////////////////////////////////////////////////////////////
     -->

    


    <!-- http://www.semanticweb.org/qihan/ontologies/2023/6/untitled-ontology-12#FollowsTestStandard -->

    <owl:ObjectProperty rdf:about="http://www.semanticweb.org/qihan/ontologies/2023/6/untitled-ontology-12#FollowsTestStandard">
        <rdfs:domain rdf:resource="http://www.semanticweb.org/qihan/ontologies/2023/6/untitled-ontology-12#Testing_Method"/>
        <rdfs:range rdf:resource="http://www.semanticweb.org/qihan/ontologies/2023/6/untitled-ontology-12#Test_Equipment"/>
        <rdfs:comment>Represents the relationship between a testing method and the standard or guideline followed for conducting the test.</rdfs:comment>
    </owl:ObjectProperty>
    


    <!-- http://www.semanticweb.org/qihan/ontologies/2023/6/untitled-ontology-12#HasTestParameter -->

    <owl:ObjectProperty rdf:about="http://www.semanticweb.org/qihan/ontologies/2023/6/untitled-ontology-12#HasTestParameter">
        <rdfs:domain rdf:resource="http://www.semanticweb.org/qihan/ontologies/2023/6/untitled-ontology-12#Testing_Method"/>
        <rdfs:range rdf:resource="http://www.semanticweb.org/qihan/ontologies/2023/6/untitled-ontology-12#Test_Parameter"/>
        <rdfs:comment>Represents the relationship between a testing method and the parameters measured or controlled during the test.</rdfs:comment>
    </owl:ObjectProperty>
    


    <!-- http://www.semanticweb.org/qihan/ontologies/2023/6/untitled-ontology-12#HasTestResult -->

    <owl:ObjectProperty rdf:about="http://www.semanticweb.org/qihan/ontologies/2023/6/untitled-ontology-12#HasTestResult">
        <rdfs:domain rdf:resource="http://www.semanticweb.org/qihan/ontologies/2023/6/untitled-ontology-12#Testing_Method"/>
        <rdfs:range rdf:resource="http://www.semanticweb.org/qihan/ontologies/2023/6/untitled-ontology-12#Result_Calculation"/>
        <rdfs:comment>Represents the relationship between a testing method and the results obtained from the test.</rdfs:comment>
    </owl:ObjectProperty>
    


    <!-- http://www.semanticweb.org/qihan/ontologies/2023/6/untitled-ontology-12#HasTestSpecimen -->

    <owl:ObjectProperty rdf:about="http://www.semanticweb.org/qihan/ontologies/2023/6/untitled-ontology-12#HasTestSpecimen">
        <rdfs:domain rdf:resource="http://www.semanticweb.org/qihan/ontologies/2023/6/untitled-ontology-12#Testing_Method"/>
        <rdfs:range rdf:resource="http://www.semanticweb.org/qihan/ontologies/2023/6/untitled-ontology-12#Test_Specimen_Geometry"/>
        <rdfs:comment>Represents the relationship between a testing method and the test specimen required for conducting the test.</rdfs:comment>
    </owl:ObjectProperty>
    


    <!-- http://www.semanticweb.org/qihan/ontologies/2023/6/untitled-ontology-12#UsedForSpecimenPreparation -->

    <owl:ObjectProperty rdf:about="http://www.semanticweb.org/qihan/ontologies/2023/6/untitled-ontology-12#UsedForSpecimenPreparation">
        <rdfs:domain rdf:resource="http://www.semanticweb.org/qihan/ontologies/2023/6/untitled-ontology-12#Specimen_Preparation_Equipment"/>
        <rdfs:range rdf:resource="http://www.semanticweb.org/qihan/ontologies/2023/6/untitled-ontology-12#Material_Manufacturing"/>
        <rdfs:range rdf:resource="http://www.semanticweb.org/qihan/ontologies/2023/6/untitled-ontology-12#Test_Specimen_Geometry"/>
    </owl:ObjectProperty>
    


    <!-- http://www.semanticweb.org/qihan/ontologies/2023/6/untitled-ontology-12#UsesTestEquipment -->

    <owl:ObjectProperty rdf:about="http://www.semanticweb.org/qihan/ontologies/2023/6/untitled-ontology-12#UsesTestEquipment">
        <rdfs:domain rdf:resource="http://www.semanticweb.org/qihan/ontologies/2023/6/untitled-ontology-12#Testing_Method"/>
        <rdfs:range rdf:resource="http://www.semanticweb.org/qihan/ontologies/2023/6/untitled-ontology-12#Test_Equipment"/>
        <rdfs:comment>Represents the relationship between a testing method and the equipment or instruments used to perform the test.</rdfs:comment>
    </owl:ObjectProperty>
    


    <!-- http://www.semanticweb.org/qihan/ontologies/2023/6/untitled-ontology-12#hasPart -->

    <owl:ObjectProperty rdf:about="http://www.semanticweb.org/qihan/ontologies/2023/6/untitled-ontology-12#hasPart"/>
    


    <!-- http://www.semanticweb.org/qihan/ontologies/2023/6/untitled-ontology-12#hasTestingMethod -->

    <owl:ObjectProperty rdf:about="http://www.semanticweb.org/qihan/ontologies/2023/6/untitled-ontology-12#hasTestingMethod">
        <rdfs:domain rdf:resource="http://www.semanticweb.org/qihan/ontologies/2023/6/untitled-ontology-12#Composite_Material"/>
        <rdfs:range rdf:resource="http://www.semanticweb.org/qihan/ontologies/2023/6/untitled-ontology-12#Testing_Method"/>
        <rdfs:comment>Represents the relationship between a composite material and the testing method used for its mechanical testing.</rdfs:comment>
    </owl:ObjectProperty>
    


    <!-- 
    ///////////////////////////////////////////////////////////////////////////////////////
    //
    // Data properties
    //
    ///////////////////////////////////////////////////////////////////////////////////////
     -->

    


    <!-- http://www.semanticweb.org/qihan/ontologies/2023/6/untitled-ontology-12#Equipment_Model -->

    <owl:DatatypeProperty rdf:about="http://www.semanticweb.org/qihan/ontologies/2023/6/untitled-ontology-12#Equipment_Model">
        <rdfs:domain rdf:resource="http://www.semanticweb.org/qihan/ontologies/2023/6/untitled-ontology-12#Specimen_Preparation_Equipment"/>
        <rdfs:domain rdf:resource="http://www.semanticweb.org/qihan/ontologies/2023/6/untitled-ontology-12#Test_Equipment"/>
        <rdfs:range rdf:resource="http://www.w3.org/2001/XMLSchema#string"/>
        <rdfs:comment>Represents the model or version of the test equipment used</rdfs:comment>
    </owl:DatatypeProperty>
    


    <!-- http://www.semanticweb.org/qihan/ontologies/2023/6/untitled-ontology-12#Equipment_Serial_Number -->

    <owl:DatatypeProperty rdf:about="http://www.semanticweb.org/qihan/ontologies/2023/6/untitled-ontology-12#Equipment_Serial_Number">
        <rdfs:domain rdf:resource="http://www.semanticweb.org/qihan/ontologies/2023/6/untitled-ontology-12#Specimen_Preparation_Equipment"/>
        <rdfs:domain rdf:resource="http://www.semanticweb.org/qihan/ontologies/2023/6/untitled-ontology-12#Test_Equipment"/>
        <rdfs:range rdf:resource="http://www.w3.org/2001/XMLSchema#string"/>
        <rdfs:comment>Represents the unique serial number assigned to the test equipment.</rdfs:comment>
    </owl:DatatypeProperty>
    


    <!-- http://www.semanticweb.org/qihan/ontologies/2023/6/untitled-ontology-12#Failure_Mode -->

    <owl:DatatypeProperty rdf:about="http://www.semanticweb.org/qihan/ontologies/2023/6/untitled-ontology-12#Failure_Mode">
        <rdfs:domain rdf:resource="http://www.semanticweb.org/qihan/ontologies/2023/6/untitled-ontology-12#Failure_Mode"/>
        <rdfs:range rdf:resource="http://www.w3.org/2001/XMLSchema#string"/>
    </owl:DatatypeProperty>
    


    <!-- http://www.semanticweb.org/qihan/ontologies/2023/6/untitled-ontology-12#Institution_Name -->

    <owl:DatatypeProperty rdf:about="http://www.semanticweb.org/qihan/ontologies/2023/6/untitled-ontology-12#Institution_Name">
        <rdfs:domain rdf:resource="http://www.semanticweb.org/qihan/ontologies/2023/6/untitled-ontology-12#Testing_Institution"/>
        <rdfs:range rdf:resource="http://www.w3.org/2001/XMLSchema#string"/>
    </owl:DatatypeProperty>
    


    <!-- http://www.semanticweb.org/qihan/ontologies/2023/6/untitled-ontology-12#Parameter_Unit -->

    <owl:DatatypeProperty rdf:about="http://www.semanticweb.org/qihan/ontologies/2023/6/untitled-ontology-12#Parameter_Unit">
        <rdfs:domain rdf:resource="http://www.semanticweb.org/qihan/ontologies/2023/6/untitled-ontology-12#Test_Environment"/>
        <rdfs:domain rdf:resource="http://www.semanticweb.org/qihan/ontologies/2023/6/untitled-ontology-12#Test_Parameter"/>
        <rdfs:range rdf:resource="http://www.w3.org/2001/XMLSchema#string"/>
        <rdfs:comment>Represents the unit of measurement for a test parameter, such as &quot;MPa&quot; for stress or &quot;mm&quot; for displacement.</rdfs:comment>
    </owl:DatatypeProperty>
    


    <!-- http://www.semanticweb.org/qihan/ontologies/2023/6/untitled-ontology-12#Parameter_Value -->

    <owl:DatatypeProperty rdf:about="http://www.semanticweb.org/qihan/ontologies/2023/6/untitled-ontology-12#Parameter_Value">
        <rdfs:domain rdf:resource="http://www.semanticweb.org/qihan/ontologies/2023/6/untitled-ontology-12#Test_Environment"/>
        <rdfs:domain rdf:resource="http://www.semanticweb.org/qihan/ontologies/2023/6/untitled-ontology-12#Test_Parameter"/>
        <rdfs:range rdf:resource="http://www.w3.org/2001/XMLSchema#decimal"/>
        <rdfs:range rdf:resource="http://www.w3.org/2001/XMLSchema#float"/>
        <rdfs:comment>Represents the specific value or measurement of a test parameter.</rdfs:comment>
    </owl:DatatypeProperty>
    


    <!-- http://www.semanticweb.org/qihan/ontologies/2023/6/untitled-ontology-12#Personnel_List -->

    <owl:DatatypeProperty rdf:about="http://www.semanticweb.org/qihan/ontologies/2023/6/untitled-ontology-12#Personnel_List">
        <rdfs:domain rdf:resource="http://www.semanticweb.org/qihan/ontologies/2023/6/untitled-ontology-12#Testing_Institution"/>
        <rdfs:range rdf:resource="http://www.w3.org/2001/XMLSchema#string"/>
    </owl:DatatypeProperty>
    


    <!-- http://www.semanticweb.org/qihan/ontologies/2023/6/untitled-ontology-12#RawMaterial -->

    <owl:DatatypeProperty rdf:about="http://www.semanticweb.org/qihan/ontologies/2023/6/untitled-ontology-12#RawMaterial">
        <rdfs:domain rdf:resource="http://www.semanticweb.org/qihan/ontologies/2023/6/untitled-ontology-12#Material_Manufacturing"/>
        <rdfs:range rdf:resource="http://www.w3.org/2001/XMLSchema#decimal"/>
        <rdfs:range rdf:resource="http://www.w3.org/2001/XMLSchema#float"/>
        <rdfs:range rdf:resource="http://www.w3.org/2001/XMLSchema#string"/>
        <rdfs:comment>Represents the raw materials used in the manufacturing process, including name and quantity</rdfs:comment>
    </owl:DatatypeProperty>
    


    <!-- http://www.semanticweb.org/qihan/ontologies/2023/6/untitled-ontology-12#Result_Unit -->

    <owl:DatatypeProperty rdf:about="http://www.semanticweb.org/qihan/ontologies/2023/6/untitled-ontology-12#Result_Unit">
        <rdfs:domain rdf:resource="http://www.semanticweb.org/qihan/ontologies/2023/6/untitled-ontology-12#Result_Calculation"/>
        <rdfs:domain rdf:resource="http://www.semanticweb.org/qihan/ontologies/2023/6/untitled-ontology-12#Statistical_Analysis"/>
        <rdfs:range rdf:resource="http://www.w3.org/2001/XMLSchema#string"/>
        <rdfs:comment>Represents the unit of measurement for a test result, such as &quot;MPa&quot; for strength or &quot;J/m²&quot; for fracture toughness.</rdfs:comment>
    </owl:DatatypeProperty>
    


    <!-- http://www.semanticweb.org/qihan/ontologies/2023/6/untitled-ontology-12#Result_Value -->

    <owl:DatatypeProperty rdf:about="http://www.semanticweb.org/qihan/ontologies/2023/6/untitled-ontology-12#Result_Value">
        <rdfs:domain rdf:resource="http://www.semanticweb.org/qihan/ontologies/2023/6/untitled-ontology-12#Result_Calculation"/>
        <rdfs:domain rdf:resource="http://www.semanticweb.org/qihan/ontologies/2023/6/untitled-ontology-12#Statistical_Analysis"/>
        <rdfs:range rdf:resource="http://www.w3.org/2001/XMLSchema#decimal"/>
        <rdfs:range rdf:resource="http://www.w3.org/2001/XMLSchema#float"/>
        <rdfs:comment>Represents the specific value or measurement of a test result</rdfs:comment>
    </owl:DatatypeProperty>
    


    <!-- http://www.semanticweb.org/qihan/ontologies/2023/6/untitled-ontology-12#Specimen_Dimensions -->

    <owl:DatatypeProperty rdf:about="http://www.semanticweb.org/qihan/ontologies/2023/6/untitled-ontology-12#Specimen_Dimensions">
        <rdfs:domain rdf:resource="http://www.semanticweb.org/qihan/ontologies/2023/6/untitled-ontology-12#Test_Specimen_Geometry"/>
        <rdfs:range rdf:resource="http://www.w3.org/2001/XMLSchema#string"/>
        <rdfs:comment>Represents the dimensions or size of a test specimen.</rdfs:comment>
    </owl:DatatypeProperty>
    


    <!-- http://www.semanticweb.org/qihan/ontologies/2023/6/untitled-ontology-12#Specimen_ID -->

    <owl:DatatypeProperty rdf:about="http://www.semanticweb.org/qihan/ontologies/2023/6/untitled-ontology-12#Specimen_ID">
        <rdfs:domain rdf:resource="http://www.semanticweb.org/qihan/ontologies/2023/6/untitled-ontology-12#Test_Specimen_Geometry"/>
        <rdfs:range rdf:resource="http://www.w3.org/2001/XMLSchema#string"/>
        <rdfs:comment>Represents the unique identifier or code assigned to a test specimen.</rdfs:comment>
    </owl:DatatypeProperty>
    


    <!-- 
    ///////////////////////////////////////////////////////////////////////////////////////
    //
    // Classes
    //
    ///////////////////////////////////////////////////////////////////////////////////////
     -->

    


    <!-- http://www.semanticweb.org/qihan/ontologies/2023/6/untitled-ontology-12#ASTM_D2290 -->

    <owl:Class rdf:about="http://www.semanticweb.org/qihan/ontologies/2023/6/untitled-ontology-12#ASTM_D2290">
        <rdfs:subClassOf rdf:resource="http://www.semanticweb.org/qihan/ontologies/2023/6/untitled-ontology-12#Circular_Disk_Specimen"/>
        <rdfs:comment>Represents a standard titled &quot;Standard Test Method for Apparent Hoop Tensile Strength of Plastic or Reinforced Plastic Pipe.&quot;</rdfs:comment>
        <rdfs:label>ASTM D2290</rdfs:label>
    </owl:Class>
    


    <!-- http://www.semanticweb.org/qihan/ontologies/2023/6/untitled-ontology-12#ASTM_D2344 -->

    <owl:Class rdf:about="http://www.semanticweb.org/qihan/ontologies/2023/6/untitled-ontology-12#ASTM_D2344">
        <rdfs:subClassOf rdf:resource="http://www.semanticweb.org/qihan/ontologies/2023/6/untitled-ontology-12#Short_Beam_Specimen"/>
        <rdfs:comment>Represents a standard titled &quot;Standard Test Method for Short-Beam Strength of Polymer Matrix Composite Materials and Their Laminates&quot;.</rdfs:comment>
        <rdfs:label>ASTM D2344</rdfs:label>
    </owl:Class>
    


    <!-- http://www.semanticweb.org/qihan/ontologies/2023/6/untitled-ontology-12#ASTM_D256 -->

    <owl:Class rdf:about="http://www.semanticweb.org/qihan/ontologies/2023/6/untitled-ontology-12#ASTM_D256">
        <rdfs:subClassOf rdf:resource="http://www.semanticweb.org/qihan/ontologies/2023/6/untitled-ontology-12#Impact_Testing"/>
        <rdfs:comment>Represents a specific ASTM standard titled &quot;Standard Test Methods for Determining the Izod Pendulum Impact Resistance of Plastics&quot;.</rdfs:comment>
        <rdfs:label>ASTM D256</rdfs:label>
    </owl:Class>
    


    <!-- http://www.semanticweb.org/qihan/ontologies/2023/6/untitled-ontology-12#ASTM_D2990 -->

    <owl:Class rdf:about="http://www.semanticweb.org/qihan/ontologies/2023/6/untitled-ontology-12#ASTM_D2990">
        <rdfs:subClassOf rdf:resource="http://www.semanticweb.org/qihan/ontologies/2023/6/untitled-ontology-12#Creep_Testing"/>
        <rdfs:comment>ASTM D2990</rdfs:comment>
        <rdfs:comment>Represents a specific ASTM standard titled &quot;Standard Test Methods for Tensile, Compressive, and Flexural Creep and Creep-Rupture of PlasticS&quot;.</rdfs:comment>
    </owl:Class>
    


    <!-- http://www.semanticweb.org/qihan/ontologies/2023/6/untitled-ontology-12#ASTM_D3039 -->

    <owl:Class rdf:about="http://www.semanticweb.org/qihan/ontologies/2023/6/untitled-ontology-12#ASTM_D3039">
        <rdfs:subClassOf rdf:resource="http://www.semanticweb.org/qihan/ontologies/2023/6/untitled-ontology-12#ASTM_Standards"/>
        <rdfs:subClassOf rdf:resource="http://www.semanticweb.org/qihan/ontologies/2023/6/untitled-ontology-12#Tensile_Testing"/>
        <rdfs:comment>Represents a Standard Test Method for Tensile Properties of Polymer Matrix Composite Materials</rdfs:comment>
        <rdfs:label>ASTM D3039</rdfs:label>
    </owl:Class>
    


    <!-- http://www.semanticweb.org/qihan/ontologies/2023/6/untitled-ontology-12#ASTM_D3167 -->

    <owl:Class rdf:about="http://www.semanticweb.org/qihan/ontologies/2023/6/untitled-ontology-12#ASTM_D3167">
        <rdfs:subClassOf rdf:resource="http://www.semanticweb.org/qihan/ontologies/2023/6/untitled-ontology-12#Peel_Testing"/>
        <rdfs:comment>Represents a specific ASTM standard that outlines the test method for measuring the peel strength of adhesives and adhesive-coated materials.</rdfs:comment>
        <rdfs:label>ASTM D3167</rdfs:label>
    </owl:Class>
    


    <!-- http://www.semanticweb.org/qihan/ontologies/2023/6/untitled-ontology-12#ASTM_D3410 -->

    <owl:Class rdf:about="http://www.semanticweb.org/qihan/ontologies/2023/6/untitled-ontology-12#ASTM_D3410">
        <rdfs:subClassOf rdf:resource="http://www.semanticweb.org/qihan/ontologies/2023/6/untitled-ontology-12#Compression_Testing"/>
        <rdfs:comment>Represents a specific ASTM standard titled &quot;Standard Test Method for Compressive Properties of Polymer Matrix Composite Materials&quot;.</rdfs:comment>
        <rdfs:label>ASTM D3410</rdfs:label>
    </owl:Class>
    


    <!-- http://www.semanticweb.org/qihan/ontologies/2023/6/untitled-ontology-12#ASTM_D3479 -->

    <owl:Class rdf:about="http://www.semanticweb.org/qihan/ontologies/2023/6/untitled-ontology-12#ASTM_D3479">
        <rdfs:subClassOf rdf:resource="http://www.semanticweb.org/qihan/ontologies/2023/6/untitled-ontology-12#Fatigue_Testing"/>
        <rdfs:comment>Represents a specific ASTM standard titled &quot;Standard Test Method for Tension-Tension Fatigue of Polymer Matrix Composite Materials&quot;.</rdfs:comment>
        <rdfs:label>ASTM D3479</rdfs:label>
    </owl:Class>
    


    <!-- http://www.semanticweb.org/qihan/ontologies/2023/6/untitled-ontology-12#ASTM_D3518 -->

    <owl:Class rdf:about="http://www.semanticweb.org/qihan/ontologies/2023/6/untitled-ontology-12#ASTM_D3518">
        <rdfs:subClassOf rdf:resource="http://www.semanticweb.org/qihan/ontologies/2023/6/untitled-ontology-12#Flat_Plate_Specimen"/>
        <rdfs:comment>Represents a standard titled &quot;Standard Test Method for In-Plane Shear Response of Polymer Matrix Composite Materials by Tensile Test of a ±45° Laminate&quot;.</rdfs:comment>
        <rdfs:label>ASTM D3518</rdfs:label>
    </owl:Class>
    


    <!-- http://www.semanticweb.org/qihan/ontologies/2023/6/untitled-ontology-12#ASTM_D5045 -->

    <owl:Class rdf:about="http://www.semanticweb.org/qihan/ontologies/2023/6/untitled-ontology-12#ASTM_D5045">
        <rdfs:subClassOf rdf:resource="http://www.semanticweb.org/qihan/ontologies/2023/6/untitled-ontology-12#End-Notched_Flexure_Specimen"/>
        <rdfs:subClassOf rdf:resource="http://www.semanticweb.org/qihan/ontologies/2023/6/untitled-ontology-12#Fracture_Toughness_Testing"/>
        <rdfs:comment>Represents a specific ASTM standard titled &quot;Standard Test Method for Plane-Strain Fracture Toughness of Metallic Materials&quot;.</rdfs:comment>
        <rdfs:label>ASTM D5045</rdfs:label>
    </owl:Class>
    


    <!-- http://www.semanticweb.org/qihan/ontologies/2023/6/untitled-ontology-12#ASTM_D5379 -->

    <owl:Class rdf:about="http://www.semanticweb.org/qihan/ontologies/2023/6/untitled-ontology-12#ASTM_D5379">
        <rdfs:subClassOf rdf:resource="http://www.semanticweb.org/qihan/ontologies/2023/6/untitled-ontology-12#ASTM_Standards"/>
        <rdfs:subClassOf rdf:resource="http://www.semanticweb.org/qihan/ontologies/2023/6/untitled-ontology-12#Shear_Testing"/>
        <rdfs:subClassOf rdf:resource="http://www.semanticweb.org/qihan/ontologies/2023/6/untitled-ontology-12#V-Notched_Beam_Specimen"/>
        <rdfs:comment>Represents the Standard Test Method for Shear Properties of Composite Materials by the V-Notched Beam Method</rdfs:comment>
        <rdfs:label>ASTM D5379</rdfs:label>
    </owl:Class>
    


    <!-- http://www.semanticweb.org/qihan/ontologies/2023/6/untitled-ontology-12#ASTM_D5448 -->

    <owl:Class rdf:about="http://www.semanticweb.org/qihan/ontologies/2023/6/untitled-ontology-12#ASTM_D5448">
        <rdfs:subClassOf rdf:resource="http://www.semanticweb.org/qihan/ontologies/2023/6/untitled-ontology-12#Hourglass_Specimen"/>
        <rdfs:comment>Represents a standard titled &quot;Standard Test Method for Inplane Shear Properties of Hoop Wound Polymer Matrix Composite Cylinders&quot;.</rdfs:comment>
        <rdfs:label>ASTM D5448</rdfs:label>
    </owl:Class>
    


    <!-- http://www.semanticweb.org/qihan/ontologies/2023/6/untitled-ontology-12#ASTM_D5528 -->

    <owl:Class rdf:about="http://www.semanticweb.org/qihan/ontologies/2023/6/untitled-ontology-12#ASTM_D5528">
        <rdfs:subClassOf rdf:resource="http://www.semanticweb.org/qihan/ontologies/2023/6/untitled-ontology-12#Double_Cantilever_Beam_Specimen"/>
        <rdfs:comment>Represents a standard titled &quot;Standard Test Method for Mode I Interlaminar Fracture Toughness of Unidirectional Fiber-Reinforced Polymer Matrix Composites&quot;.</rdfs:comment>
        <rdfs:label>ASTM D5528</rdfs:label>
    </owl:Class>
    


    <!-- http://www.semanticweb.org/qihan/ontologies/2023/6/untitled-ontology-12#ASTM_D5868 -->

    <owl:Class rdf:about="http://www.semanticweb.org/qihan/ontologies/2023/6/untitled-ontology-12#ASTM_D5868">
        <rdfs:subClassOf rdf:resource="http://www.semanticweb.org/qihan/ontologies/2023/6/untitled-ontology-12#Shear-Lap_Testing"/>
        <rdfs:comment>Represents a specific ASTM standard that provides the test method for measuring the lap shear strength of adhesively bonded metal specimens.</rdfs:comment>
        <rdfs:label>ASTM D5868</rdfs:label>
    </owl:Class>
    


    <!-- http://www.semanticweb.org/qihan/ontologies/2023/6/untitled-ontology-12#ASTM_D6272 -->

    <owl:Class rdf:about="http://www.semanticweb.org/qihan/ontologies/2023/6/untitled-ontology-12#ASTM_D6272">
        <rdfs:subClassOf rdf:resource="http://www.semanticweb.org/qihan/ontologies/2023/6/untitled-ontology-12#Four-Point_Bending_Specimen"/>
        <rdfs:comment>Represents a standard titled &quot;Standard Test Method for Flexural Properties of Unreinforced and Reinforced Plastics and Electrical Insulating Materials&quot;.</rdfs:comment>
        <rdfs:label>ASTM D6272</rdfs:label>
    </owl:Class>
    


    <!-- http://www.semanticweb.org/qihan/ontologies/2023/6/untitled-ontology-12#ASTM_D638 -->

    <owl:Class rdf:about="http://www.semanticweb.org/qihan/ontologies/2023/6/untitled-ontology-12#ASTM_D638">
        <rdfs:subClassOf rdf:resource="http://www.semanticweb.org/qihan/ontologies/2023/6/untitled-ontology-12#Dogbone_Specimen"/>
        <rdfs:comment>Represents a standard titled &quot;Standard Test Method for Tensile Properties of Plastics&quot;.</rdfs:comment>
        <rdfs:label>ASTM D638</rdfs:label>
    </owl:Class>
    


    <!-- http://www.semanticweb.org/qihan/ontologies/2023/6/untitled-ontology-12#ASTM_D790 -->

    <owl:Class rdf:about="http://www.semanticweb.org/qihan/ontologies/2023/6/untitled-ontology-12#ASTM_D790">
        <rdfs:subClassOf rdf:resource="http://www.semanticweb.org/qihan/ontologies/2023/6/untitled-ontology-12#ASTM_Standards"/>
        <rdfs:subClassOf rdf:resource="http://www.semanticweb.org/qihan/ontologies/2023/6/untitled-ontology-12#Cantilever_Beam_Specimen"/>
        <rdfs:subClassOf rdf:resource="http://www.semanticweb.org/qihan/ontologies/2023/6/untitled-ontology-12#Flexural_Testing"/>
        <rdfs:subClassOf rdf:resource="http://www.semanticweb.org/qihan/ontologies/2023/6/untitled-ontology-12#Three-Point_Bending_Specimen"/>
        <rdfs:comment>Standard Test Methods for Flexural Properties of Unreinforced and Reinforced Plastics and Electrical Insulating Materials</rdfs:comment>
        <rdfs:label>ASYM D790</rdfs:label>
    </owl:Class>
    


    <!-- http://www.semanticweb.org/qihan/ontologies/2023/6/untitled-ontology-12#ASTM_E399 -->

    <owl:Class rdf:about="http://www.semanticweb.org/qihan/ontologies/2023/6/untitled-ontology-12#ASTM_E399">
        <rdfs:subClassOf rdf:resource="http://www.semanticweb.org/qihan/ontologies/2023/6/untitled-ontology-12#Fracture_Toughness_Testing"/>
        <rdfs:label>ASTM E399</rdfs:label>
        <rdfs:label>Represents a specific ASTM standard titled &quot;Standard Test Method for Plane-Strain Fracture Toughness of Metallic Materials&quot;.</rdfs:label>
    </owl:Class>
    


    <!-- http://www.semanticweb.org/qihan/ontologies/2023/6/untitled-ontology-12#ASTM_Standards -->

    <owl:Class rdf:about="http://www.semanticweb.org/qihan/ontologies/2023/6/untitled-ontology-12#ASTM_Standards">
        <rdfs:subClassOf rdf:resource="http://www.semanticweb.org/qihan/ontologies/2023/6/untitled-ontology-12#Test_Standards"/>
        <rdfs:label>American Society for Testing and Materials (ASTM)</rdfs:label>
    </owl:Class>
    


    <!-- http://www.semanticweb.org/qihan/ontologies/2023/6/untitled-ontology-12#Abrasion_Testing_Machine -->

    <owl:Class rdf:about="http://www.semanticweb.org/qihan/ontologies/2023/6/untitled-ontology-12#Abrasion_Testing_Machine">
        <rdfs:subClassOf rdf:resource="http://www.semanticweb.org/qihan/ontologies/2023/6/untitled-ontology-12#Test_Equipment"/>
        <rdfs:comment>Represents a specific type of test equipment used to test the abrasive resistance of solid materials. It applies controlled abrasive forces to assess material durability and surface degradation.</rdfs:comment>
        <rdfs:label>Abrasion Testing Machine</rdfs:label>
    </owl:Class>
    


    <!-- http://www.semanticweb.org/qihan/ontologies/2023/6/untitled-ontology-12#Abrasive_Saw -->

    <owl:Class rdf:about="http://www.semanticweb.org/qihan/ontologies/2023/6/untitled-ontology-12#Abrasive_Saw">
        <rdfs:subClassOf rdf:resource="http://www.semanticweb.org/qihan/ontologies/2023/6/untitled-ontology-12#Sectioning_Equipment"/>
        <rdfs:comment>Represents a type of cutting tool equipped with an abrasive disc or wheel used for sectioning hard and dense materials.</rdfs:comment>
        <rdfs:label>Abrasive Saw</rdfs:label>
    </owl:Class>
    


    <!-- http://www.semanticweb.org/qihan/ontologies/2023/6/untitled-ontology-12#Acceleration -->

    <owl:Class rdf:about="http://www.semanticweb.org/qihan/ontologies/2023/6/untitled-ontology-12#Acceleration">
        <rdfs:subClassOf rdf:resource="http://www.semanticweb.org/qihan/ontologies/2023/6/untitled-ontology-12#Test_Parameter"/>
        <rdfs:comment>Represents a physical quantity that measures the rate of change of velocity of a material or object. It is an important parameter in mechanical testing to assess the material&apos;s response to dynamic forces.</rdfs:comment>
        <rdfs:label>Acceleration</rdfs:label>
    </owl:Class>
    


    <!-- http://www.semanticweb.org/qihan/ontologies/2023/6/untitled-ontology-12#Acoustic_Absorption_Coefficient -->

    <owl:Class rdf:about="http://www.semanticweb.org/qihan/ontologies/2023/6/untitled-ontology-12#Acoustic_Absorption_Coefficient">
        <rdfs:subClassOf rdf:resource="http://www.semanticweb.org/qihan/ontologies/2023/6/untitled-ontology-12#Acoustic_Properties"/>
    </owl:Class>
    


    <!-- http://www.semanticweb.org/qihan/ontologies/2023/6/untitled-ontology-12#Acoustic_Properties -->

    <owl:Class rdf:about="http://www.semanticweb.org/qihan/ontologies/2023/6/untitled-ontology-12#Acoustic_Properties">
        <rdfs:subClassOf rdf:resource="http://www.semanticweb.org/qihan/ontologies/2023/6/untitled-ontology-12#Result_Calculation"/>
    </owl:Class>
    


    <!-- http://www.semanticweb.org/qihan/ontologies/2023/6/untitled-ontology-12#Additive_Manufacturing_Processes -->

    <owl:Class rdf:about="http://www.semanticweb.org/qihan/ontologies/2023/6/untitled-ontology-12#Additive_Manufacturing_Processes">
        <rdfs:subClassOf rdf:resource="http://www.semanticweb.org/qihan/ontologies/2023/6/untitled-ontology-12#Material_Manufacturing"/>
        <rdfs:comment>Represents a group of manufacturing techniques that build objects layer by layer by adding material.</rdfs:comment>
        <rdfs:label>Additive Manufacturing Processes</rdfs:label>
    </owl:Class>
    


    <!-- http://www.semanticweb.org/qihan/ontologies/2023/6/untitled-ontology-12#Adhesive_Strength -->

    <owl:Class rdf:about="http://www.semanticweb.org/qihan/ontologies/2023/6/untitled-ontology-12#Adhesive_Strength">
        <rdfs:subClassOf rdf:resource="http://www.semanticweb.org/qihan/ontologies/2023/6/untitled-ontology-12#Result_Calculation"/>
    </owl:Class>
    


    <!-- http://www.semanticweb.org/qihan/ontologies/2023/6/untitled-ontology-12#Aging_Properties -->

    <owl:Class rdf:about="http://www.semanticweb.org/qihan/ontologies/2023/6/untitled-ontology-12#Aging_Properties">
        <rdfs:subClassOf rdf:resource="http://www.semanticweb.org/qihan/ontologies/2023/6/untitled-ontology-12#Result_Calculation"/>
    </owl:Class>
    


    <!-- http://www.semanticweb.org/qihan/ontologies/2023/6/untitled-ontology-12#Air -->

    <owl:Class rdf:about="http://www.semanticweb.org/qihan/ontologies/2023/6/untitled-ontology-12#Air">
        <rdfs:subClassOf rdf:resource="http://www.semanticweb.org/qihan/ontologies/2023/6/untitled-ontology-12#Medium"/>
        <rdfs:comment>Represents the medium of the testing environment for mechanical testing of composite material specimens. It refers to atmospheric air surrounding the specimens during testing.</rdfs:comment>
        <rdfs:label>Air</rdfs:label>
    </owl:Class>
    


    <!-- http://www.semanticweb.org/qihan/ontologies/2023/6/untitled-ontology-12#Aluminum_Core_Composite -->

    <owl:Class rdf:about="http://www.semanticweb.org/qihan/ontologies/2023/6/untitled-ontology-12#Aluminum_Core_Composite">
        <rdfs:subClassOf rdf:resource="http://www.semanticweb.org/qihan/ontologies/2023/6/untitled-ontology-12#Sandwich_Composite"/>
    </owl:Class>
    


    <!-- http://www.semanticweb.org/qihan/ontologies/2023/6/untitled-ontology-12#Aluminum_Matrix_Composite -->

    <owl:Class rdf:about="http://www.semanticweb.org/qihan/ontologies/2023/6/untitled-ontology-12#Aluminum_Matrix_Composite">
        <rdfs:subClassOf rdf:resource="http://www.semanticweb.org/qihan/ontologies/2023/6/untitled-ontology-12#Metal_Matrix_Composite"/>
    </owl:Class>
    


    <!-- http://www.semanticweb.org/qihan/ontologies/2023/6/untitled-ontology-12#Aluminum_Oxide_Matrix_Composite -->

    <owl:Class rdf:about="http://www.semanticweb.org/qihan/ontologies/2023/6/untitled-ontology-12#Aluminum_Oxide_Matrix_Composite">
        <rdfs:subClassOf rdf:resource="http://www.semanticweb.org/qihan/ontologies/2023/6/untitled-ontology-12#Ceramic_Matrix_Composite"/>
    </owl:Class>
    


    <!-- http://www.semanticweb.org/qihan/ontologies/2023/6/untitled-ontology-12#Ambient_Temperature -->

    <owl:Class rdf:about="http://www.semanticweb.org/qihan/ontologies/2023/6/untitled-ontology-12#Ambient_Temperature">
        <rdfs:subClassOf rdf:resource="http://www.semanticweb.org/qihan/ontologies/2023/6/untitled-ontology-12#Temperature"/>
        <rdfs:comment>Represents the prevailing temperature of the surrounding environment during mechanical testing of composite material specimens. It refers to the standard or room temperature conditions.</rdfs:comment>
        <rdfs:label>Ambient Temperature</rdfs:label>
    </owl:Class>
    


    <!-- http://www.semanticweb.org/qihan/ontologies/2023/6/untitled-ontology-12#Angular_Orientation -->

    <owl:Class rdf:about="http://www.semanticweb.org/qihan/ontologies/2023/6/untitled-ontology-12#Angular_Orientation">
        <rdfs:subClassOf rdf:resource="http://www.semanticweb.org/qihan/ontologies/2023/6/untitled-ontology-12#Orientation"/>
        <rdfs:comment>Represents the orientation of a material with respect to a specific angle or direction.</rdfs:comment>
        <rdfs:label>Angular Orientation</rdfs:label>
    </owl:Class>
    


    <!-- http://www.semanticweb.org/qihan/ontologies/2023/6/untitled-ontology-12#Applied_Electric_Field -->

    <owl:Class rdf:about="http://www.semanticweb.org/qihan/ontologies/2023/6/untitled-ontology-12#Applied_Electric_Field">
        <rdfs:subClassOf rdf:resource="http://www.semanticweb.org/qihan/ontologies/2023/6/untitled-ontology-12#Electric_Field"/>
        <rdfs:comment>Represents the external electric field that is intentionally applied to a material.</rdfs:comment>
        <rdfs:label>Applied Electric Field</rdfs:label>
    </owl:Class>
    


    <!-- http://www.semanticweb.org/qihan/ontologies/2023/6/untitled-ontology-12#Applied_Magnetic_Field -->

    <owl:Class rdf:about="http://www.semanticweb.org/qihan/ontologies/2023/6/untitled-ontology-12#Applied_Magnetic_Field">
        <rdfs:subClassOf rdf:resource="http://www.semanticweb.org/qihan/ontologies/2023/6/untitled-ontology-12#Magnetic_Field"/>
        <rdfs:comment>Represents the external magnetic field that is intentionally applied to a material.</rdfs:comment>
        <rdfs:label>Applied Magnetic Field</rdfs:label>
    </owl:Class>
    


    <!-- http://www.semanticweb.org/qihan/ontologies/2023/6/untitled-ontology-12#Applied_Pressure -->

    <owl:Class rdf:about="http://www.semanticweb.org/qihan/ontologies/2023/6/untitled-ontology-12#Applied_Pressure">
        <rdfs:subClassOf rdf:resource="http://www.semanticweb.org/qihan/ontologies/2023/6/untitled-ontology-12#Pressure_Condition"/>
        <rdfs:comment>Represents the pressure applied to composite material specimens during mechanical testing. It includes specific levels of compression or tension used in different testing methods.</rdfs:comment>
        <rdfs:label>Applied Pressure</rdfs:label>
    </owl:Class>
    


    <!-- http://www.semanticweb.org/qihan/ontologies/2023/6/untitled-ontology-12#Aramid_Fibre_Reinforced_Polymer -->

    <owl:Class rdf:about="http://www.semanticweb.org/qihan/ontologies/2023/6/untitled-ontology-12#Aramid_Fibre_Reinforced_Polymer">
        <rdfs:subClassOf rdf:resource="http://www.semanticweb.org/qihan/ontologies/2023/6/untitled-ontology-12#Polymer_Matrix_Composite"/>
    </owl:Class>
    


    <!-- http://www.semanticweb.org/qihan/ontologies/2023/6/untitled-ontology-12#Atmospheric_Pressure -->

    <owl:Class rdf:about="http://www.semanticweb.org/qihan/ontologies/2023/6/untitled-ontology-12#Atmospheric_Pressure">
        <rdfs:subClassOf rdf:resource="http://www.semanticweb.org/qihan/ontologies/2023/6/untitled-ontology-12#Pressure_Condition"/>
        <rdfs:comment>Represents the pressure of the surrounding air in the testing environment during mechanical testing of composite material specimens.</rdfs:comment>
        <rdfs:label>Atmospheric Pressure</rdfs:label>
    </owl:Class>
    


    <!-- http://www.semanticweb.org/qihan/ontologies/2023/6/untitled-ontology-12#Autoclave_Curing_Process -->

    <owl:Class rdf:about="http://www.semanticweb.org/qihan/ontologies/2023/6/untitled-ontology-12#Autoclave_Curing_Process">
        <rdfs:subClassOf rdf:resource="http://www.semanticweb.org/qihan/ontologies/2023/6/untitled-ontology-12#Material_Manufacturing"/>
        <rdfs:comment>Represents a manufacturing process used to cure composite materials, especially pre-impregnated materials (prepregs), under controlled high-temperature and pressure conditions.</rdfs:comment>
        <rdfs:label>Autoclave Curing Process</rdfs:label>
    </owl:Class>
    


    <!-- http://www.semanticweb.org/qihan/ontologies/2023/6/untitled-ontology-12#Automated_Fiber_Placement -->

    <owl:Class rdf:about="http://www.semanticweb.org/qihan/ontologies/2023/6/untitled-ontology-12#Automated_Fiber_Placement">
        <rdfs:subClassOf rdf:resource="http://www.semanticweb.org/qihan/ontologies/2023/6/untitled-ontology-12#Layup_Processes"/>
        <rdfs:comment>Represents a specific layup process that uses automated machinery to precisely place and align continuous fibers onto a mandrel or mold to create a composite structure.</rdfs:comment>
        <rdfs:label>Automated Fiber Placement</rdfs:label>
    </owl:Class>
    


    <!-- http://www.semanticweb.org/qihan/ontologies/2023/6/untitled-ontology-12#Automated_Tape_Layup -->

    <owl:Class rdf:about="http://www.semanticweb.org/qihan/ontologies/2023/6/untitled-ontology-12#Automated_Tape_Layup">
        <rdfs:subClassOf rdf:resource="http://www.semanticweb.org/qihan/ontologies/2023/6/untitled-ontology-12#Layup_Processes"/>
        <rdfs:comment>Represents a specific layup process where continuous fiber tapes are automatically placed onto a mold or tool to form a composite structure.</rdfs:comment>
        <rdfs:label>Automated Tape Layup</rdfs:label>
    </owl:Class>
    


    <!-- http://www.semanticweb.org/qihan/ontologies/2023/6/untitled-ontology-12#Axes -->

    <owl:Class rdf:about="http://www.semanticweb.org/qihan/ontologies/2023/6/untitled-ontology-12#Axes">
        <rdfs:subClassOf rdf:resource="http://www.semanticweb.org/qihan/ontologies/2023/6/untitled-ontology-12#Handheld_Cutting_Tools"/>
        <rdfs:comment>Represents a type of cutting tool.</rdfs:comment>
        <rdfs:label>Axes</rdfs:label>
    </owl:Class>
    


    <!-- http://www.semanticweb.org/qihan/ontologies/2023/6/untitled-ontology-12#Axial_Displacement -->

    <owl:Class rdf:about="http://www.semanticweb.org/qihan/ontologies/2023/6/untitled-ontology-12#Axial_Displacement">
        <rdfs:subClassOf rdf:resource="http://www.semanticweb.org/qihan/ontologies/2023/6/untitled-ontology-12#Displacement"/>
        <rdfs:comment>Represents the displacement or movement of a material, along the axis of the applied force or load.</rdfs:comment>
        <rdfs:label>Axial Displacement</rdfs:label>
    </owl:Class>
    


    <!-- http://www.semanticweb.org/qihan/ontologies/2023/6/untitled-ontology-12#Axial_Fatigue_Testing_Machine -->

    <owl:Class rdf:about="http://www.semanticweb.org/qihan/ontologies/2023/6/untitled-ontology-12#Axial_Fatigue_Testing_Machine">
        <rdfs:subClassOf rdf:resource="http://www.semanticweb.org/qihan/ontologies/2023/6/untitled-ontology-12#Fatigue_Testing_Machine"/>
        <rdfs:comment>Represents a specific type of testing machine used for conducting fatigue tests on composite material specimens under axial loading conditions. It applies cyclic axial loads to assess the material&apos;s fatigue life and behavior under tension-compression loading.</rdfs:comment>
        <rdfs:label>Axial Fatigue Testing Machine</rdfs:label>
    </owl:Class>
    


    <!-- http://www.semanticweb.org/qihan/ontologies/2023/6/untitled-ontology-12#Axial_Filament_Winding -->

    <owl:Class rdf:about="http://www.semanticweb.org/qihan/ontologies/2023/6/untitled-ontology-12#Axial_Filament_Winding">
        <rdfs:subClassOf rdf:resource="http://www.semanticweb.org/qihan/ontologies/2023/6/untitled-ontology-12#Filament_Winding_Processes"/>
        <rdfs:comment>Represents a specific filament winding process where continuous fibers are wound along the length (axial direction) of a mandrel or mold.</rdfs:comment>
        <rdfs:label>Axial Filament Winding</rdfs:label>
    </owl:Class>
    


    <!-- http://www.semanticweb.org/qihan/ontologies/2023/6/untitled-ontology-12#Axial_Strain -->

    <owl:Class rdf:about="http://www.semanticweb.org/qihan/ontologies/2023/6/untitled-ontology-12#Axial_Strain">
        <rdfs:subClassOf rdf:resource="http://www.semanticweb.org/qihan/ontologies/2023/6/untitled-ontology-12#Strain"/>
        <rdfs:comment>Represents the change in length or deformation along the longitudinal axis of a material under an applied axial load.</rdfs:comment>
        <rdfs:label>Axial Strain</rdfs:label>
    </owl:Class>
    


    <!-- http://www.semanticweb.org/qihan/ontologies/2023/6/untitled-ontology-12#BMC_Compression_Molding -->

    <owl:Class rdf:about="http://www.semanticweb.org/qihan/ontologies/2023/6/untitled-ontology-12#BMC_Compression_Molding">
        <rdfs:subClassOf rdf:resource="http://www.semanticweb.org/qihan/ontologies/2023/6/untitled-ontology-12#Bulk_Molding_Compound_Processes"/>
        <rdfs:comment>Represents a specific manufacturing process that uses the bulk molding compound (BMC) method to produce composite materials.</rdfs:comment>
        <rdfs:label>BMC Compression Molding</rdfs:label>
    </owl:Class>
    


    <!-- http://www.semanticweb.org/qihan/ontologies/2023/6/untitled-ontology-12#BMC_Fabrication -->

    <owl:Class rdf:about="http://www.semanticweb.org/qihan/ontologies/2023/6/untitled-ontology-12#BMC_Fabrication">
        <rdfs:subClassOf rdf:resource="http://www.semanticweb.org/qihan/ontologies/2023/6/untitled-ontology-12#Bulk_Molding_Compound_Processes"/>
        <rdfs:comment>Represents a category of manufacturing processes that utilize the bulk molding compound (BMC) method to fabricate composite materials.</rdfs:comment>
        <rdfs:label>BMC Fabrication</rdfs:label>
    </owl:Class>
    


    <!-- http://www.semanticweb.org/qihan/ontologies/2023/6/untitled-ontology-12#BS_EN_ISO_14125 -->

    <owl:Class rdf:about="http://www.semanticweb.org/qihan/ontologies/2023/6/untitled-ontology-12#BS_EN_ISO_14125">
        <rdfs:subClassOf rdf:resource="http://www.semanticweb.org/qihan/ontologies/2023/6/untitled-ontology-12#BS_Standards"/>
        <rdfs:comment>Fibre-reinforced plastic composites - Determination of flexural properties</rdfs:comment>
        <rdfs:label>BS EN ISO 14125</rdfs:label>
    </owl:Class>
    


    <!-- http://www.semanticweb.org/qihan/ontologies/2023/6/untitled-ontology-12#BS_EN_ISO_178 -->

    <owl:Class rdf:about="http://www.semanticweb.org/qihan/ontologies/2023/6/untitled-ontology-12#BS_EN_ISO_178">
        <rdfs:subClassOf rdf:resource="http://www.semanticweb.org/qihan/ontologies/2023/6/untitled-ontology-12#BS_Standards"/>
        <rdfs:comment>Plastics - Determination of Flexural Properties</rdfs:comment>
        <rdfs:label>BS EN ISO 178</rdfs:label>
    </owl:Class>
    


    <!-- http://www.semanticweb.org/qihan/ontologies/2023/6/untitled-ontology-12#BS_EN_ISO_527 -->

    <owl:Class rdf:about="http://www.semanticweb.org/qihan/ontologies/2023/6/untitled-ontology-12#BS_EN_ISO_527">
        <rdfs:subClassOf rdf:resource="http://www.semanticweb.org/qihan/ontologies/2023/6/untitled-ontology-12#BS_Standards"/>
        <rdfs:comment>Plastics - Determination of Tensile Properties</rdfs:comment>
        <rdfs:label>BS EN ISO 527</rdfs:label>
    </owl:Class>
    


    <!-- http://www.semanticweb.org/qihan/ontologies/2023/6/untitled-ontology-12#BS_Standards -->

    <owl:Class rdf:about="http://www.semanticweb.org/qihan/ontologies/2023/6/untitled-ontology-12#BS_Standards">
        <rdfs:subClassOf rdf:resource="http://www.semanticweb.org/qihan/ontologies/2023/6/untitled-ontology-12#Test_Standards"/>
        <rdfs:label>British Standards (BS)</rdfs:label>
    </owl:Class>
    


    <!-- http://www.semanticweb.org/qihan/ontologies/2023/6/untitled-ontology-12#Balsa_Wood_Core_Composite -->

    <owl:Class rdf:about="http://www.semanticweb.org/qihan/ontologies/2023/6/untitled-ontology-12#Balsa_Wood_Core_Composite">
        <rdfs:subClassOf rdf:resource="http://www.semanticweb.org/qihan/ontologies/2023/6/untitled-ontology-12#Sandwich_Composite"/>
    </owl:Class>
    


    <!-- http://www.semanticweb.org/qihan/ontologies/2023/6/untitled-ontology-12#Bamboo_Composite -->

    <owl:Class rdf:about="http://www.semanticweb.org/qihan/ontologies/2023/6/untitled-ontology-12#Bamboo_Composite">
        <rdfs:subClassOf rdf:resource="http://www.semanticweb.org/qihan/ontologies/2023/6/untitled-ontology-12#Natural_Fiber_Composite"/>
    </owl:Class>
    


    <!-- http://www.semanticweb.org/qihan/ontologies/2023/6/untitled-ontology-12#Belt_Grinder -->

    <owl:Class rdf:about="http://www.semanticweb.org/qihan/ontologies/2023/6/untitled-ontology-12#Belt_Grinder">
        <rdfs:subClassOf rdf:resource="http://www.semanticweb.org/qihan/ontologies/2023/6/untitled-ontology-12#Grinding_and_Sanding_Equipment"/>
        <rdfs:comment>Represents a type of grinding machine equipped with an abrasive belt that rotates on two or more pulleys.</rdfs:comment>
        <rdfs:label>Belt Grinder</rdfs:label>
    </owl:Class>
    


    <!-- http://www.semanticweb.org/qihan/ontologies/2023/6/untitled-ontology-12#Bidirectional_Composite -->

    <owl:Class rdf:about="http://www.semanticweb.org/qihan/ontologies/2023/6/untitled-ontology-12#Bidirectional_Composite">
        <rdfs:subClassOf rdf:resource="http://www.semanticweb.org/qihan/ontologies/2023/6/untitled-ontology-12#Continuous_Fiber_Composite"/>
    </owl:Class>
    


    <!-- http://www.semanticweb.org/qihan/ontologies/2023/6/untitled-ontology-12#Bio-based_Composite -->

    <owl:Class rdf:about="http://www.semanticweb.org/qihan/ontologies/2023/6/untitled-ontology-12#Bio-based_Composite">
        <rdfs:subClassOf rdf:resource="http://www.semanticweb.org/qihan/ontologies/2023/6/untitled-ontology-12#Composite_Material"/>
    </owl:Class>
    


    <!-- http://www.semanticweb.org/qihan/ontologies/2023/6/untitled-ontology-12#Biofiber_Reinforced_Composite -->

    <owl:Class rdf:about="http://www.semanticweb.org/qihan/ontologies/2023/6/untitled-ontology-12#Biofiber_Reinforced_Composite">
        <rdfs:subClassOf rdf:resource="http://www.semanticweb.org/qihan/ontologies/2023/6/untitled-ontology-12#Bio-based_Composite"/>
    </owl:Class>
    


    <!-- http://www.semanticweb.org/qihan/ontologies/2023/6/untitled-ontology-12#Biopolymer_Matrix_Composite -->

    <owl:Class rdf:about="http://www.semanticweb.org/qihan/ontologies/2023/6/untitled-ontology-12#Biopolymer_Matrix_Composite">
        <rdfs:subClassOf rdf:resource="http://www.semanticweb.org/qihan/ontologies/2023/6/untitled-ontology-12#Bio-based_Composite"/>
    </owl:Class>
    


    <!-- http://www.semanticweb.org/qihan/ontologies/2023/6/untitled-ontology-12#Bond_Strength -->

    <owl:Class rdf:about="http://www.semanticweb.org/qihan/ontologies/2023/6/untitled-ontology-12#Bond_Strength">
        <rdfs:subClassOf rdf:resource="http://www.semanticweb.org/qihan/ontologies/2023/6/untitled-ontology-12#Adhesive_Strength"/>
    </owl:Class>
    


    <!-- http://www.semanticweb.org/qihan/ontologies/2023/6/untitled-ontology-12#Braided_Composite -->

    <owl:Class rdf:about="http://www.semanticweb.org/qihan/ontologies/2023/6/untitled-ontology-12#Braided_Composite">
        <rdfs:subClassOf rdf:resource="http://www.semanticweb.org/qihan/ontologies/2023/6/untitled-ontology-12#Continuous_Fiber_Composite"/>
    </owl:Class>
    


    <!-- http://www.semanticweb.org/qihan/ontologies/2023/6/untitled-ontology-12#Brinell_Hardness -->

    <owl:Class rdf:about="http://www.semanticweb.org/qihan/ontologies/2023/6/untitled-ontology-12#Brinell_Hardness">
        <rdfs:subClassOf rdf:resource="http://www.semanticweb.org/qihan/ontologies/2023/6/untitled-ontology-12#Hardness"/>
    </owl:Class>
    


    <!-- http://www.semanticweb.org/qihan/ontologies/2023/6/untitled-ontology-12#Brinell_Hardness_Tester -->

    <owl:Class rdf:about="http://www.semanticweb.org/qihan/ontologies/2023/6/untitled-ontology-12#Brinell_Hardness_Tester">
        <rdfs:subClassOf rdf:resource="http://www.semanticweb.org/qihan/ontologies/2023/6/untitled-ontology-12#Hardness_Tester"/>
        <rdfs:comment>Represents a specific type of hardness tester used to determine the Brinell hardness of materials, including composite material specimens.</rdfs:comment>
        <rdfs:label>Brinell Hardness Tester</rdfs:label>
    </owl:Class>
    


    <!-- http://www.semanticweb.org/qihan/ontologies/2023/6/untitled-ontology-12#Brinell_Hardness_Testing -->

    <owl:Class rdf:about="http://www.semanticweb.org/qihan/ontologies/2023/6/untitled-ontology-12#Brinell_Hardness_Testing">
        <rdfs:subClassOf rdf:resource="http://www.semanticweb.org/qihan/ontologies/2023/6/untitled-ontology-12#Hardness_Testing"/>
        <rdfs:comment>Represents a type of hardness testing method used to determine the hardness of materials, by indenting a hard ball indenter into the material&apos;s surface under a specified load.</rdfs:comment>
        <rdfs:label>Brinell Hardness Testing</rdfs:label>
    </owl:Class>
    


    <!-- http://www.semanticweb.org/qihan/ontologies/2023/6/untitled-ontology-12#Brittle_Fracture -->

    <owl:Class rdf:about="http://www.semanticweb.org/qihan/ontologies/2023/6/untitled-ontology-12#Brittle_Fracture">
        <rdfs:subClassOf rdf:resource="http://www.semanticweb.org/qihan/ontologies/2023/6/untitled-ontology-12#Failure_Mode"/>
    </owl:Class>
    


    <!-- http://www.semanticweb.org/qihan/ontologies/2023/6/untitled-ontology-12#Bulk_Molding_Compound_Processes -->

    <owl:Class rdf:about="http://www.semanticweb.org/qihan/ontologies/2023/6/untitled-ontology-12#Bulk_Molding_Compound_Processes">
        <rdfs:subClassOf rdf:resource="http://www.semanticweb.org/qihan/ontologies/2023/6/untitled-ontology-12#Material_Manufacturing"/>
        <rdfs:comment>Represents a group of manufacturing processes used to produce composite materials through the bulk molding compound (BMC) method. BMC is a mixture of resin, reinforcement fibers, and additives that is heated and molded into the desired shape using compression molding or injection molding techniques.</rdfs:comment>
        <rdfs:label>Bulk Molding Compound Processes (BMC)</rdfs:label>
    </owl:Class>
    


    <!-- http://www.semanticweb.org/qihan/ontologies/2023/6/untitled-ontology-12#Cantilever_Beam_Specimen -->

    <owl:Class rdf:about="http://www.semanticweb.org/qihan/ontologies/2023/6/untitled-ontology-12#Cantilever_Beam_Specimen">
        <rdfs:subClassOf rdf:resource="http://www.semanticweb.org/qihan/ontologies/2023/6/untitled-ontology-12#Test_Specimen_Geometry"/>
        <rdfs:comment>Represents a type of test specimen with one fixed end and one free end, resembling a cantilever beam.</rdfs:comment>
        <rdfs:label>Cantilever Beam Specimen</rdfs:label>
    </owl:Class>
    


    <!-- http://www.semanticweb.org/qihan/ontologies/2023/6/untitled-ontology-12#Carbon_Fibre_Reinforced_Polymer -->

    <owl:Class rdf:about="http://www.semanticweb.org/qihan/ontologies/2023/6/untitled-ontology-12#Carbon_Fibre_Reinforced_Polymer">
        <rdfs:subClassOf rdf:resource="http://www.semanticweb.org/qihan/ontologies/2023/6/untitled-ontology-12#Polymer_Matrix_Composite"/>
    </owl:Class>
    


    <!-- http://www.semanticweb.org/qihan/ontologies/2023/6/untitled-ontology-12#Carbon_Matrix_Composite -->

    <owl:Class rdf:about="http://www.semanticweb.org/qihan/ontologies/2023/6/untitled-ontology-12#Carbon_Matrix_Composite">
        <rdfs:subClassOf rdf:resource="http://www.semanticweb.org/qihan/ontologies/2023/6/untitled-ontology-12#Ceramic_Matrix_Composite"/>
    </owl:Class>
    


    <!-- http://www.semanticweb.org/qihan/ontologies/2023/6/untitled-ontology-12#Carbon_Nanotube_Composite -->

    <owl:Class rdf:about="http://www.semanticweb.org/qihan/ontologies/2023/6/untitled-ontology-12#Carbon_Nanotube_Composite">
        <rdfs:subClassOf rdf:resource="http://www.semanticweb.org/qihan/ontologies/2023/6/untitled-ontology-12#Nanocomposite"/>
    </owl:Class>
    


    <!-- http://www.semanticweb.org/qihan/ontologies/2023/6/untitled-ontology-12#Casting_Machine -->

    <owl:Class rdf:about="http://www.semanticweb.org/qihan/ontologies/2023/6/untitled-ontology-12#Casting_Machine">
        <rdfs:subClassOf rdf:resource="http://www.semanticweb.org/qihan/ontologies/2023/6/untitled-ontology-12#Specimen_Preparation_Equipment"/>
        <rdfs:comment>Represents a general category of equipment used in the casting process to produce composite components.</rdfs:comment>
        <rdfs:label>Cast Machine</rdfs:label>
    </owl:Class>
    


    <!-- http://www.semanticweb.org/qihan/ontologies/2023/6/untitled-ontology-12#Cellulose-based_Composite -->

    <owl:Class rdf:about="http://www.semanticweb.org/qihan/ontologies/2023/6/untitled-ontology-12#Cellulose-based_Composite">
        <rdfs:subClassOf rdf:resource="http://www.semanticweb.org/qihan/ontologies/2023/6/untitled-ontology-12#Bio-based_Composite"/>
    </owl:Class>
    


    <!-- http://www.semanticweb.org/qihan/ontologies/2023/6/untitled-ontology-12#Centrifugal_casting_machine -->

    <owl:Class rdf:about="http://www.semanticweb.org/qihan/ontologies/2023/6/untitled-ontology-12#Centrifugal_casting_machine">
        <rdfs:subClassOf rdf:resource="http://www.semanticweb.org/qihan/ontologies/2023/6/untitled-ontology-12#Casting_Machine"/>
        <rdfs:comment>Represents a type of casting machine that utilizes centrifugal force to distribute molten material evenly in a mold.</rdfs:comment>
        <rdfs:label>Centrifugal Casting Machine</rdfs:label>
    </owl:Class>
    


    <!-- http://www.semanticweb.org/qihan/ontologies/2023/6/untitled-ontology-12#Ceramic-Metal_Functionally_Graded_Composite -->

    <owl:Class rdf:about="http://www.semanticweb.org/qihan/ontologies/2023/6/untitled-ontology-12#Ceramic-Metal_Functionally_Graded_Composite">
        <rdfs:subClassOf rdf:resource="http://www.semanticweb.org/qihan/ontologies/2023/6/untitled-ontology-12#Functionally_Graded_Composite"/>
    </owl:Class>
    


    <!-- http://www.semanticweb.org/qihan/ontologies/2023/6/untitled-ontology-12#Ceramic-Polymer_Functionally_Graded_Composite -->

    <owl:Class rdf:about="http://www.semanticweb.org/qihan/ontologies/2023/6/untitled-ontology-12#Ceramic-Polymer_Functionally_Graded_Composite">
        <rdfs:subClassOf rdf:resource="http://www.semanticweb.org/qihan/ontologies/2023/6/untitled-ontology-12#Functionally_Graded_Composite"/>
    </owl:Class>
    


    <!-- http://www.semanticweb.org/qihan/ontologies/2023/6/untitled-ontology-12#Ceramic_Matrix_Composite -->

    <owl:Class rdf:about="http://www.semanticweb.org/qihan/ontologies/2023/6/untitled-ontology-12#Ceramic_Matrix_Composite">
        <rdfs:subClassOf rdf:resource="http://www.semanticweb.org/qihan/ontologies/2023/6/untitled-ontology-12#Composite_Material"/>
    </owl:Class>
    


    <!-- http://www.semanticweb.org/qihan/ontologies/2023/6/untitled-ontology-12#Ceramic_Nanocomposite -->

    <owl:Class rdf:about="http://www.semanticweb.org/qihan/ontologies/2023/6/untitled-ontology-12#Ceramic_Nanocomposite">
        <rdfs:subClassOf rdf:resource="http://www.semanticweb.org/qihan/ontologies/2023/6/untitled-ontology-12#Nanocomposite"/>
    </owl:Class>
    


    <!-- http://www.semanticweb.org/qihan/ontologies/2023/6/untitled-ontology-12#Charpy_Impact_Tester -->

    <owl:Class rdf:about="http://www.semanticweb.org/qihan/ontologies/2023/6/untitled-ontology-12#Charpy_Impact_Tester">
        <rdfs:subClassOf rdf:resource="http://www.semanticweb.org/qihan/ontologies/2023/6/untitled-ontology-12#Impact_Tester"/>
        <rdfs:comment>Represents a specific type of impact tester used to measure the impact toughness of materials.</rdfs:comment>
        <rdfs:label>Charpy Impact Tester</rdfs:label>
    </owl:Class>
    


    <!-- http://www.semanticweb.org/qihan/ontologies/2023/6/untitled-ontology-12#Chemical_Resistance -->

    <owl:Class rdf:about="http://www.semanticweb.org/qihan/ontologies/2023/6/untitled-ontology-12#Chemical_Resistance">
        <rdfs:subClassOf rdf:resource="http://www.semanticweb.org/qihan/ontologies/2023/6/untitled-ontology-12#Result_Calculation"/>
    </owl:Class>
    


    <!-- http://www.semanticweb.org/qihan/ontologies/2023/6/untitled-ontology-12#Chemical_Stability -->

    <owl:Class rdf:about="http://www.semanticweb.org/qihan/ontologies/2023/6/untitled-ontology-12#Chemical_Stability">
        <rdfs:subClassOf rdf:resource="http://www.semanticweb.org/qihan/ontologies/2023/6/untitled-ontology-12#Chemical_Resistance"/>
    </owl:Class>
    


    <!-- http://www.semanticweb.org/qihan/ontologies/2023/6/untitled-ontology-12#Chopped_Fiber_Composite -->

    <owl:Class rdf:about="http://www.semanticweb.org/qihan/ontologies/2023/6/untitled-ontology-12#Chopped_Fiber_Composite">
        <rdfs:subClassOf rdf:resource="http://www.semanticweb.org/qihan/ontologies/2023/6/untitled-ontology-12#Discontinuous_Fiber_Composite"/>
    </owl:Class>
    


    <!-- http://www.semanticweb.org/qihan/ontologies/2023/6/untitled-ontology-12#Circular_Disk_Specimen -->

    <owl:Class rdf:about="http://www.semanticweb.org/qihan/ontologies/2023/6/untitled-ontology-12#Circular_Disk_Specimen">
        <rdfs:subClassOf rdf:resource="http://www.semanticweb.org/qihan/ontologies/2023/6/untitled-ontology-12#Test_Specimen_Geometry"/>
        <rdfs:comment>Represents a type of test specimen with a circular shape, often used for tests involving compression, tension, or shear loading.</rdfs:comment>
        <rdfs:label>Circular Disk Specimen</rdfs:label>
    </owl:Class>
    


    <!-- http://www.semanticweb.org/qihan/ontologies/2023/6/untitled-ontology-12#Climate_Chamber -->

    <owl:Class rdf:about="http://www.semanticweb.org/qihan/ontologies/2023/6/untitled-ontology-12#Climate_Chamber">
        <rdfs:subClassOf rdf:resource="http://www.semanticweb.org/qihan/ontologies/2023/6/untitled-ontology-12#Environmental_Chamber"/>
        <rdfs:comment>Represents a specialized chamber or enclosure used to control and maintain specific environmental conditions, such as temperature, humidity, and sometimes pressure, during testing of composite material specimens.</rdfs:comment>
        <rdfs:label>Climate Chamber</rdfs:label>
    </owl:Class>
    


    <!-- http://www.semanticweb.org/qihan/ontologies/2023/6/untitled-ontology-12#Clip-On_Extensometer -->

    <owl:Class rdf:about="http://www.semanticweb.org/qihan/ontologies/2023/6/untitled-ontology-12#Clip-On_Extensometer">
        <rdfs:subClassOf rdf:resource="http://www.semanticweb.org/qihan/ontologies/2023/6/untitled-ontology-12#Extensometer"/>
        <rdfs:comment>Represents a type of extensometer used for measuring the deformation or strain of composite material specimens during mechanical testing.</rdfs:comment>
        <rdfs:label>Clip-On Extensometer</rdfs:label>
    </owl:Class>
    


    <!-- http://www.semanticweb.org/qihan/ontologies/2023/6/untitled-ontology-12#Closed_Molding_Compression_Molding -->

    <owl:Class rdf:about="http://www.semanticweb.org/qihan/ontologies/2023/6/untitled-ontology-12#Closed_Molding_Compression_Molding">
        <rdfs:subClassOf rdf:resource="http://www.semanticweb.org/qihan/ontologies/2023/6/untitled-ontology-12#Compression_Molding_Processes"/>
        <rdfs:comment>Represents a specific type of compression molding process where the composite material is placed into a mold cavity that is fully enclosed.</rdfs:comment>
        <rdfs:label>Closed Molding Compression Molding</rdfs:label>
    </owl:Class>
    


    <!-- http://www.semanticweb.org/qihan/ontologies/2023/6/untitled-ontology-12#Coating_Thickness -->

    <owl:Class rdf:about="http://www.semanticweb.org/qihan/ontologies/2023/6/untitled-ontology-12#Coating_Thickness">
        <rdfs:subClassOf rdf:resource="http://www.semanticweb.org/qihan/ontologies/2023/6/untitled-ontology-12#Thickness"/>
        <rdfs:comment>Represents the measurement of the thickness of a coating or layer applied on the surface of a material.</rdfs:comment>
        <rdfs:label>Coating Thickness</rdfs:label>
    </owl:Class>
    


    <!-- http://www.semanticweb.org/qihan/ontologies/2023/6/untitled-ontology-12#Coefficient_of_Friction -->

    <owl:Class rdf:about="http://www.semanticweb.org/qihan/ontologies/2023/6/untitled-ontology-12#Coefficient_of_Friction">
        <rdfs:subClassOf rdf:resource="http://www.semanticweb.org/qihan/ontologies/2023/6/untitled-ontology-12#Wear_Resistance"/>
    </owl:Class>
    


    <!-- http://www.semanticweb.org/qihan/ontologies/2023/6/untitled-ontology-12#Coir_Fiber_Composite -->

    <owl:Class rdf:about="http://www.semanticweb.org/qihan/ontologies/2023/6/untitled-ontology-12#Coir_Fiber_Composite">
        <rdfs:subClassOf rdf:resource="http://www.semanticweb.org/qihan/ontologies/2023/6/untitled-ontology-12#Natural_Fiber_Composite"/>
    </owl:Class>
    


    <!-- http://www.semanticweb.org/qihan/ontologies/2023/6/untitled-ontology-12#Composite_Material -->

    <owl:Class rdf:about="http://www.semanticweb.org/qihan/ontologies/2023/6/untitled-ontology-12#Composite_Material">
        <rdfs:subClassOf rdf:resource="http://www.semanticweb.org/qihan/ontologies/2023/6/untitled-ontology-12#Material"/>
    </owl:Class>
    


    <!-- http://www.semanticweb.org/qihan/ontologies/2023/6/untitled-ontology-12#Compression_Instron_Machine -->

    <owl:Class rdf:about="http://www.semanticweb.org/qihan/ontologies/2023/6/untitled-ontology-12#Compression_Instron_Machine">
        <rdfs:subClassOf rdf:resource="http://www.semanticweb.org/qihan/ontologies/2023/6/untitled-ontology-12#Instron_Machine"/>
        <rdfs:comment>Represents a specific type of Instron machine used for conducting compression tests on materials.</rdfs:comment>
        <rdfs:label>Compression Imstron Machine</rdfs:label>
    </owl:Class>
    


    <!-- http://www.semanticweb.org/qihan/ontologies/2023/6/untitled-ontology-12#Compression_Molding -->

    <owl:Class rdf:about="http://www.semanticweb.org/qihan/ontologies/2023/6/untitled-ontology-12#Compression_Molding">
        <rdfs:subClassOf rdf:resource="http://www.semanticweb.org/qihan/ontologies/2023/6/untitled-ontology-12#Molding_Machine"/>
        <rdfs:comment>Represents a molding process where a material, often in a heated and plasticized state, is placed in a mold cavity and compressed to take the desired shape.</rdfs:comment>
        <rdfs:label>Compression Molding</rdfs:label>
    </owl:Class>
    


    <!-- http://www.semanticweb.org/qihan/ontologies/2023/6/untitled-ontology-12#Compression_Molding_Processes -->

    <owl:Class rdf:about="http://www.semanticweb.org/qihan/ontologies/2023/6/untitled-ontology-12#Compression_Molding_Processes">
        <rdfs:subClassOf rdf:resource="http://www.semanticweb.org/qihan/ontologies/2023/6/untitled-ontology-12#Material_Manufacturing"/>
        <rdfs:comment>Represents a group of manufacturing processes that utilize compression molding techniques to shape and cure composite materials.</rdfs:comment>
        <rdfs:label>Compression Molding Processes</rdfs:label>
    </owl:Class>
    


    <!-- http://www.semanticweb.org/qihan/ontologies/2023/6/untitled-ontology-12#Compression_Testing -->

    <owl:Class rdf:about="http://www.semanticweb.org/qihan/ontologies/2023/6/untitled-ontology-12#Compression_Testing">
        <rdfs:subClassOf rdf:resource="http://www.semanticweb.org/qihan/ontologies/2023/6/untitled-ontology-12#Testing_Method"/>
        <rdfs:comment>Represents a testing method used to evaluate the mechanical properties of materials under compressive loads.</rdfs:comment>
        <rdfs:label>Compression Testing</rdfs:label>
    </owl:Class>
    


    <!-- http://www.semanticweb.org/qihan/ontologies/2023/6/untitled-ontology-12#Compressive_Load -->

    <owl:Class rdf:about="http://www.semanticweb.org/qihan/ontologies/2023/6/untitled-ontology-12#Compressive_Load">
        <rdfs:subClassOf rdf:resource="http://www.semanticweb.org/qihan/ontologies/2023/6/untitled-ontology-12#Load"/>
        <rdfs:comment>Represents the external force or load applied to a material, in a direction that tends to compress or shorten the material along its axis.</rdfs:comment>
        <rdfs:label>Compressive Load</rdfs:label>
    </owl:Class>
    


    <!-- http://www.semanticweb.org/qihan/ontologies/2023/6/untitled-ontology-12#Compressive_Residual_Stress -->

    <owl:Class rdf:about="http://www.semanticweb.org/qihan/ontologies/2023/6/untitled-ontology-12#Compressive_Residual_Stress">
        <rdfs:subClassOf rdf:resource="http://www.semanticweb.org/qihan/ontologies/2023/6/untitled-ontology-12#Residual_Stress"/>
    </owl:Class>
    


    <!-- http://www.semanticweb.org/qihan/ontologies/2023/6/untitled-ontology-12#Compressive_Strain_Rate -->

    <owl:Class rdf:about="http://www.semanticweb.org/qihan/ontologies/2023/6/untitled-ontology-12#Compressive_Strain_Rate">
        <rdfs:subClassOf rdf:resource="http://www.semanticweb.org/qihan/ontologies/2023/6/untitled-ontology-12#Strain_Rate"/>
        <rdfs:comment>Represents the rate at which a material undergoes compressive strain or deformation over time.</rdfs:comment>
        <rdfs:label>Compressive Strain Rate</rdfs:label>
    </owl:Class>
    


    <!-- http://www.semanticweb.org/qihan/ontologies/2023/6/untitled-ontology-12#Compressive_Strength -->

    <owl:Class rdf:about="http://www.semanticweb.org/qihan/ontologies/2023/6/untitled-ontology-12#Compressive_Strength">
        <rdfs:subClassOf rdf:resource="http://www.semanticweb.org/qihan/ontologies/2023/6/untitled-ontology-12#Strength"/>
    </owl:Class>
    


    <!-- http://www.semanticweb.org/qihan/ontologies/2023/6/untitled-ontology-12#Compressive_Stress -->

    <owl:Class rdf:about="http://www.semanticweb.org/qihan/ontologies/2023/6/untitled-ontology-12#Compressive_Stress">
        <rdfs:subClassOf rdf:resource="http://www.semanticweb.org/qihan/ontologies/2023/6/untitled-ontology-12#Stress"/>
        <rdfs:comment>Represents the internal resistance or force per unit area that a material experiences when subjected to compressive forces.</rdfs:comment>
        <rdfs:label>Compressive Stress</rdfs:label>
    </owl:Class>
    


    <!-- http://www.semanticweb.org/qihan/ontologies/2023/6/untitled-ontology-12#Computer_Numerical_Control_Cutting_Machine -->

    <owl:Class rdf:about="http://www.semanticweb.org/qihan/ontologies/2023/6/untitled-ontology-12#Computer_Numerical_Control_Cutting_Machine">
        <rdfs:subClassOf rdf:resource="http://www.semanticweb.org/qihan/ontologies/2023/6/untitled-ontology-12#Cutting_Equipment"/>
        <rdfs:comment>Represents a type of cutting machine equipped with computer numerical control (CNC) technology.</rdfs:comment>
        <rdfs:label>Computer Numeriical Control (CNC) Cutting Machine</rdfs:label>
    </owl:Class>
    


    <!-- http://www.semanticweb.org/qihan/ontologies/2023/6/untitled-ontology-12#Computer_Numerical_Control_Milling_Machine -->

    <owl:Class rdf:about="http://www.semanticweb.org/qihan/ontologies/2023/6/untitled-ontology-12#Computer_Numerical_Control_Milling_Machine">
        <rdfs:subClassOf rdf:resource="http://www.semanticweb.org/qihan/ontologies/2023/6/untitled-ontology-12#Machining_Equipment"/>
        <rdfs:comment>Represents a type of milling machine equipped with computer numerical control (CNC) technology.</rdfs:comment>
        <rdfs:label>Computer Numerical Control (CNC) Milling Machine</rdfs:label>
    </owl:Class>
    


    <!-- http://www.semanticweb.org/qihan/ontologies/2023/6/untitled-ontology-12#Computer_Numerical_Control_Turning_Machine -->

    <owl:Class rdf:about="http://www.semanticweb.org/qihan/ontologies/2023/6/untitled-ontology-12#Computer_Numerical_Control_Turning_Machine">
        <rdfs:subClassOf rdf:resource="http://www.semanticweb.org/qihan/ontologies/2023/6/untitled-ontology-12#Machining_Equipment"/>
        <rdfs:comment>Represents a type of turning machine equipped with computer numerical control (CNC) technology.</rdfs:comment>
        <rdfs:label>Computer Numerical Control (CNC) Turning Machine</rdfs:label>
    </owl:Class>
    


    <!-- http://www.semanticweb.org/qihan/ontologies/2023/6/untitled-ontology-12#Constant_Load_Creep_Testing_Machine -->

    <owl:Class rdf:about="http://www.semanticweb.org/qihan/ontologies/2023/6/untitled-ontology-12#Constant_Load_Creep_Testing_Machine">
        <rdfs:subClassOf rdf:resource="http://www.semanticweb.org/qihan/ontologies/2023/6/untitled-ontology-12#Creep_Testing_Machine"/>
        <rdfs:comment>Represents a specific type of test equipment used for creep testing of composite material specimens under constant load conditions. It applies a constant load or force to the specimens over an extended period to evaluate their time-dependent deformation behaviour.</rdfs:comment>
        <rdfs:label>Constant Load Creep Testing Machine</rdfs:label>
    </owl:Class>
    


    <!-- http://www.semanticweb.org/qihan/ontologies/2023/6/untitled-ontology-12#Constant_Stress_Creep_Testing_Machine -->

    <owl:Class rdf:about="http://www.semanticweb.org/qihan/ontologies/2023/6/untitled-ontology-12#Constant_Stress_Creep_Testing_Machine">
        <rdfs:subClassOf rdf:resource="http://www.semanticweb.org/qihan/ontologies/2023/6/untitled-ontology-12#Creep_Testing_Machine"/>
        <rdfs:comment>Represents a specific type of test equipment used for creep testing of composite material specimens under constant stress conditions. It applies a constant stress or pressure to the specimens over an extended period to assess their time-dependent deformation behavior.</rdfs:comment>
        <rdfs:label>Constant Stress Creep Testing Machine</rdfs:label>
    </owl:Class>
    


    <!-- http://www.semanticweb.org/qihan/ontologies/2023/6/untitled-ontology-12#Contact_Extensometer -->

    <owl:Class rdf:about="http://www.semanticweb.org/qihan/ontologies/2023/6/untitled-ontology-12#Contact_Extensometer">
        <rdfs:subClassOf rdf:resource="http://www.semanticweb.org/qihan/ontologies/2023/6/untitled-ontology-12#Extensometer"/>
        <rdfs:comment>Represents a type of extensometer used to measure the deformation or strain of composite material specimens by making physical contact with the specimen surface.</rdfs:comment>
        <rdfs:label>Contact Extensometer</rdfs:label>
    </owl:Class>
    


    <!-- http://www.semanticweb.org/qihan/ontologies/2023/6/untitled-ontology-12#Continuous_Fiber_Composite -->

    <owl:Class rdf:about="http://www.semanticweb.org/qihan/ontologies/2023/6/untitled-ontology-12#Continuous_Fiber_Composite">
        <rdfs:subClassOf rdf:resource="http://www.semanticweb.org/qihan/ontologies/2023/6/untitled-ontology-12#Composite_Material"/>
    </owl:Class>
    


    <!-- http://www.semanticweb.org/qihan/ontologies/2023/6/untitled-ontology-12#Continuous_Fiber_Fabrication -->

    <owl:Class rdf:about="http://www.semanticweb.org/qihan/ontologies/2023/6/untitled-ontology-12#Continuous_Fiber_Fabrication">
        <rdfs:subClassOf rdf:resource="http://www.semanticweb.org/qihan/ontologies/2023/6/untitled-ontology-12#Additive_Manufacturing_Processes"/>
        <rdfs:comment>Represents a specific technique used in composite material manufacturing to integrate continuous fibers into a matrix material to enhance mechanical properties.</rdfs:comment>
        <rdfs:label>Continuous Fibre Fabrication (CFF)</rdfs:label>
    </owl:Class>
    


    <!-- http://www.semanticweb.org/qihan/ontologies/2023/6/untitled-ontology-12#Continuous_casting_machine -->

    <owl:Class rdf:about="http://www.semanticweb.org/qihan/ontologies/2023/6/untitled-ontology-12#Continuous_casting_machine">
        <rdfs:subClassOf rdf:resource="http://www.semanticweb.org/qihan/ontologies/2023/6/untitled-ontology-12#Casting_Machine"/>
        <rdfs:comment>Represents a type of casting machine used for continuously producing long and uniform metal or alloy products.</rdfs:comment>
        <rdfs:label>Continuous Casting Machine</rdfs:label>
    </owl:Class>
    


    <!-- http://www.semanticweb.org/qihan/ontologies/2023/6/untitled-ontology-12#Copper_Matrix_Composite -->

    <owl:Class rdf:about="http://www.semanticweb.org/qihan/ontologies/2023/6/untitled-ontology-12#Copper_Matrix_Composite">
        <rdfs:subClassOf rdf:resource="http://www.semanticweb.org/qihan/ontologies/2023/6/untitled-ontology-12#Metal_Matrix_Composite"/>
    </owl:Class>
    


    <!-- http://www.semanticweb.org/qihan/ontologies/2023/6/untitled-ontology-12#Corrosion_Resistance -->

    <owl:Class rdf:about="http://www.semanticweb.org/qihan/ontologies/2023/6/untitled-ontology-12#Corrosion_Resistance">
        <rdfs:subClassOf rdf:resource="http://www.semanticweb.org/qihan/ontologies/2023/6/untitled-ontology-12#Chemical_Resistance"/>
    </owl:Class>
    


    <!-- http://www.semanticweb.org/qihan/ontologies/2023/6/untitled-ontology-12#Creep_Behaviour -->

    <owl:Class rdf:about="http://www.semanticweb.org/qihan/ontologies/2023/6/untitled-ontology-12#Creep_Behaviour">
        <rdfs:subClassOf rdf:resource="http://www.semanticweb.org/qihan/ontologies/2023/6/untitled-ontology-12#Result_Calculation"/>
    </owl:Class>
    


    <!-- http://www.semanticweb.org/qihan/ontologies/2023/6/untitled-ontology-12#Creep_Rate -->

    <owl:Class rdf:about="http://www.semanticweb.org/qihan/ontologies/2023/6/untitled-ontology-12#Creep_Rate">
        <rdfs:subClassOf rdf:resource="http://www.semanticweb.org/qihan/ontologies/2023/6/untitled-ontology-12#Creep_Behaviour"/>
    </owl:Class>
    


    <!-- http://www.semanticweb.org/qihan/ontologies/2023/6/untitled-ontology-12#Creep_Strain -->

    <owl:Class rdf:about="http://www.semanticweb.org/qihan/ontologies/2023/6/untitled-ontology-12#Creep_Strain">
        <rdfs:subClassOf rdf:resource="http://www.semanticweb.org/qihan/ontologies/2023/6/untitled-ontology-12#Creep_Behaviour"/>
    </owl:Class>
    


    <!-- http://www.semanticweb.org/qihan/ontologies/2023/6/untitled-ontology-12#Creep_Testing -->

    <owl:Class rdf:about="http://www.semanticweb.org/qihan/ontologies/2023/6/untitled-ontology-12#Creep_Testing">
        <rdfs:subClassOf rdf:resource="http://www.semanticweb.org/qihan/ontologies/2023/6/untitled-ontology-12#Testing_Method"/>
        <rdfs:comment>Represents a type of mechanical testing used to study the time-dependent deformation behavior of materials, when subjected to a constant load or stress over an extended period.</rdfs:comment>
        <rdfs:label>Creep Testing</rdfs:label>
    </owl:Class>
    


    <!-- http://www.semanticweb.org/qihan/ontologies/2023/6/untitled-ontology-12#Creep_Testing_Machine -->

    <owl:Class rdf:about="http://www.semanticweb.org/qihan/ontologies/2023/6/untitled-ontology-12#Creep_Testing_Machine">
        <rdfs:subClassOf rdf:resource="http://www.semanticweb.org/qihan/ontologies/2023/6/untitled-ontology-12#Test_Equipment"/>
        <rdfs:comment>Represents a specific type of test equipment used to create a creep curve on how much pressure and stress a material can handle. The machine is able to calculate the stress rate, time and pressure.</rdfs:comment>
        <rdfs:label>Creep Testing Machine</rdfs:label>
    </owl:Class>
    


    <!-- http://www.semanticweb.org/qihan/ontologies/2023/6/untitled-ontology-12#Creep_Time -->

    <owl:Class rdf:about="http://www.semanticweb.org/qihan/ontologies/2023/6/untitled-ontology-12#Creep_Time">
        <rdfs:subClassOf rdf:resource="http://www.semanticweb.org/qihan/ontologies/2023/6/untitled-ontology-12#Time"/>
        <rdfs:comment>Represents the time duration during which a material is subjected to a constant load or stress.</rdfs:comment>
        <rdfs:label>Creep Time</rdfs:label>
    </owl:Class>
    


    <!-- http://www.semanticweb.org/qihan/ontologies/2023/6/untitled-ontology-12#Crockmeter_Abrasion_Tester -->

    <owl:Class rdf:about="http://www.semanticweb.org/qihan/ontologies/2023/6/untitled-ontology-12#Crockmeter_Abrasion_Tester">
        <rdfs:subClassOf rdf:resource="http://www.semanticweb.org/qihan/ontologies/2023/6/untitled-ontology-12#Abrasion_Testing_Machine"/>
        <rdfs:comment>Represents a specific type of test equipment used to assess the abrasion resistance of composite material specimens by rubbing against a standard fabric or material.</rdfs:comment>
        <rdfs:label>Crockmeter Abrasion Tester</rdfs:label>
    </owl:Class>
    


    <!-- http://www.semanticweb.org/qihan/ontologies/2023/6/untitled-ontology-12#Cutting_Equipment -->

    <owl:Class rdf:about="http://www.semanticweb.org/qihan/ontologies/2023/6/untitled-ontology-12#Cutting_Equipment">
        <rdfs:subClassOf rdf:resource="http://www.semanticweb.org/qihan/ontologies/2023/6/untitled-ontology-12#Specimen_Preparation_Equipment"/>
        <rdfs:comment>Represents equipment specifically designed for cutting composite materials into the desired shapes and sizes for test specimens.</rdfs:comment>
        <rdfs:label>Cutting Equipment</rdfs:label>
    </owl:Class>
    


    <!-- http://www.semanticweb.org/qihan/ontologies/2023/6/untitled-ontology-12#Cyclic_Loading_Frequency -->

    <owl:Class rdf:about="http://www.semanticweb.org/qihan/ontologies/2023/6/untitled-ontology-12#Cyclic_Loading_Frequency">
        <rdfs:subClassOf rdf:resource="http://www.semanticweb.org/qihan/ontologies/2023/6/untitled-ontology-12#Frequency"/>
        <rdfs:comment>Represents the rate or frequency at which cyclic loading or repeated stress is applied to a material.</rdfs:comment>
        <rdfs:label>Cyclic Loading Frequency</rdfs:label>
    </owl:Class>
    


    <!-- http://www.semanticweb.org/qihan/ontologies/2023/6/untitled-ontology-12#Cycling_Temperature -->

    <owl:Class rdf:about="http://www.semanticweb.org/qihan/ontologies/2023/6/untitled-ontology-12#Cycling_Temperature">
        <rdfs:subClassOf rdf:resource="http://www.semanticweb.org/qihan/ontologies/2023/6/untitled-ontology-12#Temperature"/>
        <rdfs:comment>Represents the variation or cycling of temperature during mechanical testing of composite material specimens. It refers to the controlled fluctuation of temperature within specific ranges over time.</rdfs:comment>
        <rdfs:label>Cycling Temperature</rdfs:label>
    </owl:Class>
    


    <!-- http://www.semanticweb.org/qihan/ontologies/2023/6/untitled-ontology-12#DIN_EN_ISO_14125 -->

    <owl:Class rdf:about="http://www.semanticweb.org/qihan/ontologies/2023/6/untitled-ontology-12#DIN_EN_ISO_14125">
        <rdfs:subClassOf rdf:resource="http://www.semanticweb.org/qihan/ontologies/2023/6/untitled-ontology-12#DIN_Standards"/>
        <rdfs:comment>Fibre-reinforced plastic composites - Determination of flexural properties</rdfs:comment>
        <rdfs:label>DIN EN ISO 14125</rdfs:label>
    </owl:Class>
    


    <!-- http://www.semanticweb.org/qihan/ontologies/2023/6/untitled-ontology-12#DIN_EN_ISO_178 -->

    <owl:Class rdf:about="http://www.semanticweb.org/qihan/ontologies/2023/6/untitled-ontology-12#DIN_EN_ISO_178">
        <rdfs:subClassOf rdf:resource="http://www.semanticweb.org/qihan/ontologies/2023/6/untitled-ontology-12#DIN_Standards"/>
        <rdfs:comment>Plastics - Determination of Flexural Properties</rdfs:comment>
        <rdfs:label>DIN EN ISO 178</rdfs:label>
    </owl:Class>
    


    <!-- http://www.semanticweb.org/qihan/ontologies/2023/6/untitled-ontology-12#DIN_EN_ISO_527 -->

    <owl:Class rdf:about="http://www.semanticweb.org/qihan/ontologies/2023/6/untitled-ontology-12#DIN_EN_ISO_527">
        <rdfs:subClassOf rdf:resource="http://www.semanticweb.org/qihan/ontologies/2023/6/untitled-ontology-12#DIN_Standards"/>
        <rdfs:comment>Plastics - Determination of Tensile Properties</rdfs:comment>
        <rdfs:label>DIN EN ISO 527</rdfs:label>
    </owl:Class>
    


    <!-- http://www.semanticweb.org/qihan/ontologies/2023/6/untitled-ontology-12#DIN_Standards -->

    <owl:Class rdf:about="http://www.semanticweb.org/qihan/ontologies/2023/6/untitled-ontology-12#DIN_Standards">
        <rdfs:subClassOf rdf:resource="http://www.semanticweb.org/qihan/ontologies/2023/6/untitled-ontology-12#Test_Standards"/>
        <rdfs:label>Deutsches Institut für Normung (DIN)</rdfs:label>
    </owl:Class>
    


    <!-- http://www.semanticweb.org/qihan/ontologies/2023/6/untitled-ontology-12#Damping_Capacity -->

    <owl:Class rdf:about="http://www.semanticweb.org/qihan/ontologies/2023/6/untitled-ontology-12#Damping_Capacity">
        <rdfs:subClassOf rdf:resource="http://www.semanticweb.org/qihan/ontologies/2023/6/untitled-ontology-12#Result_Calculation"/>
    </owl:Class>
    


    <!-- http://www.semanticweb.org/qihan/ontologies/2023/6/untitled-ontology-12#Data_Visualization -->

    <owl:Class rdf:about="http://www.semanticweb.org/qihan/ontologies/2023/6/untitled-ontology-12#Data_Visualization">
        <rdfs:subClassOf rdf:resource="http://www.semanticweb.org/qihan/ontologies/2023/6/untitled-ontology-12#Result_Analysis"/>
    </owl:Class>
    


    <!-- http://www.semanticweb.org/qihan/ontologies/2023/6/untitled-ontology-12#Delamination -->

    <owl:Class rdf:about="http://www.semanticweb.org/qihan/ontologies/2023/6/untitled-ontology-12#Delamination">
        <rdfs:subClassOf rdf:resource="http://www.semanticweb.org/qihan/ontologies/2023/6/untitled-ontology-12#Failure_Mode"/>
    </owl:Class>
    


    <!-- http://www.semanticweb.org/qihan/ontologies/2023/6/untitled-ontology-12#Die_casting_machine -->

    <owl:Class rdf:about="http://www.semanticweb.org/qihan/ontologies/2023/6/untitled-ontology-12#Die_casting_machine">
        <rdfs:subClassOf rdf:resource="http://www.semanticweb.org/qihan/ontologies/2023/6/untitled-ontology-12#Casting_Machine"/>
        <rdfs:comment>Represents a type of casting machine used in the die casting process to produce metal components with complex shapes and high precision.</rdfs:comment>
        <rdfs:label>Die Casting Machine</rdfs:label>
    </owl:Class>
    


    <!-- http://www.semanticweb.org/qihan/ontologies/2023/6/untitled-ontology-12#Differential_Scanning_Calorimeter -->

    <owl:Class rdf:about="http://www.semanticweb.org/qihan/ontologies/2023/6/untitled-ontology-12#Differential_Scanning_Calorimeter">
        <rdfs:subClassOf rdf:resource="http://www.semanticweb.org/qihan/ontologies/2023/6/untitled-ontology-12#Thermal_Analysis_Equipment"/>
        <rdfs:comment>Represents a specific type of thermal analysis equipment used to measure the heat flow and heat capacity of materials.</rdfs:comment>
        <rdfs:label>Differential Scanning Calorimeter (DSC)</rdfs:label>
    </owl:Class>
    


    <!-- http://www.semanticweb.org/qihan/ontologies/2023/6/untitled-ontology-12#Digital_Image_Correlation_Camera -->

    <owl:Class rdf:about="http://www.semanticweb.org/qihan/ontologies/2023/6/untitled-ontology-12#Digital_Image_Correlation_Camera">
        <rdfs:subClassOf rdf:resource="http://www.semanticweb.org/qihan/ontologies/2023/6/untitled-ontology-12#High-Speed_Camera"/>
        <rdfs:comment>Represents a type of camera used in Digital Image Correlation systems for measuring deformation and strain in composite material specimens.</rdfs:comment>
        <rdfs:label>Digital Image Correlation Camera</rdfs:label>
    </owl:Class>
    


    <!-- http://www.semanticweb.org/qihan/ontologies/2023/6/untitled-ontology-12#Dimensional_Changes -->

    <owl:Class rdf:about="http://www.semanticweb.org/qihan/ontologies/2023/6/untitled-ontology-12#Dimensional_Changes">
        <rdfs:subClassOf rdf:resource="http://www.semanticweb.org/qihan/ontologies/2023/6/untitled-ontology-12#Result_Calculation"/>
    </owl:Class>
    


    <!-- http://www.semanticweb.org/qihan/ontologies/2023/6/untitled-ontology-12#Disc_Sander -->

    <owl:Class rdf:about="http://www.semanticweb.org/qihan/ontologies/2023/6/untitled-ontology-12#Disc_Sander">
        <rdfs:subClassOf rdf:resource="http://www.semanticweb.org/qihan/ontologies/2023/6/untitled-ontology-12#Grinding_and_Sanding_Equipment"/>
        <rdfs:comment>Represents a type of sanding machine with a circular sanding disc mounted on a rotating spindle.</rdfs:comment>
        <rdfs:label>Disc Sander</rdfs:label>
    </owl:Class>
    


    <!-- http://www.semanticweb.org/qihan/ontologies/2023/6/untitled-ontology-12#Discontinuous_Fiber_Composite -->

    <owl:Class rdf:about="http://www.semanticweb.org/qihan/ontologies/2023/6/untitled-ontology-12#Discontinuous_Fiber_Composite">
        <rdfs:subClassOf rdf:resource="http://www.semanticweb.org/qihan/ontologies/2023/6/untitled-ontology-12#Composite_Material"/>
    </owl:Class>
    


    <!-- http://www.semanticweb.org/qihan/ontologies/2023/6/untitled-ontology-12#Displacement -->

    <owl:Class rdf:about="http://www.semanticweb.org/qihan/ontologies/2023/6/untitled-ontology-12#Displacement">
        <rdfs:subClassOf rdf:resource="http://www.semanticweb.org/qihan/ontologies/2023/6/untitled-ontology-12#Test_Parameter"/>
        <rdfs:comment>Represents a physical quantity that measures the change in position of a material or object. It is a key parameter in mechanical testing to determine material deformation and behavior under applied loads.</rdfs:comment>
        <rdfs:label>Displacement</rdfs:label>
    </owl:Class>
    


    <!-- http://www.semanticweb.org/qihan/ontologies/2023/6/untitled-ontology-12#Dogbone_Specimen -->

    <owl:Class rdf:about="http://www.semanticweb.org/qihan/ontologies/2023/6/untitled-ontology-12#Dogbone_Specimen">
        <rdfs:subClassOf rdf:resource="http://www.semanticweb.org/qihan/ontologies/2023/6/untitled-ontology-12#Test_Specimen_Geometry"/>
        <rdfs:comment>Represents a type of test specimen with a distinctive shape resembling a dogbone, with a reduced cross-sectional area at the center and broader ends.</rdfs:comment>
        <rdfs:label>Dogbone Specimen</rdfs:label>
    </owl:Class>
    


    <!-- http://www.semanticweb.org/qihan/ontologies/2023/6/untitled-ontology-12#Double_Cantilever_Beam_Specimen -->

    <owl:Class rdf:about="http://www.semanticweb.org/qihan/ontologies/2023/6/untitled-ontology-12#Double_Cantilever_Beam_Specimen">
        <rdfs:subClassOf rdf:resource="http://www.semanticweb.org/qihan/ontologies/2023/6/untitled-ontology-12#Test_Specimen_Geometry"/>
        <rdfs:comment>Represents a type of test specimen with two cantilever beams placed back to back, creating a crack or defect between the beams.</rdfs:comment>
        <rdfs:label>Double Cantilever Beam Specimen</rdfs:label>
    </owl:Class>
    


    <!-- http://www.semanticweb.org/qihan/ontologies/2023/6/untitled-ontology-12#Drape_Forming -->

    <owl:Class rdf:about="http://www.semanticweb.org/qihan/ontologies/2023/6/untitled-ontology-12#Drape_Forming">
        <rdfs:subClassOf rdf:resource="http://www.semanticweb.org/qihan/ontologies/2023/6/untitled-ontology-12#Sheet_Forming_Processes"/>
        <rdfs:comment>Represents a specific sheet forming process where a pre-cut composite sheet is draped or placed over a mold or tool with the desired shape.</rdfs:comment>
        <rdfs:label>Drape Forming</rdfs:label>
    </owl:Class>
    


    <!-- http://www.semanticweb.org/qihan/ontologies/2023/6/untitled-ontology-12#Drilling_Machine -->

    <owl:Class rdf:about="http://www.semanticweb.org/qihan/ontologies/2023/6/untitled-ontology-12#Drilling_Machine">
        <rdfs:subClassOf rdf:resource="http://www.semanticweb.org/qihan/ontologies/2023/6/untitled-ontology-12#Machining_Equipment"/>
        <rdfs:comment>Represents a type of machining equipment used for drilling holes in workpieces.</rdfs:comment>
        <rdfs:label>Drilling Machine</rdfs:label>
    </owl:Class>
    


    <!-- http://www.semanticweb.org/qihan/ontologies/2023/6/untitled-ontology-12#Drop_Weight_Impact_Tester -->

    <owl:Class rdf:about="http://www.semanticweb.org/qihan/ontologies/2023/6/untitled-ontology-12#Drop_Weight_Impact_Tester">
        <rdfs:subClassOf rdf:resource="http://www.semanticweb.org/qihan/ontologies/2023/6/untitled-ontology-12#Impact_Tester"/>
        <rdfs:comment>Represents a specific type of impact tester used to evaluate the impact resistance and fracture behavior of materials, including composite material specimens.</rdfs:comment>
        <rdfs:label>Drop Weight Impact Tester</rdfs:label>
    </owl:Class>
    


    <!-- http://www.semanticweb.org/qihan/ontologies/2023/6/untitled-ontology-12#Dry_Condition -->

    <owl:Class rdf:about="http://www.semanticweb.org/qihan/ontologies/2023/6/untitled-ontology-12#Dry_Condition">
        <rdfs:subClassOf rdf:resource="http://www.semanticweb.org/qihan/ontologies/2023/6/untitled-ontology-12#Moisture_Content"/>
        <rdfs:comment>Represents the state or condition of a material, when it is free from moisture or water content.</rdfs:comment>
        <rdfs:label>Dry Condition</rdfs:label>
    </owl:Class>
    


    <!-- http://www.semanticweb.org/qihan/ontologies/2023/6/untitled-ontology-12#Ductile_Failure -->

    <owl:Class rdf:about="http://www.semanticweb.org/qihan/ontologies/2023/6/untitled-ontology-12#Ductile_Failure">
        <rdfs:subClassOf rdf:resource="http://www.semanticweb.org/qihan/ontologies/2023/6/untitled-ontology-12#Failure_Mode"/>
    </owl:Class>
    


    <!-- http://www.semanticweb.org/qihan/ontologies/2023/6/untitled-ontology-12#Dynamic_Mechanical_Analyzer -->

    <owl:Class rdf:about="http://www.semanticweb.org/qihan/ontologies/2023/6/untitled-ontology-12#Dynamic_Mechanical_Analyzer">
        <rdfs:subClassOf rdf:resource="http://www.semanticweb.org/qihan/ontologies/2023/6/untitled-ontology-12#Test_Equipment"/>
        <rdfs:comment>Represents a specific type of test equipment used to measure the viscoelastic properties of composite material specimens. It applies varying loads and frequencies to analyze the mechanical behavior of materials as a function of time and temperature.</rdfs:comment>
        <rdfs:label>Dynamic Mechanical Analyzer (DMA)</rdfs:label>
    </owl:Class>
    


    <!-- http://www.semanticweb.org/qihan/ontologies/2023/6/untitled-ontology-12#EN_2561 -->

    <owl:Class rdf:about="http://www.semanticweb.org/qihan/ontologies/2023/6/untitled-ontology-12#EN_2561">
        <rdfs:subClassOf rdf:resource="http://www.semanticweb.org/qihan/ontologies/2023/6/untitled-ontology-12#EN_Standards"/>
        <rdfs:comment>Aerospace series - Fibre reinforced plastics - Determination of compressive strength after impact</rdfs:comment>
        <rdfs:label>EN 2561</rdfs:label>
    </owl:Class>
    


    <!-- http://www.semanticweb.org/qihan/ontologies/2023/6/untitled-ontology-12#EN_ISO_13003 -->

    <owl:Class rdf:about="http://www.semanticweb.org/qihan/ontologies/2023/6/untitled-ontology-12#EN_ISO_13003">
        <rdfs:subClassOf rdf:resource="http://www.semanticweb.org/qihan/ontologies/2023/6/untitled-ontology-12#EN_Standards"/>
        <rdfs:comment>Fibre-reinforced plastic composites - Determination of fatigue properties</rdfs:comment>
        <rdfs:label>EN ISO 13003</rdfs:label>
    </owl:Class>
    


    <!-- http://www.semanticweb.org/qihan/ontologies/2023/6/untitled-ontology-12#EN_ISO_14125 -->

    <owl:Class rdf:about="http://www.semanticweb.org/qihan/ontologies/2023/6/untitled-ontology-12#EN_ISO_14125">
        <rdfs:subClassOf rdf:resource="http://www.semanticweb.org/qihan/ontologies/2023/6/untitled-ontology-12#EN_Standards"/>
        <rdfs:comment>Fibre-reinforced plastic composites - Determination of flexural properties</rdfs:comment>
        <rdfs:label>EN ISO 14125</rdfs:label>
    </owl:Class>
    


    <!-- http://www.semanticweb.org/qihan/ontologies/2023/6/untitled-ontology-12#EN_Standards -->

    <owl:Class rdf:about="http://www.semanticweb.org/qihan/ontologies/2023/6/untitled-ontology-12#EN_Standards">
        <rdfs:subClassOf rdf:resource="http://www.semanticweb.org/qihan/ontologies/2023/6/untitled-ontology-12#Test_Standards"/>
        <rdfs:label>European Norms (EN)</rdfs:label>
    </owl:Class>
    


    <!-- http://www.semanticweb.org/qihan/ontologies/2023/6/untitled-ontology-12#Electric_Field -->

    <owl:Class rdf:about="http://www.semanticweb.org/qihan/ontologies/2023/6/untitled-ontology-12#Electric_Field">
        <rdfs:subClassOf rdf:resource="http://www.semanticweb.org/qihan/ontologies/2023/6/untitled-ontology-12#Test_Parameter"/>
        <rdfs:comment>Represents a physical quantity that describes the intensity of an electric force experienced by charged particles in a material.</rdfs:comment>
        <rdfs:label>Electric Field</rdfs:label>
    </owl:Class>
    


    <!-- http://www.semanticweb.org/qihan/ontologies/2023/6/untitled-ontology-12#Electric_Potential -->

    <owl:Class rdf:about="http://www.semanticweb.org/qihan/ontologies/2023/6/untitled-ontology-12#Electric_Potential">
        <rdfs:subClassOf rdf:resource="http://www.semanticweb.org/qihan/ontologies/2023/6/untitled-ontology-12#Electric_Field"/>
        <rdfs:comment>Represents the electrical potential or voltage difference between two points in a material.</rdfs:comment>
        <rdfs:label>Electric Potential</rdfs:label>
    </owl:Class>
    


    <!-- http://www.semanticweb.org/qihan/ontologies/2023/6/untitled-ontology-12#Electrical_Power -->

    <owl:Class rdf:about="http://www.semanticweb.org/qihan/ontologies/2023/6/untitled-ontology-12#Electrical_Power">
        <rdfs:subClassOf rdf:resource="http://www.semanticweb.org/qihan/ontologies/2023/6/untitled-ontology-12#Power"/>
        <rdfs:comment>Represents the amount of electrical energy consumed, generated, or transferred by a system.</rdfs:comment>
        <rdfs:label>Electrical Power</rdfs:label>
    </owl:Class>
    


    <!-- http://www.semanticweb.org/qihan/ontologies/2023/6/untitled-ontology-12#Electriical_Conductivity -->

    <owl:Class rdf:about="http://www.semanticweb.org/qihan/ontologies/2023/6/untitled-ontology-12#Electriical_Conductivity">
        <rdfs:subClassOf rdf:resource="http://www.semanticweb.org/qihan/ontologies/2023/6/untitled-ontology-12#Result_Calculation"/>
    </owl:Class>
    


    <!-- http://www.semanticweb.org/qihan/ontologies/2023/6/untitled-ontology-12#Electro-Mechnical_Testing_Machine -->

    <owl:Class rdf:about="http://www.semanticweb.org/qihan/ontologies/2023/6/untitled-ontology-12#Electro-Mechnical_Testing_Machine">
        <rdfs:subClassOf rdf:resource="http://www.semanticweb.org/qihan/ontologies/2023/6/untitled-ontology-12#Universal_Testing_Machine"/>
        <rdfs:comment>Represents a type of testing machine that uses electric motors to apply forces and deformations to materials.</rdfs:comment>
        <rdfs:label>Electro-Mechanical Testing Machine</rdfs:label>
    </owl:Class>
    


    <!-- http://www.semanticweb.org/qihan/ontologies/2023/6/untitled-ontology-12#Elevated_Temperature -->

    <owl:Class rdf:about="http://www.semanticweb.org/qihan/ontologies/2023/6/untitled-ontology-12#Elevated_Temperature">
        <rdfs:subClassOf rdf:resource="http://www.semanticweb.org/qihan/ontologies/2023/6/untitled-ontology-12#Temperature"/>
        <rdfs:comment>Represents higher-than-ambient temperatures applied to composite material specimens during mechanical testing. It involves subjecting the specimens to elevated thermal conditions for specific testing purposes.</rdfs:comment>
        <rdfs:label>Elevated Temperature</rdfs:label>
    </owl:Class>
    


    <!-- http://www.semanticweb.org/qihan/ontologies/2023/6/untitled-ontology-12#End-Notched_Flexure_Specimen -->

    <owl:Class rdf:about="http://www.semanticweb.org/qihan/ontologies/2023/6/untitled-ontology-12#End-Notched_Flexure_Specimen">
        <rdfs:subClassOf rdf:resource="http://www.semanticweb.org/qihan/ontologies/2023/6/untitled-ontology-12#Test_Specimen_Geometry"/>
        <rdfs:comment>Represents a type of test specimen with a notch or groove at one end, designed to induce controlled crack propagation during a flexural test.</rdfs:comment>
        <rdfs:label>End-Notched Flexure Specimen</rdfs:label>
    </owl:Class>
    


    <!-- http://www.semanticweb.org/qihan/ontologies/2023/6/untitled-ontology-12#Energy_Absorption -->

    <owl:Class rdf:about="http://www.semanticweb.org/qihan/ontologies/2023/6/untitled-ontology-12#Energy_Absorption">
        <rdfs:subClassOf rdf:resource="http://www.semanticweb.org/qihan/ontologies/2023/6/untitled-ontology-12#Toughness"/>
    </owl:Class>
    


    <!-- http://www.semanticweb.org/qihan/ontologies/2023/6/untitled-ontology-12#Environmental_Aging_Resistance -->

    <owl:Class rdf:about="http://www.semanticweb.org/qihan/ontologies/2023/6/untitled-ontology-12#Environmental_Aging_Resistance">
        <rdfs:subClassOf rdf:resource="http://www.semanticweb.org/qihan/ontologies/2023/6/untitled-ontology-12#Aging_Properties"/>
    </owl:Class>
    


    <!-- http://www.semanticweb.org/qihan/ontologies/2023/6/untitled-ontology-12#Environmental_Chamber -->

    <owl:Class rdf:about="http://www.semanticweb.org/qihan/ontologies/2023/6/untitled-ontology-12#Environmental_Chamber">
        <rdfs:subClassOf rdf:resource="http://www.semanticweb.org/qihan/ontologies/2023/6/untitled-ontology-12#Test_Equipment"/>
        <rdfs:comment>Represents a specialized enclosure or chamber used during mechanical testing of composite material specimens to control and maintain specific environmental conditions, such as temperature, humidity, and gas atmosphere.</rdfs:comment>
        <rdfs:label>Environmental Chamber</rdfs:label>
    </owl:Class>
    


    <!-- http://www.semanticweb.org/qihan/ontologies/2023/6/untitled-ontology-12#Erosion -->

    <owl:Class rdf:about="http://www.semanticweb.org/qihan/ontologies/2023/6/untitled-ontology-12#Erosion">
        <rdfs:subClassOf rdf:resource="http://www.semanticweb.org/qihan/ontologies/2023/6/untitled-ontology-12#Failure_Mode"/>
    </owl:Class>
    


    <!-- http://www.semanticweb.org/qihan/ontologies/2023/6/untitled-ontology-12#Extensometer -->

    <owl:Class rdf:about="http://www.semanticweb.org/qihan/ontologies/2023/6/untitled-ontology-12#Extensometer">
        <rdfs:subClassOf rdf:resource="http://www.semanticweb.org/qihan/ontologies/2023/6/untitled-ontology-12#Test_Equipment"/>
        <rdfs:comment>Represents a measuring device or sensor used to measure the changes in length or deformation of composite material specimens during mechanical testing. It provides accurate strain measurements.</rdfs:comment>
        <rdfs:label>Extensometer</rdfs:label>
    </owl:Class>
    


    <!-- http://www.semanticweb.org/qihan/ontologies/2023/6/untitled-ontology-12#Failure_Mode -->

    <owl:Class rdf:about="http://www.semanticweb.org/qihan/ontologies/2023/6/untitled-ontology-12#Failure_Mode">
        <rdfs:subClassOf rdf:resource="http://www.semanticweb.org/qihan/ontologies/2023/6/untitled-ontology-12#Result_Analysis"/>
    </owl:Class>
    


    <!-- http://www.semanticweb.org/qihan/ontologies/2023/6/untitled-ontology-12#Fatigue_Crack_Growth_Rate -->

    <owl:Class rdf:about="http://www.semanticweb.org/qihan/ontologies/2023/6/untitled-ontology-12#Fatigue_Crack_Growth_Rate">
        <rdfs:subClassOf rdf:resource="http://www.semanticweb.org/qihan/ontologies/2023/6/untitled-ontology-12#Fatigue_Life"/>
    </owl:Class>
    


    <!-- http://www.semanticweb.org/qihan/ontologies/2023/6/untitled-ontology-12#Fatigue_Endurance_Limit -->

    <owl:Class rdf:about="http://www.semanticweb.org/qihan/ontologies/2023/6/untitled-ontology-12#Fatigue_Endurance_Limit">
        <rdfs:subClassOf rdf:resource="http://www.semanticweb.org/qihan/ontologies/2023/6/untitled-ontology-12#Fatigue_Life"/>
    </owl:Class>
    


    <!-- http://www.semanticweb.org/qihan/ontologies/2023/6/untitled-ontology-12#Fatigue_Life -->

    <owl:Class rdf:about="http://www.semanticweb.org/qihan/ontologies/2023/6/untitled-ontology-12#Fatigue_Life">
        <rdfs:subClassOf rdf:resource="http://www.semanticweb.org/qihan/ontologies/2023/6/untitled-ontology-12#Result_Calculation"/>
    </owl:Class>
    


    <!-- http://www.semanticweb.org/qihan/ontologies/2023/6/untitled-ontology-12#Fatigue_Strength -->

    <owl:Class rdf:about="http://www.semanticweb.org/qihan/ontologies/2023/6/untitled-ontology-12#Fatigue_Strength">
        <rdfs:subClassOf rdf:resource="http://www.semanticweb.org/qihan/ontologies/2023/6/untitled-ontology-12#Fatigue_Life"/>
    </owl:Class>
    


    <!-- http://www.semanticweb.org/qihan/ontologies/2023/6/untitled-ontology-12#Fatigue_Testing -->

    <owl:Class rdf:about="http://www.semanticweb.org/qihan/ontologies/2023/6/untitled-ontology-12#Fatigue_Testing">
        <rdfs:subClassOf rdf:resource="http://www.semanticweb.org/qihan/ontologies/2023/6/untitled-ontology-12#Testing_Method"/>
        <rdfs:comment>Represents a type of mechanical testing used to evaluate the fatigue behavior and durability of materials under cyclic loading conditions.</rdfs:comment>
        <rdfs:label>Fatigue Testing</rdfs:label>
    </owl:Class>
    


    <!-- http://www.semanticweb.org/qihan/ontologies/2023/6/untitled-ontology-12#Fatigue_Testing_Machine -->

    <owl:Class rdf:about="http://www.semanticweb.org/qihan/ontologies/2023/6/untitled-ontology-12#Fatigue_Testing_Machine">
        <rdfs:subClassOf rdf:resource="http://www.semanticweb.org/qihan/ontologies/2023/6/untitled-ontology-12#Test_Equipment"/>
        <rdfs:comment>Represents a specific type of test equipment used to subject composite material specimens to cyclic loading and evaluate their fatigue behavior and durability under repetitive stress.</rdfs:comment>
        <rdfs:label>Fatigue Testing Machine</rdfs:label>
    </owl:Class>
    


    <!-- http://www.semanticweb.org/qihan/ontologies/2023/6/untitled-ontology-12#Fiber_Placement -->

    <owl:Class rdf:about="http://www.semanticweb.org/qihan/ontologies/2023/6/untitled-ontology-12#Fiber_Placement">
        <rdfs:subClassOf rdf:resource="http://www.semanticweb.org/qihan/ontologies/2023/6/untitled-ontology-12#Layup_Processes"/>
        <rdfs:comment>Represents a layup process in which continuous fibers are manually placed onto a mold or tool to create a composite structure.</rdfs:comment>
        <rdfs:label>Fiber Placement</rdfs:label>
    </owl:Class>
    


    <!-- http://www.semanticweb.org/qihan/ontologies/2023/6/untitled-ontology-12#Fibre_Mat_Reinforced_Composite -->

    <owl:Class rdf:about="http://www.semanticweb.org/qihan/ontologies/2023/6/untitled-ontology-12#Fibre_Mat_Reinforced_Composite">
        <rdfs:subClassOf rdf:resource="http://www.semanticweb.org/qihan/ontologies/2023/6/untitled-ontology-12#Discontinuous_Fiber_Composite"/>
    </owl:Class>
    


    <!-- http://www.semanticweb.org/qihan/ontologies/2023/6/untitled-ontology-12#Filament_Winding_Processes -->

    <owl:Class rdf:about="http://www.semanticweb.org/qihan/ontologies/2023/6/untitled-ontology-12#Filament_Winding_Processes">
        <rdfs:subClassOf rdf:resource="http://www.semanticweb.org/qihan/ontologies/2023/6/untitled-ontology-12#Material_Manufacturing"/>
        <rdfs:comment>Represents a category of manufacturing processes used to produce composite structures by winding continuous fibers (filaments) around a mandrel or mold in a specific pattern.</rdfs:comment>
        <rdfs:label>Filament Winding Processes</rdfs:label>
    </owl:Class>
    


    <!-- http://www.semanticweb.org/qihan/ontologies/2023/6/untitled-ontology-12#Flat_Plate_Specimen -->

    <owl:Class rdf:about="http://www.semanticweb.org/qihan/ontologies/2023/6/untitled-ontology-12#Flat_Plate_Specimen">
        <rdfs:subClassOf rdf:resource="http://www.semanticweb.org/qihan/ontologies/2023/6/untitled-ontology-12#Test_Specimen_Geometry"/>
        <rdfs:comment>Represents a type of test specimen with a flat and uniform thickness, often used for simple and basic mechanical tests, such as tension and compression tests.</rdfs:comment>
        <rdfs:label>Flat Plate Specimen</rdfs:label>
    </owl:Class>
    


    <!-- http://www.semanticweb.org/qihan/ontologies/2023/6/untitled-ontology-12#Flax_Fiber_Composite -->

    <owl:Class rdf:about="http://www.semanticweb.org/qihan/ontologies/2023/6/untitled-ontology-12#Flax_Fiber_Composite">
        <rdfs:subClassOf rdf:resource="http://www.semanticweb.org/qihan/ontologies/2023/6/untitled-ontology-12#Natural_Fiber_Composite"/>
    </owl:Class>
    


    <!-- http://www.semanticweb.org/qihan/ontologies/2023/6/untitled-ontology-12#Flexural_Instron_Machine -->

    <owl:Class rdf:about="http://www.semanticweb.org/qihan/ontologies/2023/6/untitled-ontology-12#Flexural_Instron_Machine">
        <rdfs:subClassOf rdf:resource="http://www.semanticweb.org/qihan/ontologies/2023/6/untitled-ontology-12#Instron_Machine"/>
        <rdfs:comment>Represents a specific type of Instron machine used for conducting flexural or bending tests on materials.</rdfs:comment>
        <rdfs:label>Flextural Instron Machine</rdfs:label>
    </owl:Class>
    


    <!-- http://www.semanticweb.org/qihan/ontologies/2023/6/untitled-ontology-12#Flexural_Load -->

    <owl:Class rdf:about="http://www.semanticweb.org/qihan/ontologies/2023/6/untitled-ontology-12#Flexural_Load">
        <rdfs:subClassOf rdf:resource="http://www.semanticweb.org/qihan/ontologies/2023/6/untitled-ontology-12#Load"/>
        <rdfs:comment>Represents the external force or load applied to a material, to cause bending or flexural deformation.</rdfs:comment>
        <rdfs:label>Flexural Load</rdfs:label>
    </owl:Class>
    


    <!-- http://www.semanticweb.org/qihan/ontologies/2023/6/untitled-ontology-12#Flexural_Modulus -->

    <owl:Class rdf:about="http://www.semanticweb.org/qihan/ontologies/2023/6/untitled-ontology-12#Flexural_Modulus">
        <rdfs:subClassOf rdf:resource="http://www.semanticweb.org/qihan/ontologies/2023/6/untitled-ontology-12#Stiffness"/>
    </owl:Class>
    


    <!-- http://www.semanticweb.org/qihan/ontologies/2023/6/untitled-ontology-12#Flexural_Strength -->

    <owl:Class rdf:about="http://www.semanticweb.org/qihan/ontologies/2023/6/untitled-ontology-12#Flexural_Strength">
        <rdfs:subClassOf rdf:resource="http://www.semanticweb.org/qihan/ontologies/2023/6/untitled-ontology-12#Strength"/>
    </owl:Class>
    


    <!-- http://www.semanticweb.org/qihan/ontologies/2023/6/untitled-ontology-12#Flexural_Stress -->

    <owl:Class rdf:about="http://www.semanticweb.org/qihan/ontologies/2023/6/untitled-ontology-12#Flexural_Stress">
        <rdfs:subClassOf rdf:resource="http://www.semanticweb.org/qihan/ontologies/2023/6/untitled-ontology-12#Stress"/>
        <rdfs:comment>Represents the internal resistance or force per unit area that a material experiences when subjected to bending forces.</rdfs:comment>
        <rdfs:label>Flexural Stress</rdfs:label>
    </owl:Class>
    


    <!-- http://www.semanticweb.org/qihan/ontologies/2023/6/untitled-ontology-12#Flexural_Testing -->

    <owl:Class rdf:about="http://www.semanticweb.org/qihan/ontologies/2023/6/untitled-ontology-12#Flexural_Testing">
        <rdfs:subClassOf rdf:resource="http://www.semanticweb.org/qihan/ontologies/2023/6/untitled-ontology-12#Testing_Method"/>
        <rdfs:comment>Represents a type of mechanical testing used to evaluate the flexural or bending properties of materials.</rdfs:comment>
        <rdfs:label>Flexural Testing</rdfs:label>
    </owl:Class>
    


    <!-- http://www.semanticweb.org/qihan/ontologies/2023/6/untitled-ontology-12#Fluids -->

    <owl:Class rdf:about="http://www.semanticweb.org/qihan/ontologies/2023/6/untitled-ontology-12#Fluids">
        <rdfs:subClassOf rdf:resource="http://www.semanticweb.org/qihan/ontologies/2023/6/untitled-ontology-12#Medium"/>
        <rdfs:comment>Represents the medium of the testing environment for mechanical testing of composite material specimens. It includes various types of liquids or gases used as testing mediums, such as water, oil, or gases other than air.</rdfs:comment>
        <rdfs:label>Fluids</rdfs:label>
    </owl:Class>
    


    <!-- http://www.semanticweb.org/qihan/ontologies/2023/6/untitled-ontology-12#Foam_Core_Composite -->

    <owl:Class rdf:about="http://www.semanticweb.org/qihan/ontologies/2023/6/untitled-ontology-12#Foam_Core_Composite">
        <rdfs:subClassOf rdf:resource="http://www.semanticweb.org/qihan/ontologies/2023/6/untitled-ontology-12#Sandwich_Composite"/>
    </owl:Class>
    


    <!-- http://www.semanticweb.org/qihan/ontologies/2023/6/untitled-ontology-12#Four-Point_Bending_Specimen -->

    <owl:Class rdf:about="http://www.semanticweb.org/qihan/ontologies/2023/6/untitled-ontology-12#Four-Point_Bending_Specimen">
        <rdfs:subClassOf rdf:resource="http://www.semanticweb.org/qihan/ontologies/2023/6/untitled-ontology-12#Test_Specimen_Geometry"/>
        <rdfs:comment>Represents a type of test specimen with two loading points and two support points, creating a four-point bending configuration.</rdfs:comment>
        <rdfs:label>Four Point Bending Specimen</rdfs:label>
    </owl:Class>
    


    <!-- http://www.semanticweb.org/qihan/ontologies/2023/6/untitled-ontology-12#Fracture_Toughness -->

    <owl:Class rdf:about="http://www.semanticweb.org/qihan/ontologies/2023/6/untitled-ontology-12#Fracture_Toughness">
        <rdfs:subClassOf rdf:resource="http://www.semanticweb.org/qihan/ontologies/2023/6/untitled-ontology-12#Toughness"/>
    </owl:Class>
    


    <!-- http://www.semanticweb.org/qihan/ontologies/2023/6/untitled-ontology-12#Fracture_Toughness_Testing -->

    <owl:Class rdf:about="http://www.semanticweb.org/qihan/ontologies/2023/6/untitled-ontology-12#Fracture_Toughness_Testing">
        <rdfs:subClassOf rdf:resource="http://www.semanticweb.org/qihan/ontologies/2023/6/untitled-ontology-12#Testing_Method"/>
        <rdfs:comment>Represents a type of mechanical testing used to measure the fracture toughness of materials.</rdfs:comment>
        <rdfs:label>Fracture Toughness Testing</rdfs:label>
    </owl:Class>
    


    <!-- http://www.semanticweb.org/qihan/ontologies/2023/6/untitled-ontology-12#Frequency -->

    <owl:Class rdf:about="http://www.semanticweb.org/qihan/ontologies/2023/6/untitled-ontology-12#Frequency">
        <rdfs:subClassOf rdf:resource="http://www.semanticweb.org/qihan/ontologies/2023/6/untitled-ontology-12#Test_Parameter"/>
        <rdfs:comment>Represents a physical quantity that measures the number of occurrences of a periodic event or vibration per unit of time.</rdfs:comment>
        <rdfs:label>Frequency</rdfs:label>
    </owl:Class>
    


    <!-- http://www.semanticweb.org/qihan/ontologies/2023/6/untitled-ontology-12#Full-Bridge_Configuration -->

    <owl:Class rdf:about="http://www.semanticweb.org/qihan/ontologies/2023/6/untitled-ontology-12#Full-Bridge_Configuration">
        <rdfs:subClassOf rdf:resource="http://www.semanticweb.org/qihan/ontologies/2023/6/untitled-ontology-12#Strain_Gauge_Configuration"/>
        <rdfs:comment>Represents a configuration of strain gauges or sensors in which all four arms of the Wheatstone bridge circuit are active. The full-bridge configuration is commonly used for accurate measurement of strain in mechanical testing and structural monitoring applications.</rdfs:comment>
        <rdfs:label>Full-Bridge Configuration</rdfs:label>
    </owl:Class>
    


    <!-- http://www.semanticweb.org/qihan/ontologies/2023/6/untitled-ontology-12#Functionally_Graded_Composite -->

    <owl:Class rdf:about="http://www.semanticweb.org/qihan/ontologies/2023/6/untitled-ontology-12#Functionally_Graded_Composite">
        <rdfs:subClassOf rdf:resource="http://www.semanticweb.org/qihan/ontologies/2023/6/untitled-ontology-12#Composite_Material"/>
    </owl:Class>
    


    <!-- http://www.semanticweb.org/qihan/ontologies/2023/6/untitled-ontology-12#Fused_Deposition_Modeling -->

    <owl:Class rdf:about="http://www.semanticweb.org/qihan/ontologies/2023/6/untitled-ontology-12#Fused_Deposition_Modeling">
        <rdfs:subClassOf rdf:resource="http://www.semanticweb.org/qihan/ontologies/2023/6/untitled-ontology-12#Additive_Manufacturing_Processes"/>
        <rdfs:comment>Represents an additive manufacturing process that uses a thermoplastic filament as the feedstock to build 3D objects layer by layer.</rdfs:comment>
        <rdfs:label>Fused Deposition Modelling (FDM)</rdfs:label>
    </owl:Class>
    


    <!-- http://www.semanticweb.org/qihan/ontologies/2023/6/untitled-ontology-12#GOST_R_ISO_14125 -->

    <owl:Class rdf:about="http://www.semanticweb.org/qihan/ontologies/2023/6/untitled-ontology-12#GOST_R_ISO_14125">
        <rdfs:subClassOf rdf:resource="http://www.semanticweb.org/qihan/ontologies/2023/6/untitled-ontology-12#GOST_Standards"/>
        <rdfs:comment>Fibre-reinforced plastic composites - Determination of flexural properties</rdfs:comment>
        <rdfs:label>GOST R ISO 14125</rdfs:label>
    </owl:Class>
    


    <!-- http://www.semanticweb.org/qihan/ontologies/2023/6/untitled-ontology-12#GOST_R_ISO_178 -->

    <owl:Class rdf:about="http://www.semanticweb.org/qihan/ontologies/2023/6/untitled-ontology-12#GOST_R_ISO_178">
        <rdfs:subClassOf rdf:resource="http://www.semanticweb.org/qihan/ontologies/2023/6/untitled-ontology-12#GOST_Standards"/>
        <rdfs:comment>Plastics - Determination of Flexural Properties</rdfs:comment>
        <rdfs:label>GOST R ISO 178</rdfs:label>
    </owl:Class>
    


    <!-- http://www.semanticweb.org/qihan/ontologies/2023/6/untitled-ontology-12#GOST_R_ISO_527 -->

    <owl:Class rdf:about="http://www.semanticweb.org/qihan/ontologies/2023/6/untitled-ontology-12#GOST_R_ISO_527">
        <rdfs:subClassOf rdf:resource="http://www.semanticweb.org/qihan/ontologies/2023/6/untitled-ontology-12#GOST_Standards"/>
        <rdfs:comment>Plastics - Determination of Tensile Properties</rdfs:comment>
        <rdfs:label>GOST R ISO 527</rdfs:label>
    </owl:Class>
    


    <!-- http://www.semanticweb.org/qihan/ontologies/2023/6/untitled-ontology-12#GOST_Standards -->

    <owl:Class rdf:about="http://www.semanticweb.org/qihan/ontologies/2023/6/untitled-ontology-12#GOST_Standards">
        <rdfs:subClassOf rdf:resource="http://www.semanticweb.org/qihan/ontologies/2023/6/untitled-ontology-12#Test_Standards"/>
        <rdfs:label>Gosudarstvennye Standarty - Russian Standards (GOST)</rdfs:label>
    </owl:Class>
    


    <!-- http://www.semanticweb.org/qihan/ontologies/2023/6/untitled-ontology-12#Glass_Fibre_Reinforced_Polymer -->

    <owl:Class rdf:about="http://www.semanticweb.org/qihan/ontologies/2023/6/untitled-ontology-12#Glass_Fibre_Reinforced_Polymer">
        <rdfs:subClassOf rdf:resource="http://www.semanticweb.org/qihan/ontologies/2023/6/untitled-ontology-12#Polymer_Matrix_Composite"/>
    </owl:Class>
    


    <!-- http://www.semanticweb.org/qihan/ontologies/2023/6/untitled-ontology-12#Government_Testing_Agency -->

    <owl:Class rdf:about="http://www.semanticweb.org/qihan/ontologies/2023/6/untitled-ontology-12#Government_Testing_Agency">
        <rdfs:subClassOf rdf:resource="http://www.semanticweb.org/qihan/ontologies/2023/6/untitled-ontology-12#Testing_Institution"/>
        <rdfs:comment>Represents a specific type of testing institution that is operated and funded by a government entity.</rdfs:comment>
        <rdfs:label>Government Testing Agency</rdfs:label>
    </owl:Class>
    


    <!-- http://www.semanticweb.org/qihan/ontologies/2023/6/untitled-ontology-12#Graphene_Composite -->

    <owl:Class rdf:about="http://www.semanticweb.org/qihan/ontologies/2023/6/untitled-ontology-12#Graphene_Composite">
        <rdfs:subClassOf rdf:resource="http://www.semanticweb.org/qihan/ontologies/2023/6/untitled-ontology-12#Nanocomposite"/>
    </owl:Class>
    


    <!-- http://www.semanticweb.org/qihan/ontologies/2023/6/untitled-ontology-12#Grinding_Wheel -->

    <owl:Class rdf:about="http://www.semanticweb.org/qihan/ontologies/2023/6/untitled-ontology-12#Grinding_Wheel">
        <rdfs:subClassOf rdf:resource="http://www.semanticweb.org/qihan/ontologies/2023/6/untitled-ontology-12#Grinding_and_Sanding_Equipment"/>
        <rdfs:comment>Represents an abrasive wheel used in grinding machines for material removal and surface finishing.</rdfs:comment>
        <rdfs:label>Grinding Wheel</rdfs:label>
    </owl:Class>
    


    <!-- http://www.semanticweb.org/qihan/ontologies/2023/6/untitled-ontology-12#Grinding_and_Sanding_Equipment -->

    <owl:Class rdf:about="http://www.semanticweb.org/qihan/ontologies/2023/6/untitled-ontology-12#Grinding_and_Sanding_Equipment">
        <rdfs:subClassOf rdf:resource="http://www.semanticweb.org/qihan/ontologies/2023/6/untitled-ontology-12#Specimen_Preparation_Equipment"/>
        <rdfs:comment>Represents a category of machines and tools used for material removal and surface finishing through grinding and sanding processes.</rdfs:comment>
        <rdfs:label>Grinding and Sanding Equipment</rdfs:label>
    </owl:Class>
    


    <!-- http://www.semanticweb.org/qihan/ontologies/2023/6/untitled-ontology-12#Guarded_Heat_Flow_Meter -->

    <owl:Class rdf:about="http://www.semanticweb.org/qihan/ontologies/2023/6/untitled-ontology-12#Guarded_Heat_Flow_Meter">
        <rdfs:subClassOf rdf:resource="http://www.semanticweb.org/qihan/ontologies/2023/6/untitled-ontology-12#Thermal_Conductivity_Measurement_Apparatus"/>
        <rdfs:comment>Represents a specialized instrument used to measure the thermal conductivity of materials.</rdfs:comment>
        <rdfs:label>Guarded Heat Flow Meter</rdfs:label>
    </owl:Class>
    


    <!-- http://www.semanticweb.org/qihan/ontologies/2023/6/untitled-ontology-12#Hacksaws -->

    <owl:Class rdf:about="http://www.semanticweb.org/qihan/ontologies/2023/6/untitled-ontology-12#Hacksaws">
        <rdfs:subClassOf rdf:resource="http://www.semanticweb.org/qihan/ontologies/2023/6/untitled-ontology-12#Handheld_Cutting_Tools"/>
        <rdfs:comment>Represents a type of cutting tool.</rdfs:comment>
        <rdfs:label>Hacksaws</rdfs:label>
    </owl:Class>
    


    <!-- http://www.semanticweb.org/qihan/ontologies/2023/6/untitled-ontology-12#Half-Bridge_Configuration -->

    <owl:Class rdf:about="http://www.semanticweb.org/qihan/ontologies/2023/6/untitled-ontology-12#Half-Bridge_Configuration">
        <rdfs:subClassOf rdf:resource="http://www.semanticweb.org/qihan/ontologies/2023/6/untitled-ontology-12#Strain_Gauge_Configuration"/>
        <rdfs:comment>Represents a configuration of strain gauges or sensors in which only two arms of the Wheatstone bridge circuit are active.</rdfs:comment>
        <rdfs:label>Half-Bridge Configuration</rdfs:label>
    </owl:Class>
    


    <!-- http://www.semanticweb.org/qihan/ontologies/2023/6/untitled-ontology-12#Hand_Layup -->

    <owl:Class rdf:about="http://www.semanticweb.org/qihan/ontologies/2023/6/untitled-ontology-12#Hand_Layup">
        <rdfs:subClassOf rdf:resource="http://www.semanticweb.org/qihan/ontologies/2023/6/untitled-ontology-12#Layup_Processes"/>
        <rdfs:comment>Represents a manual layup process where layers of reinforcing fibers and resin are manually positioned onto a mold or tool to form a composite laminate.</rdfs:comment>
        <rdfs:label>Hand Layup</rdfs:label>
    </owl:Class>
    


    <!-- http://www.semanticweb.org/qihan/ontologies/2023/6/untitled-ontology-12#Hand_Layup_and_Press_Forming -->

    <owl:Class rdf:about="http://www.semanticweb.org/qihan/ontologies/2023/6/untitled-ontology-12#Hand_Layup_and_Press_Forming">
        <rdfs:subClassOf rdf:resource="http://www.semanticweb.org/qihan/ontologies/2023/6/untitled-ontology-12#Sheet_Forming_Processes"/>
        <rdfs:comment>Represents a specific sheet forming process where layers of dry fibers or pre-impregnated prepreg sheets are manually laid up in a mold or tool.</rdfs:comment>
        <rdfs:label>Hand Layup and Press Forming</rdfs:label>
    </owl:Class>
    


    <!-- http://www.semanticweb.org/qihan/ontologies/2023/6/untitled-ontology-12#Handheld_Cutting_Tools -->

    <owl:Class rdf:about="http://www.semanticweb.org/qihan/ontologies/2023/6/untitled-ontology-12#Handheld_Cutting_Tools">
        <rdfs:subClassOf rdf:resource="http://www.semanticweb.org/qihan/ontologies/2023/6/untitled-ontology-12#Cutting_Equipment"/>
        <rdfs:comment>Represents a category of cutting tools that are operated manually by hand.</rdfs:comment>
        <rdfs:label>Handheld Cutting Tools</rdfs:label>
    </owl:Class>
    


    <!-- http://www.semanticweb.org/qihan/ontologies/2023/6/untitled-ontology-12#Handsaws -->

    <owl:Class rdf:about="http://www.semanticweb.org/qihan/ontologies/2023/6/untitled-ontology-12#Handsaws">
        <rdfs:subClassOf rdf:resource="http://www.semanticweb.org/qihan/ontologies/2023/6/untitled-ontology-12#Handheld_Cutting_Tools"/>
        <rdfs:comment>Represents a type of cutting tool.</rdfs:comment>
        <rdfs:label>Handsaws</rdfs:label>
    </owl:Class>
    


    <!-- http://www.semanticweb.org/qihan/ontologies/2023/6/untitled-ontology-12#Hardness -->

    <owl:Class rdf:about="http://www.semanticweb.org/qihan/ontologies/2023/6/untitled-ontology-12#Hardness">
        <rdfs:subClassOf rdf:resource="http://www.semanticweb.org/qihan/ontologies/2023/6/untitled-ontology-12#Result_Calculation"/>
    </owl:Class>
    


    <!-- http://www.semanticweb.org/qihan/ontologies/2023/6/untitled-ontology-12#Hardness_Tester -->

    <owl:Class rdf:about="http://www.semanticweb.org/qihan/ontologies/2023/6/untitled-ontology-12#Hardness_Tester">
        <rdfs:subClassOf rdf:resource="http://www.semanticweb.org/qihan/ontologies/2023/6/untitled-ontology-12#Test_Equipment"/>
        <rdfs:comment>Represents a test equipment used to determine the hardness of composite material specimens. It measures the material&apos;s resistance to indentation or scratching under specified conditions.</rdfs:comment>
        <rdfs:label>Hardness Tester</rdfs:label>
    </owl:Class>
    


    <!-- http://www.semanticweb.org/qihan/ontologies/2023/6/untitled-ontology-12#Hardness_Testing -->

    <owl:Class rdf:about="http://www.semanticweb.org/qihan/ontologies/2023/6/untitled-ontology-12#Hardness_Testing">
        <rdfs:subClassOf rdf:resource="http://www.semanticweb.org/qihan/ontologies/2023/6/untitled-ontology-12#Testing_Method"/>
        <rdfs:label>Hardness Testing</rdfs:label>
    </owl:Class>
    


    <!-- http://www.semanticweb.org/qihan/ontologies/2023/6/untitled-ontology-12#Heat_Deflection_Temperature_Testing -->

    <owl:Class rdf:about="http://www.semanticweb.org/qihan/ontologies/2023/6/untitled-ontology-12#Heat_Deflection_Temperature_Testing">
        <rdfs:subClassOf rdf:resource="http://www.semanticweb.org/qihan/ontologies/2023/6/untitled-ontology-12#Thermal_Testing"/>
        <rdfs:comment>Represents a type of thermal testing used to determine the heat deflection temperature (HDT) of materials.</rdfs:comment>
        <rdfs:label>Heat Deflection Temperature</rdfs:label>
    </owl:Class>
    


    <!-- http://www.semanticweb.org/qihan/ontologies/2023/6/untitled-ontology-12#Hemp_Fiber_Composite -->

    <owl:Class rdf:about="http://www.semanticweb.org/qihan/ontologies/2023/6/untitled-ontology-12#Hemp_Fiber_Composite">
        <rdfs:subClassOf rdf:resource="http://www.semanticweb.org/qihan/ontologies/2023/6/untitled-ontology-12#Natural_Fiber_Composite"/>
    </owl:Class>
    


    <!-- http://www.semanticweb.org/qihan/ontologies/2023/6/untitled-ontology-12#High-Speed_Camera -->

    <owl:Class rdf:about="http://www.semanticweb.org/qihan/ontologies/2023/6/untitled-ontology-12#High-Speed_Camera">
        <rdfs:subClassOf rdf:resource="http://www.semanticweb.org/qihan/ontologies/2023/6/untitled-ontology-12#Test_Equipment"/>
        <rdfs:comment>Represents a specialized camera capable of capturing high-speed video recordings during mechanical testing of composite material specimens. It enables the visualization and analysis of rapid material responses and failure modes.</rdfs:comment>
        <rdfs:label>High-Speed Camera</rdfs:label>
    </owl:Class>
    


    <!-- http://www.semanticweb.org/qihan/ontologies/2023/6/untitled-ontology-12#Honeycomb_Core_Composite -->

    <owl:Class rdf:about="http://www.semanticweb.org/qihan/ontologies/2023/6/untitled-ontology-12#Honeycomb_Core_Composite">
        <rdfs:subClassOf rdf:resource="http://www.semanticweb.org/qihan/ontologies/2023/6/untitled-ontology-12#Sandwich_Composite"/>
    </owl:Class>
    


    <!-- http://www.semanticweb.org/qihan/ontologies/2023/6/untitled-ontology-12#Hoop_Filament_Winding -->

    <owl:Class rdf:about="http://www.semanticweb.org/qihan/ontologies/2023/6/untitled-ontology-12#Hoop_Filament_Winding">
        <rdfs:subClassOf rdf:resource="http://www.semanticweb.org/qihan/ontologies/2023/6/untitled-ontology-12#Filament_Winding_Processes"/>
        <rdfs:comment>Represents a specific filament winding process where continuous fibers are wound around a mandrel or mold in a circumferential direction (hoop direction).</rdfs:comment>
        <rdfs:label>Hoop Filament Winding</rdfs:label>
    </owl:Class>
    


    <!-- http://www.semanticweb.org/qihan/ontologies/2023/6/untitled-ontology-12#Hourglass_Specimen -->

    <owl:Class rdf:about="http://www.semanticweb.org/qihan/ontologies/2023/6/untitled-ontology-12#Hourglass_Specimen">
        <rdfs:subClassOf rdf:resource="http://www.semanticweb.org/qihan/ontologies/2023/6/untitled-ontology-12#Test_Specimen_Geometry"/>
        <rdfs:comment>Represents a type of test specimen with a waist-like or hourglass shape, often used in compression tests to induce localized deformation and controlled failure.</rdfs:comment>
        <rdfs:label>Hourglass Specimen</rdfs:label>
    </owl:Class>
    


    <!-- http://www.semanticweb.org/qihan/ontologies/2023/6/untitled-ontology-12#Humidity -->

    <owl:Class rdf:about="http://www.semanticweb.org/qihan/ontologies/2023/6/untitled-ontology-12#Humidity">
        <rdfs:subClassOf rdf:resource="http://www.semanticweb.org/qihan/ontologies/2023/6/untitled-ontology-12#Test_Environment"/>
        <rdfs:subClassOf rdf:resource="http://www.semanticweb.org/qihan/ontologies/2023/6/untitled-ontology-12#Test_Parameter"/>
        <rdfs:comment>Represents the amount of water vapor present in the air or atmosphere. Humidity is typically measured as a percentage, indicating the relative amount of water vapor compared to the maximum amount the air can hold at a specific temperature.</rdfs:comment>
        <rdfs:label>Humidty</rdfs:label>
    </owl:Class>
    


    <!-- http://www.semanticweb.org/qihan/ontologies/2023/6/untitled-ontology-12#Hybrid_Polymer_Matrix_Composite -->

    <owl:Class rdf:about="http://www.semanticweb.org/qihan/ontologies/2023/6/untitled-ontology-12#Hybrid_Polymer_Matrix_Composite">
        <rdfs:subClassOf rdf:resource="http://www.semanticweb.org/qihan/ontologies/2023/6/untitled-ontology-12#Polymer_Matrix_Composite"/>
    </owl:Class>
    


    <!-- http://www.semanticweb.org/qihan/ontologies/2023/6/untitled-ontology-12#Hydraulic_Testing_Machine -->

    <owl:Class rdf:about="http://www.semanticweb.org/qihan/ontologies/2023/6/untitled-ontology-12#Hydraulic_Testing_Machine">
        <rdfs:subClassOf rdf:resource="http://www.semanticweb.org/qihan/ontologies/2023/6/untitled-ontology-12#Universal_Testing_Machine"/>
        <rdfs:comment>Represents a type of testing machine that uses hydraulic systems to apply forces and deformations to materials.</rdfs:comment>
        <rdfs:label>Hydraulic Testing Machine</rdfs:label>
    </owl:Class>
    


    <!-- http://www.semanticweb.org/qihan/ontologies/2023/6/untitled-ontology-12#ISO_11542 -->

    <owl:Class rdf:about="http://www.semanticweb.org/qihan/ontologies/2023/6/untitled-ontology-12#ISO_11542">
        <rdfs:subClassOf rdf:resource="http://www.semanticweb.org/qihan/ontologies/2023/6/untitled-ontology-12#Double_Cantilever_Beam_Specimen"/>
        <rdfs:comment>Represents a standard titled &quot;Carbon fibre-reinforced plastics — Determination of interlaminar shear stress, ±45° shear method&quot;.</rdfs:comment>
        <rdfs:label>ISO 11542</rdfs:label>
    </owl:Class>
    


    <!-- http://www.semanticweb.org/qihan/ontologies/2023/6/untitled-ontology-12#ISO_13003 -->

    <owl:Class rdf:about="http://www.semanticweb.org/qihan/ontologies/2023/6/untitled-ontology-12#ISO_13003">
        <rdfs:subClassOf rdf:resource="http://www.semanticweb.org/qihan/ontologies/2023/6/untitled-ontology-12#Fatigue_Testing"/>
        <rdfs:comment>Represents a specific ISO standard titled &quot;Fibre-Reinforced Plastic Composites - Determination of Flexural Properties&quot;.</rdfs:comment>
        <rdfs:label>ISO 13003</rdfs:label>
    </owl:Class>
    


    <!-- http://www.semanticweb.org/qihan/ontologies/2023/6/untitled-ontology-12#ISO_13586 -->

    <owl:Class rdf:about="http://www.semanticweb.org/qihan/ontologies/2023/6/untitled-ontology-12#ISO_13586">
        <rdfs:subClassOf rdf:resource="http://www.semanticweb.org/qihan/ontologies/2023/6/untitled-ontology-12#End-Notched_Flexure_Specimen"/>
        <rdfs:comment>Represents a standard titled &quot;Carbon fibre-reinforced plastics — Determination of compressive properties perpendicular to the plane of the laminate&quot;.</rdfs:comment>
        <rdfs:label>ISO 13586</rdfs:label>
    </owl:Class>
    


    <!-- http://www.semanticweb.org/qihan/ontologies/2023/6/untitled-ontology-12#ISO_14125 -->

    <owl:Class rdf:about="http://www.semanticweb.org/qihan/ontologies/2023/6/untitled-ontology-12#ISO_14125">
        <rdfs:subClassOf rdf:resource="http://www.semanticweb.org/qihan/ontologies/2023/6/untitled-ontology-12#Four-Point_Bending_Specimen"/>
        <rdfs:subClassOf rdf:resource="http://www.semanticweb.org/qihan/ontologies/2023/6/untitled-ontology-12#Short_Beam_Specimen"/>
        <rdfs:comment>Represents a standard titled &quot;Fibre-reinforced plastic composites - Determination of flexural properties&quot;.</rdfs:comment>
        <rdfs:label>ISO 14125</rdfs:label>
    </owl:Class>
    


    <!-- http://www.semanticweb.org/qihan/ontologies/2023/6/untitled-ontology-12#ISO_14126 -->

    <owl:Class rdf:about="http://www.semanticweb.org/qihan/ontologies/2023/6/untitled-ontology-12#ISO_14126">
        <rdfs:subClassOf rdf:resource="http://www.semanticweb.org/qihan/ontologies/2023/6/untitled-ontology-12#Compression_Testing"/>
        <rdfs:comment>Represents a specific ISO standard titled &quot;Fibre-Reinforced Plastic Composites - Determination of Apparent Interlaminar Shear Strength by Short-Beam Method&quot;.</rdfs:comment>
        <rdfs:label>ISO 14126</rdfs:label>
    </owl:Class>
    


    <!-- http://www.semanticweb.org/qihan/ontologies/2023/6/untitled-ontology-12#ISO_14129 -->

    <owl:Class rdf:about="http://www.semanticweb.org/qihan/ontologies/2023/6/untitled-ontology-12#ISO_14129">
        <rdfs:subClassOf rdf:resource="http://www.semanticweb.org/qihan/ontologies/2023/6/untitled-ontology-12#Shear_Testing"/>
        <rdfs:comment>Represents a specific ISO standard that specifies the test method for determining the in-plane shear properties of continuous fiber-reinforced composite materials.</rdfs:comment>
        <rdfs:label>ISO 14129</rdfs:label>
    </owl:Class>
    


    <!-- http://www.semanticweb.org/qihan/ontologies/2023/6/untitled-ontology-12#ISO_14130 -->

    <owl:Class rdf:about="http://www.semanticweb.org/qihan/ontologies/2023/6/untitled-ontology-12#ISO_14130">
        <rdfs:subClassOf rdf:resource="http://www.semanticweb.org/qihan/ontologies/2023/6/untitled-ontology-12#Flat_Plate_Specimen"/>
        <rdfs:subClassOf rdf:resource="http://www.semanticweb.org/qihan/ontologies/2023/6/untitled-ontology-12#Hourglass_Specimen"/>
        <rdfs:subClassOf rdf:resource="http://www.semanticweb.org/qihan/ontologies/2023/6/untitled-ontology-12#ISO_Standards"/>
        <rdfs:subClassOf rdf:resource="http://www.semanticweb.org/qihan/ontologies/2023/6/untitled-ontology-12#V-Notched_Beam_Specimen"/>
        <rdfs:comment>Fibre-reinforced plastic composites - Determination of shear properties by the plate twist method</rdfs:comment>
        <rdfs:label>ISO 14130</rdfs:label>
    </owl:Class>
    


    <!-- http://www.semanticweb.org/qihan/ontologies/2023/6/untitled-ontology-12#ISO_178 -->

    <owl:Class rdf:about="http://www.semanticweb.org/qihan/ontologies/2023/6/untitled-ontology-12#ISO_178">
        <rdfs:subClassOf rdf:resource="http://www.semanticweb.org/qihan/ontologies/2023/6/untitled-ontology-12#Cantilever_Beam_Specimen"/>
        <rdfs:subClassOf rdf:resource="http://www.semanticweb.org/qihan/ontologies/2023/6/untitled-ontology-12#Flexural_Testing"/>
        <rdfs:subClassOf rdf:resource="http://www.semanticweb.org/qihan/ontologies/2023/6/untitled-ontology-12#ISO_Standards"/>
        <rdfs:subClassOf rdf:resource="http://www.semanticweb.org/qihan/ontologies/2023/6/untitled-ontology-12#Three-Point_Bending_Specimen"/>
        <rdfs:comment>Plastics - Determination of Flexural Properties</rdfs:comment>
        <rdfs:label>ISO 178</rdfs:label>
    </owl:Class>
    


    <!-- http://www.semanticweb.org/qihan/ontologies/2023/6/untitled-ontology-12#ISO_179 -->

    <owl:Class rdf:about="http://www.semanticweb.org/qihan/ontologies/2023/6/untitled-ontology-12#ISO_179">
        <rdfs:subClassOf rdf:resource="http://www.semanticweb.org/qihan/ontologies/2023/6/untitled-ontology-12#Impact_Testing"/>
        <rdfs:comment>Represents a specific ISO standard titled &quot;Plastics - Determination of Charpy Impact Strength&quot;.</rdfs:comment>
        <rdfs:label>ISO 179</rdfs:label>
    </owl:Class>
    


    <!-- http://www.semanticweb.org/qihan/ontologies/2023/6/untitled-ontology-12#ISO_527 -->

    <owl:Class rdf:about="http://www.semanticweb.org/qihan/ontologies/2023/6/untitled-ontology-12#ISO_527">
        <rdfs:subClassOf rdf:resource="http://www.semanticweb.org/qihan/ontologies/2023/6/untitled-ontology-12#Dogbone_Specimen"/>
        <rdfs:subClassOf rdf:resource="http://www.semanticweb.org/qihan/ontologies/2023/6/untitled-ontology-12#ISO_Standards"/>
        <rdfs:subClassOf rdf:resource="http://www.semanticweb.org/qihan/ontologies/2023/6/untitled-ontology-12#Tensile_Testing"/>
        <rdfs:comment>Represents a specific ISO standard that outlines the test methods for determining the tensile properties of plastic materials, including thermoplastic and thermosetting materials.</rdfs:comment>
        <rdfs:label>ISO 527</rdfs:label>
    </owl:Class>
    


    <!-- http://www.semanticweb.org/qihan/ontologies/2023/6/untitled-ontology-12#ISO_7751 -->

    <owl:Class rdf:about="http://www.semanticweb.org/qihan/ontologies/2023/6/untitled-ontology-12#ISO_7751">
        <rdfs:subClassOf rdf:resource="http://www.semanticweb.org/qihan/ontologies/2023/6/untitled-ontology-12#Circular_Disk_Specimen"/>
        <rdfs:comment>Represents a standard titled &quot;Plastics - Compression-moulding test specimens of thermoplastic materials&quot;.</rdfs:comment>
        <rdfs:label>ISO 7751</rdfs:label>
    </owl:Class>
    


    <!-- http://www.semanticweb.org/qihan/ontologies/2023/6/untitled-ontology-12#ISO_Standards -->

    <owl:Class rdf:about="http://www.semanticweb.org/qihan/ontologies/2023/6/untitled-ontology-12#ISO_Standards">
        <rdfs:subClassOf rdf:resource="http://www.semanticweb.org/qihan/ontologies/2023/6/untitled-ontology-12#Test_Standards"/>
        <rdfs:label>International Organization for Standardization (ISO)</rdfs:label>
    </owl:Class>
    


    <!-- http://www.semanticweb.org/qihan/ontologies/2023/6/untitled-ontology-12#Impact_Acceleration -->

    <owl:Class rdf:about="http://www.semanticweb.org/qihan/ontologies/2023/6/untitled-ontology-12#Impact_Acceleration">
        <rdfs:subClassOf rdf:resource="http://www.semanticweb.org/qihan/ontologies/2023/6/untitled-ontology-12#Acceleration"/>
        <rdfs:comment>Represents the rate of change of velocity experienced by a material due to an impact or suddene application of force.</rdfs:comment>
        <rdfs:label>Impact Acceleration</rdfs:label>
    </owl:Class>
    


    <!-- http://www.semanticweb.org/qihan/ontologies/2023/6/untitled-ontology-12#Impact_Load -->

    <owl:Class rdf:about="http://www.semanticweb.org/qihan/ontologies/2023/6/untitled-ontology-12#Impact_Load">
        <rdfs:subClassOf rdf:resource="http://www.semanticweb.org/qihan/ontologies/2023/6/untitled-ontology-12#Load"/>
        <rdfs:comment>Represents the sudden and intense external force or load applied to a material, in a short duration.</rdfs:comment>
        <rdfs:label>Impact Load</rdfs:label>
    </owl:Class>
    


    <!-- http://www.semanticweb.org/qihan/ontologies/2023/6/untitled-ontology-12#Impact_Tester -->

    <owl:Class rdf:about="http://www.semanticweb.org/qihan/ontologies/2023/6/untitled-ontology-12#Impact_Tester">
        <rdfs:subClassOf rdf:resource="http://www.semanticweb.org/qihan/ontologies/2023/6/untitled-ontology-12#Test_Equipment"/>
        <rdfs:comment>Represents a specific type of test equipment used to evaluate the impact resistance and toughness of composite material specimens. It applies controlled impact loads to assess the material&apos;s ability to withstand sudden forces and absorb energy without fracturing.</rdfs:comment>
        <rdfs:label>Impact Tester</rdfs:label>
    </owl:Class>
    


    <!-- http://www.semanticweb.org/qihan/ontologies/2023/6/untitled-ontology-12#Impact_Testing -->

    <owl:Class rdf:about="http://www.semanticweb.org/qihan/ontologies/2023/6/untitled-ontology-12#Impact_Testing">
        <rdfs:subClassOf rdf:resource="http://www.semanticweb.org/qihan/ontologies/2023/6/untitled-ontology-12#Testing_Method"/>
        <rdfs:comment>Represents a type of mechanical testing used to assess the ability of materials to resist sudden and dynamic loading.</rdfs:comment>
        <rdfs:label>Impact Testing</rdfs:label>
    </owl:Class>
    


    <!-- http://www.semanticweb.org/qihan/ontologies/2023/6/untitled-ontology-12#Impact_Toughness -->

    <owl:Class rdf:about="http://www.semanticweb.org/qihan/ontologies/2023/6/untitled-ontology-12#Impact_Toughness">
        <rdfs:subClassOf rdf:resource="http://www.semanticweb.org/qihan/ontologies/2023/6/untitled-ontology-12#Toughness"/>
    </owl:Class>
    


    <!-- http://www.semanticweb.org/qihan/ontologies/2023/6/untitled-ontology-12#In-Testing_Phase -->

    <owl:Class rdf:about="http://www.semanticweb.org/qihan/ontologies/2023/6/untitled-ontology-12#In-Testing_Phase">
        <rdfs:comment>Represents the phase of mechanical testing where actual tests are performed on composite material specimens</rdfs:comment>
    </owl:Class>
    


    <!-- http://www.semanticweb.org/qihan/ontologies/2023/6/untitled-ontology-12#Incorporation_of_Nanomaterials_into_Composites -->

    <owl:Class rdf:about="http://www.semanticweb.org/qihan/ontologies/2023/6/untitled-ontology-12#Incorporation_of_Nanomaterials_into_Composites">
        <rdfs:subClassOf rdf:resource="http://www.semanticweb.org/qihan/ontologies/2023/6/untitled-ontology-12#Nanocomposite_Synthesis"/>
        <rdfs:comment>Represents the process of integrating nanomaterials, such as nanoparticles, nanofibers, or nanotubes, into the matrix of composite materials to form nanocomposites.</rdfs:comment>
        <rdfs:label>Incorporation of Nanomaterials into Composites</rdfs:label>
    </owl:Class>
    


    <!-- http://www.semanticweb.org/qihan/ontologies/2023/6/untitled-ontology-12#Industry_Testing_Laboratory -->

    <owl:Class rdf:about="http://www.semanticweb.org/qihan/ontologies/2023/6/untitled-ontology-12#Industry_Testing_Laboratory">
        <rdfs:subClassOf rdf:resource="http://www.semanticweb.org/qihan/ontologies/2023/6/untitled-ontology-12#Testing_Institution"/>
        <rdfs:comment>Represents a specialized laboratory or testing facility operated by a private industry or manufacturing company.</rdfs:comment>
        <rdfs:label>Industry Testing Laboratory</rdfs:label>
    </owl:Class>
    


    <!-- http://www.semanticweb.org/qihan/ontologies/2023/6/untitled-ontology-12#Ingot_casting_machine -->

    <owl:Class rdf:about="http://www.semanticweb.org/qihan/ontologies/2023/6/untitled-ontology-12#Ingot_casting_machine">
        <rdfs:subClassOf rdf:resource="http://www.semanticweb.org/qihan/ontologies/2023/6/untitled-ontology-12#Casting_Machine"/>
        <rdfs:comment>Represents a type of casting machine used to produce ingots, which are large metal blocks or bars used as raw materials for further processing.</rdfs:comment>
        <rdfs:label>Ingot Casting Machine</rdfs:label>
    </owl:Class>
    


    <!-- http://www.semanticweb.org/qihan/ontologies/2023/6/untitled-ontology-12#Injection_Molding -->

    <owl:Class rdf:about="http://www.semanticweb.org/qihan/ontologies/2023/6/untitled-ontology-12#Injection_Molding">
        <rdfs:subClassOf rdf:resource="http://www.semanticweb.org/qihan/ontologies/2023/6/untitled-ontology-12#Molding_Machine"/>
        <rdfs:comment>Represents a molding process in which a material, usually plastic, is injected into a mold cavity under high pressure.</rdfs:comment>
        <rdfs:label>Injection Molding</rdfs:label>
    </owl:Class>
    


    <!-- http://www.semanticweb.org/qihan/ontologies/2023/6/untitled-ontology-12#Instron_Machine -->

    <owl:Class rdf:about="http://www.semanticweb.org/qihan/ontologies/2023/6/untitled-ontology-12#Instron_Machine">
        <rdfs:subClassOf rdf:resource="http://www.semanticweb.org/qihan/ontologies/2023/6/untitled-ontology-12#Test_Equipment"/>
        <rdfs:comment>Represents a brand or type of testing machine manufactured by Instron, a well-known company specializing in materials testing equipment.</rdfs:comment>
        <rdfs:label>Instron Machine</rdfs:label>
    </owl:Class>
    


    <!-- http://www.semanticweb.org/qihan/ontologies/2023/6/untitled-ontology-12#Interfacial_Shear_Strength -->

    <owl:Class rdf:about="http://www.semanticweb.org/qihan/ontologies/2023/6/untitled-ontology-12#Interfacial_Shear_Strength">
        <rdfs:subClassOf rdf:resource="http://www.semanticweb.org/qihan/ontologies/2023/6/untitled-ontology-12#Adhesive_Strength"/>
    </owl:Class>
    


    <!-- http://www.semanticweb.org/qihan/ontologies/2023/6/untitled-ontology-12#Interlaminar_Shear_Strength -->

    <owl:Class rdf:about="http://www.semanticweb.org/qihan/ontologies/2023/6/untitled-ontology-12#Interlaminar_Shear_Strength">
        <rdfs:subClassOf rdf:resource="http://www.semanticweb.org/qihan/ontologies/2023/6/untitled-ontology-12#Strength"/>
    </owl:Class>
    


    <!-- http://www.semanticweb.org/qihan/ontologies/2023/6/untitled-ontology-12#Internal_Friction -->

    <owl:Class rdf:about="http://www.semanticweb.org/qihan/ontologies/2023/6/untitled-ontology-12#Internal_Friction">
        <rdfs:subClassOf rdf:resource="http://www.semanticweb.org/qihan/ontologies/2023/6/untitled-ontology-12#Damping_Capacity"/>
    </owl:Class>
    


    <!-- http://www.semanticweb.org/qihan/ontologies/2023/6/untitled-ontology-12#Iosipescu_Shear_Test_Apparatus -->

    <owl:Class rdf:about="http://www.semanticweb.org/qihan/ontologies/2023/6/untitled-ontology-12#Iosipescu_Shear_Test_Apparatus">
        <rdfs:subClassOf rdf:resource="http://www.semanticweb.org/qihan/ontologies/2023/6/untitled-ontology-12#Shear_Testing_Apparatus"/>
        <rdfs:comment>Represents a specialized testing apparatus used to perform the Iosipescu shear test on composite material specimens.</rdfs:comment>
        <rdfs:label>Iosipescu Shear Test Apparatus</rdfs:label>
    </owl:Class>
    


    <!-- http://www.semanticweb.org/qihan/ontologies/2023/6/untitled-ontology-12#Iron_Matrix_Composite -->

    <owl:Class rdf:about="http://www.semanticweb.org/qihan/ontologies/2023/6/untitled-ontology-12#Iron_Matrix_Composite">
        <rdfs:subClassOf rdf:resource="http://www.semanticweb.org/qihan/ontologies/2023/6/untitled-ontology-12#Metal_Matrix_Composite"/>
    </owl:Class>
    


    <!-- http://www.semanticweb.org/qihan/ontologies/2023/6/untitled-ontology-12#Izod_Impact_Tester -->

    <owl:Class rdf:about="http://www.semanticweb.org/qihan/ontologies/2023/6/untitled-ontology-12#Izod_Impact_Tester">
        <rdfs:subClassOf rdf:resource="http://www.semanticweb.org/qihan/ontologies/2023/6/untitled-ontology-12#Impact_Tester"/>
        <rdfs:comment>Represents a specific type of impact tester used to determine the impact strength and toughness of materials, including composite material specimens.</rdfs:comment>
        <rdfs:label>Izod Impact Tester</rdfs:label>
    </owl:Class>
    


    <!-- http://www.semanticweb.org/qihan/ontologies/2023/6/untitled-ontology-12#JIS_K_6911 -->

    <owl:Class rdf:about="http://www.semanticweb.org/qihan/ontologies/2023/6/untitled-ontology-12#JIS_K_6911">
        <rdfs:subClassOf rdf:resource="http://www.semanticweb.org/qihan/ontologies/2023/6/untitled-ontology-12#JIS_Standards"/>
        <rdfs:comment>Methods of test for determining the plane shear strength of fibre-reinforced plastics</rdfs:comment>
        <rdfs:label>JIS K 6911</rdfs:label>
    </owl:Class>
    


    <!-- http://www.semanticweb.org/qihan/ontologies/2023/6/untitled-ontology-12#JIS_K_7076 -->

    <owl:Class rdf:about="http://www.semanticweb.org/qihan/ontologies/2023/6/untitled-ontology-12#JIS_K_7076">
        <rdfs:subClassOf rdf:resource="http://www.semanticweb.org/qihan/ontologies/2023/6/untitled-ontology-12#JIS_Standards"/>
        <rdfs:comment>Fibre-reinforced plastic composites - Determination of flexural properties</rdfs:comment>
        <rdfs:label>JIS K 7076</rdfs:label>
    </owl:Class>
    


    <!-- http://www.semanticweb.org/qihan/ontologies/2023/6/untitled-ontology-12#JIS_K_7163 -->

    <owl:Class rdf:about="http://www.semanticweb.org/qihan/ontologies/2023/6/untitled-ontology-12#JIS_K_7163">
        <rdfs:subClassOf rdf:resource="http://www.semanticweb.org/qihan/ontologies/2023/6/untitled-ontology-12#JIS_Standards"/>
        <rdfs:comment>Fibre-reinforced plastic composites - Determination of compressive properties</rdfs:comment>
        <rdfs:label>JIS K 7163</rdfs:label>
    </owl:Class>
    


    <!-- http://www.semanticweb.org/qihan/ontologies/2023/6/untitled-ontology-12#JIS_Standards -->

    <owl:Class rdf:about="http://www.semanticweb.org/qihan/ontologies/2023/6/untitled-ontology-12#JIS_Standards">
        <rdfs:subClassOf rdf:resource="http://www.semanticweb.org/qihan/ontologies/2023/6/untitled-ontology-12#Test_Standards"/>
        <rdfs:label>Japanese Industrial Standards (JIS)</rdfs:label>
    </owl:Class>
    


    <!-- http://www.semanticweb.org/qihan/ontologies/2023/6/untitled-ontology-12#Jolt_Machines -->

    <owl:Class rdf:about="http://www.semanticweb.org/qihan/ontologies/2023/6/untitled-ontology-12#Jolt_Machines">
        <rdfs:subClassOf rdf:resource="http://www.semanticweb.org/qihan/ontologies/2023/6/untitled-ontology-12#Molding_Machine"/>
        <rdfs:comment>Represents a type of molding machine used in foundries to compact sand molds.</rdfs:comment>
        <rdfs:label>Jolt Machines</rdfs:label>
    </owl:Class>
    


    <!-- http://www.semanticweb.org/qihan/ontologies/2023/6/untitled-ontology-12#Knitted_Fabric_Composite -->

    <owl:Class rdf:about="http://www.semanticweb.org/qihan/ontologies/2023/6/untitled-ontology-12#Knitted_Fabric_Composite">
        <rdfs:subClassOf rdf:resource="http://www.semanticweb.org/qihan/ontologies/2023/6/untitled-ontology-12#Continuous_Fiber_Composite"/>
    </owl:Class>
    


    <!-- http://www.semanticweb.org/qihan/ontologies/2023/6/untitled-ontology-12#Laser_Cutting_Machine -->

    <owl:Class rdf:about="http://www.semanticweb.org/qihan/ontologies/2023/6/untitled-ontology-12#Laser_Cutting_Machine">
        <rdfs:subClassOf rdf:resource="http://www.semanticweb.org/qihan/ontologies/2023/6/untitled-ontology-12#Cutting_Equipment"/>
        <rdfs:comment>Represents a type of cutting machine that uses a focused laser beam to cut through various materials.</rdfs:comment>
        <rdfs:label>Laser Cutting Machine</rdfs:label>
    </owl:Class>
    


    <!-- http://www.semanticweb.org/qihan/ontologies/2023/6/untitled-ontology-12#Laser_Flash_Apparatus -->

    <owl:Class rdf:about="http://www.semanticweb.org/qihan/ontologies/2023/6/untitled-ontology-12#Laser_Flash_Apparatus">
        <rdfs:subClassOf rdf:resource="http://www.semanticweb.org/qihan/ontologies/2023/6/untitled-ontology-12#Thermal_Conductivity_Measurement_Apparatus"/>
        <rdfs:comment>Represents a specialized apparatus used to measure the thermal diffusivity and specific heat of materials.</rdfs:comment>
        <rdfs:label>Laser Flash Apparatus</rdfs:label>
    </owl:Class>
    


    <!-- http://www.semanticweb.org/qihan/ontologies/2023/6/untitled-ontology-12#Lateral_Displacement -->

    <owl:Class rdf:about="http://www.semanticweb.org/qihan/ontologies/2023/6/untitled-ontology-12#Lateral_Displacement">
        <rdfs:subClassOf rdf:resource="http://www.semanticweb.org/qihan/ontologies/2023/6/untitled-ontology-12#Displacement"/>
        <rdfs:comment>Represents the displacement or movement of a material, in a direction perpendicular to the applied force or load.</rdfs:comment>
        <rdfs:label>Lateral Displacement</rdfs:label>
    </owl:Class>
    


    <!-- http://www.semanticweb.org/qihan/ontologies/2023/6/untitled-ontology-12#Lateral_Strain -->

    <owl:Class rdf:about="http://www.semanticweb.org/qihan/ontologies/2023/6/untitled-ontology-12#Lateral_Strain">
        <rdfs:subClassOf rdf:resource="http://www.semanticweb.org/qihan/ontologies/2023/6/untitled-ontology-12#Strain"/>
        <rdfs:comment>Represents the change in width or deformation perpendicular to the longitudinal axis of a material under an applied load.</rdfs:comment>
        <rdfs:label>Lateral Strain</rdfs:label>
    </owl:Class>
    


    <!-- http://www.semanticweb.org/qihan/ontologies/2023/6/untitled-ontology-12#Lathe -->

    <owl:Class rdf:about="http://www.semanticweb.org/qihan/ontologies/2023/6/untitled-ontology-12#Lathe">
        <rdfs:subClassOf rdf:resource="http://www.semanticweb.org/qihan/ontologies/2023/6/untitled-ontology-12#Machining_Equipment"/>
        <rdfs:comment>Represents a type of machining equipment used for turning operations to create cylindrical shapes on workpieces.</rdfs:comment>
        <rdfs:label>Lathe</rdfs:label>
    </owl:Class>
    


    <!-- http://www.semanticweb.org/qihan/ontologies/2023/6/untitled-ontology-12#Layup_Processes -->

    <owl:Class rdf:about="http://www.semanticweb.org/qihan/ontologies/2023/6/untitled-ontology-12#Layup_Processes">
        <rdfs:subClassOf rdf:resource="http://www.semanticweb.org/qihan/ontologies/2023/6/untitled-ontology-12#Material_Manufacturing"/>
        <rdfs:comment>Represents a category of manufacturing processes used to build composite structures by laying up layers of reinforcing fibers and resin to form a laminate.</rdfs:comment>
        <rdfs:label>Layup Processes</rdfs:label>
    </owl:Class>
    


    <!-- http://www.semanticweb.org/qihan/ontologies/2023/6/untitled-ontology-12#Lignin-based_Composite -->

    <owl:Class rdf:about="http://www.semanticweb.org/qihan/ontologies/2023/6/untitled-ontology-12#Lignin-based_Composite">
        <rdfs:subClassOf rdf:resource="http://www.semanticweb.org/qihan/ontologies/2023/6/untitled-ontology-12#Bio-based_Composite"/>
    </owl:Class>
    


    <!-- http://www.semanticweb.org/qihan/ontologies/2023/6/untitled-ontology-12#Load -->

    <owl:Class rdf:about="http://www.semanticweb.org/qihan/ontologies/2023/6/untitled-ontology-12#Load">
        <rdfs:subClassOf rdf:resource="http://www.semanticweb.org/qihan/ontologies/2023/6/untitled-ontology-12#Test_Parameter"/>
        <rdfs:comment>Represents the force or weight applied to a material.</rdfs:comment>
        <rdfs:label>Load</rdfs:label>
    </owl:Class>
    


    <!-- http://www.semanticweb.org/qihan/ontologies/2023/6/untitled-ontology-12#Loading_Rate -->

    <owl:Class rdf:about="http://www.semanticweb.org/qihan/ontologies/2023/6/untitled-ontology-12#Loading_Rate">
        <rdfs:subClassOf rdf:resource="http://www.semanticweb.org/qihan/ontologies/2023/6/untitled-ontology-12#Time"/>
        <rdfs:comment>Represents the rate at which an external load or stress is applied to a material during test.</rdfs:comment>
        <rdfs:label>Loading Rate</rdfs:label>
    </owl:Class>
    


    <!-- http://www.semanticweb.org/qihan/ontologies/2023/6/untitled-ontology-12#Long_Fiber_Reinforced_Composite -->

    <owl:Class rdf:about="http://www.semanticweb.org/qihan/ontologies/2023/6/untitled-ontology-12#Long_Fiber_Reinforced_Composite">
        <rdfs:subClassOf rdf:resource="http://www.semanticweb.org/qihan/ontologies/2023/6/untitled-ontology-12#Discontinuous_Fiber_Composite"/>
    </owl:Class>
    


    <!-- http://www.semanticweb.org/qihan/ontologies/2023/6/untitled-ontology-12#Longitudinal_Orientation -->

    <owl:Class rdf:about="http://www.semanticweb.org/qihan/ontologies/2023/6/untitled-ontology-12#Longitudinal_Orientation">
        <rdfs:subClassOf rdf:resource="http://www.semanticweb.org/qihan/ontologies/2023/6/untitled-ontology-12#Orientation"/>
        <rdfs:comment>Represents the orientation of a material along its longitudinal axis.</rdfs:comment>
        <rdfs:label>Longitudinal Orientation</rdfs:label>
    </owl:Class>
    


    <!-- http://www.semanticweb.org/qihan/ontologies/2023/6/untitled-ontology-12#Loss_Factor -->

    <owl:Class rdf:about="http://www.semanticweb.org/qihan/ontologies/2023/6/untitled-ontology-12#Loss_Factor">
        <rdfs:subClassOf rdf:resource="http://www.semanticweb.org/qihan/ontologies/2023/6/untitled-ontology-12#Damping_Capacity"/>
    </owl:Class>
    


    <!-- http://www.semanticweb.org/qihan/ontologies/2023/6/untitled-ontology-12#MIL-STD-461 -->

    <owl:Class rdf:about="http://www.semanticweb.org/qihan/ontologies/2023/6/untitled-ontology-12#MIL-STD-461">
        <rdfs:subClassOf rdf:resource="http://www.semanticweb.org/qihan/ontologies/2023/6/untitled-ontology-12#MIL_Standards"/>
        <rdfs:comment>Requirements for the Control of Electromagnetic Interference Characteristics of Subsystems and Equipment</rdfs:comment>
        <rdfs:label>MIL STD 461</rdfs:label>
    </owl:Class>
    


    <!-- http://www.semanticweb.org/qihan/ontologies/2023/6/untitled-ontology-12#MIL-STD-810 -->

    <owl:Class rdf:about="http://www.semanticweb.org/qihan/ontologies/2023/6/untitled-ontology-12#MIL-STD-810">
        <rdfs:subClassOf rdf:resource="http://www.semanticweb.org/qihan/ontologies/2023/6/untitled-ontology-12#MIL_Standards"/>
        <rdfs:comment>Environmental Engineering Considerations and Laboratory Tests</rdfs:comment>
        <rdfs:label>MIL STD 810</rdfs:label>
    </owl:Class>
    


    <!-- http://www.semanticweb.org/qihan/ontologies/2023/6/untitled-ontology-12#MIL-STD-883 -->

    <owl:Class rdf:about="http://www.semanticweb.org/qihan/ontologies/2023/6/untitled-ontology-12#MIL-STD-883">
        <rdfs:subClassOf rdf:resource="http://www.semanticweb.org/qihan/ontologies/2023/6/untitled-ontology-12#MIL_Standards"/>
        <rdfs:comment>Test Methods and Procedures for Microelectronics</rdfs:comment>
        <rdfs:label>MIL STD 883</rdfs:label>
    </owl:Class>
    


    <!-- http://www.semanticweb.org/qihan/ontologies/2023/6/untitled-ontology-12#MIL_Standards -->

    <owl:Class rdf:about="http://www.semanticweb.org/qihan/ontologies/2023/6/untitled-ontology-12#MIL_Standards">
        <rdfs:subClassOf rdf:resource="http://www.semanticweb.org/qihan/ontologies/2023/6/untitled-ontology-12#Test_Standards"/>
        <rdfs:label>Military Standards (MIL)</rdfs:label>
    </owl:Class>
    


    <!-- http://www.semanticweb.org/qihan/ontologies/2023/6/untitled-ontology-12#Machining_Equipment -->

    <owl:Class rdf:about="http://www.semanticweb.org/qihan/ontologies/2023/6/untitled-ontology-12#Machining_Equipment">
        <rdfs:subClassOf rdf:resource="http://www.semanticweb.org/qihan/ontologies/2023/6/untitled-ontology-12#Specimen_Preparation_Equipment"/>
        <rdfs:comment>Represents equipment used for machining composite materials to prepare test specimens with specific geometries and dimensions</rdfs:comment>
        <rdfs:label>Machining Equipment</rdfs:label>
    </owl:Class>
    


    <!-- http://www.semanticweb.org/qihan/ontologies/2023/6/untitled-ontology-12#Magnesium_Matrix_Composite -->

    <owl:Class rdf:about="http://www.semanticweb.org/qihan/ontologies/2023/6/untitled-ontology-12#Magnesium_Matrix_Composite">
        <rdfs:subClassOf rdf:resource="http://www.semanticweb.org/qihan/ontologies/2023/6/untitled-ontology-12#Metal_Matrix_Composite"/>
    </owl:Class>
    


    <!-- http://www.semanticweb.org/qihan/ontologies/2023/6/untitled-ontology-12#Magnetic_Field -->

    <owl:Class rdf:about="http://www.semanticweb.org/qihan/ontologies/2023/6/untitled-ontology-12#Magnetic_Field">
        <rdfs:subClassOf rdf:resource="http://www.semanticweb.org/qihan/ontologies/2023/6/untitled-ontology-12#Test_Parameter"/>
        <rdfs:comment>Represents a physical quantity that describes the intensity and direction of a magnetic force experienced by magnetic materials.</rdfs:comment>
        <rdfs:label>Magnetic Field</rdfs:label>
    </owl:Class>
    


    <!-- http://www.semanticweb.org/qihan/ontologies/2023/6/untitled-ontology-12#Magnetic_Flux_Density -->

    <owl:Class rdf:about="http://www.semanticweb.org/qihan/ontologies/2023/6/untitled-ontology-12#Magnetic_Flux_Density">
        <rdfs:subClassOf rdf:resource="http://www.semanticweb.org/qihan/ontologies/2023/6/untitled-ontology-12#Magnetic_Field"/>
        <rdfs:comment>Represents the measure of magnetic field strength or magnetic flux per unit area of a material.</rdfs:comment>
        <rdfs:label>Magnetic Flux Density</rdfs:label>
    </owl:Class>
    


    <!-- http://www.semanticweb.org/qihan/ontologies/2023/6/untitled-ontology-12#Material -->

    <owl:Class rdf:about="http://www.semanticweb.org/qihan/ontologies/2023/6/untitled-ontology-12#Material"/>
    


    <!-- http://www.semanticweb.org/qihan/ontologies/2023/6/untitled-ontology-12#Material_Manufacturing -->

    <owl:Class rdf:about="http://www.semanticweb.org/qihan/ontologies/2023/6/untitled-ontology-12#Material_Manufacturing">
        <rdfs:subClassOf rdf:resource="http://www.semanticweb.org/qihan/ontologies/2023/6/untitled-ontology-12#Pre-Testing_Phase"/>
        <rdfs:comment>Represents the process of producing or fabricating composite materials and other types of materials.</rdfs:comment>
        <rdfs:label>Material Manufacturing</rdfs:label>
    </owl:Class>
    


    <!-- http://www.semanticweb.org/qihan/ontologies/2023/6/untitled-ontology-12#Material_Preparation -->

    <owl:Class rdf:about="http://www.semanticweb.org/qihan/ontologies/2023/6/untitled-ontology-12#Material_Preparation">
        <rdfs:subClassOf rdf:resource="http://www.semanticweb.org/qihan/ontologies/2023/6/untitled-ontology-12#Pre-Testing_Phase"/>
        <rdfs:subClassOf>
            <owl:Restriction>
                <owl:onProperty rdf:resource="http://www.semanticweb.org/qihan/ontologies/2023/6/untitled-ontology-12#hasPart"/>
                <owl:someValuesFrom rdf:resource="http://www.semanticweb.org/qihan/ontologies/2023/6/untitled-ontology-12#Material_Preparation"/>
            </owl:Restriction>
        </rdfs:subClassOf>
    </owl:Class>
    


    <!-- http://www.semanticweb.org/qihan/ontologies/2023/6/untitled-ontology-12#Mechanical_Power -->

    <owl:Class rdf:about="http://www.semanticweb.org/qihan/ontologies/2023/6/untitled-ontology-12#Mechanical_Power">
        <rdfs:subClassOf rdf:resource="http://www.semanticweb.org/qihan/ontologies/2023/6/untitled-ontology-12#Power"/>
        <rdfs:comment>Represents the amount of mechanical energy consumed, generated, or transferred by a system.</rdfs:comment>
        <rdfs:label>Mechanical Power</rdfs:label>
    </owl:Class>
    


    <!-- http://www.semanticweb.org/qihan/ontologies/2023/6/untitled-ontology-12#Medium -->

    <owl:Class rdf:about="http://www.semanticweb.org/qihan/ontologies/2023/6/untitled-ontology-12#Medium">
        <rdfs:subClassOf rdf:resource="http://www.semanticweb.org/qihan/ontologies/2023/6/untitled-ontology-12#Test_Environment"/>
        <rdfs:comment>Represents the medium or environment in which the mechanical testing of composite material specimens takes place.</rdfs:comment>
        <rdfs:label>Medium</rdfs:label>
    </owl:Class>
    


    <!-- http://www.semanticweb.org/qihan/ontologies/2023/6/untitled-ontology-12#Metal-Ceramic_Functionally_Graded_Composite -->

    <owl:Class rdf:about="http://www.semanticweb.org/qihan/ontologies/2023/6/untitled-ontology-12#Metal-Ceramic_Functionally_Graded_Composite">
        <rdfs:subClassOf rdf:resource="http://www.semanticweb.org/qihan/ontologies/2023/6/untitled-ontology-12#Functionally_Graded_Composite"/>
    </owl:Class>
    


    <!-- http://www.semanticweb.org/qihan/ontologies/2023/6/untitled-ontology-12#Metal-Polymer_Functionally_Graded_Composite -->

    <owl:Class rdf:about="http://www.semanticweb.org/qihan/ontologies/2023/6/untitled-ontology-12#Metal-Polymer_Functionally_Graded_Composite">
        <rdfs:subClassOf rdf:resource="http://www.semanticweb.org/qihan/ontologies/2023/6/untitled-ontology-12#Functionally_Graded_Composite"/>
    </owl:Class>
    


    <!-- http://www.semanticweb.org/qihan/ontologies/2023/6/untitled-ontology-12#Metal_Matrix_Composite -->

    <owl:Class rdf:about="http://www.semanticweb.org/qihan/ontologies/2023/6/untitled-ontology-12#Metal_Matrix_Composite">
        <rdfs:subClassOf rdf:resource="http://www.semanticweb.org/qihan/ontologies/2023/6/untitled-ontology-12#Composite_Material"/>
    </owl:Class>
    


    <!-- http://www.semanticweb.org/qihan/ontologies/2023/6/untitled-ontology-12#Metal_Nanocomposite -->

    <owl:Class rdf:about="http://www.semanticweb.org/qihan/ontologies/2023/6/untitled-ontology-12#Metal_Nanocomposite">
        <rdfs:subClassOf rdf:resource="http://www.semanticweb.org/qihan/ontologies/2023/6/untitled-ontology-12#Nanocomposite"/>
    </owl:Class>
    


    <!-- http://www.semanticweb.org/qihan/ontologies/2023/6/untitled-ontology-12#Microcapsule-based_Self-healing_Composite -->

    <owl:Class rdf:about="http://www.semanticweb.org/qihan/ontologies/2023/6/untitled-ontology-12#Microcapsule-based_Self-healing_Composite">
        <rdfs:subClassOf rdf:resource="http://www.semanticweb.org/qihan/ontologies/2023/6/untitled-ontology-12#Self-healing_Composite"/>
    </owl:Class>
    


    <!-- http://www.semanticweb.org/qihan/ontologies/2023/6/untitled-ontology-12#Microchannel-based_Self-healing_Composite -->

    <owl:Class rdf:about="http://www.semanticweb.org/qihan/ontologies/2023/6/untitled-ontology-12#Microchannel-based_Self-healing_Composite">
        <rdfs:subClassOf rdf:resource="http://www.semanticweb.org/qihan/ontologies/2023/6/untitled-ontology-12#Self-healing_Composite"/>
    </owl:Class>
    


    <!-- http://www.semanticweb.org/qihan/ontologies/2023/6/untitled-ontology-12#Microscope -->

    <owl:Class rdf:about="http://www.semanticweb.org/qihan/ontologies/2023/6/untitled-ontology-12#Microscope">
        <rdfs:subClassOf rdf:resource="http://www.semanticweb.org/qihan/ontologies/2023/6/untitled-ontology-12#Test_Equipment"/>
        <rdfs:comment>Represents a laboratory instrument used to examine and analyze composite material specimens at a microscopic level.</rdfs:comment>
        <rdfs:label>Microscope</rdfs:label>
    </owl:Class>
    


    <!-- http://www.semanticweb.org/qihan/ontologies/2023/6/untitled-ontology-12#Microvascular_Network-based_Self-healing_Composite -->

    <owl:Class rdf:about="http://www.semanticweb.org/qihan/ontologies/2023/6/untitled-ontology-12#Microvascular_Network-based_Self-healing_Composite">
        <rdfs:subClassOf rdf:resource="http://www.semanticweb.org/qihan/ontologies/2023/6/untitled-ontology-12#Self-healing_Composite"/>
    </owl:Class>
    


    <!-- http://www.semanticweb.org/qihan/ontologies/2023/6/untitled-ontology-12#Moisture_Absorption -->

    <owl:Class rdf:about="http://www.semanticweb.org/qihan/ontologies/2023/6/untitled-ontology-12#Moisture_Absorption">
        <rdfs:subClassOf rdf:resource="http://www.semanticweb.org/qihan/ontologies/2023/6/untitled-ontology-12#Moisture_Content"/>
        <rdfs:comment>Represents the process of a material absorbing moisture or water from its surroundings.</rdfs:comment>
        <rdfs:label>Moisture Absorption</rdfs:label>
    </owl:Class>
    


    <!-- http://www.semanticweb.org/qihan/ontologies/2023/6/untitled-ontology-12#Moisture_Content -->

    <owl:Class rdf:about="http://www.semanticweb.org/qihan/ontologies/2023/6/untitled-ontology-12#Moisture_Content">
        <rdfs:subClassOf rdf:resource="http://www.semanticweb.org/qihan/ontologies/2023/6/untitled-ontology-12#Test_Parameter"/>
        <rdfs:comment>Represents the amount of water or moisture present in a material.</rdfs:comment>
        <rdfs:label>Moisture Content</rdfs:label>
    </owl:Class>
    


    <!-- http://www.semanticweb.org/qihan/ontologies/2023/6/untitled-ontology-12#Moisture_Expansion_Coefficient -->

    <owl:Class rdf:about="http://www.semanticweb.org/qihan/ontologies/2023/6/untitled-ontology-12#Moisture_Expansion_Coefficient">
        <rdfs:subClassOf rdf:resource="http://www.semanticweb.org/qihan/ontologies/2023/6/untitled-ontology-12#Dimensional_Changes"/>
    </owl:Class>
    


    <!-- http://www.semanticweb.org/qihan/ontologies/2023/6/untitled-ontology-12#Molding_Machine -->

    <owl:Class rdf:about="http://www.semanticweb.org/qihan/ontologies/2023/6/untitled-ontology-12#Molding_Machine">
        <rdfs:subClassOf rdf:resource="http://www.semanticweb.org/qihan/ontologies/2023/6/untitled-ontology-12#Specimen_Preparation_Equipment"/>
        <rdfs:comment>Represents a general category of machines used in the manufacturing process to shape materials into specific forms and sizes.</rdfs:comment>
        <rdfs:label>Molding Machine</rdfs:label>
    </owl:Class>
    


    <!-- http://www.semanticweb.org/qihan/ontologies/2023/6/untitled-ontology-12#Mullite_Matrix_Composite -->

    <owl:Class rdf:about="http://www.semanticweb.org/qihan/ontologies/2023/6/untitled-ontology-12#Mullite_Matrix_Composite">
        <rdfs:subClassOf rdf:resource="http://www.semanticweb.org/qihan/ontologies/2023/6/untitled-ontology-12#Ceramic_Matrix_Composite"/>
    </owl:Class>
    


    <!-- http://www.semanticweb.org/qihan/ontologies/2023/6/untitled-ontology-12#NIST_SP_800-22 -->

    <owl:Class rdf:about="http://www.semanticweb.org/qihan/ontologies/2023/6/untitled-ontology-12#NIST_SP_800-22">
        <rdfs:subClassOf rdf:resource="http://www.semanticweb.org/qihan/ontologies/2023/6/untitled-ontology-12#NIST_Standards"/>
        <rdfs:comment>A Statistical Test Suite for Random and Pseudorandom Number Generators</rdfs:comment>
        <rdfs:label>NIST SP 800-22</rdfs:label>
    </owl:Class>
    


    <!-- http://www.semanticweb.org/qihan/ontologies/2023/6/untitled-ontology-12#NIST_SP_800-53 -->

    <owl:Class rdf:about="http://www.semanticweb.org/qihan/ontologies/2023/6/untitled-ontology-12#NIST_SP_800-53">
        <rdfs:subClassOf rdf:resource="http://www.semanticweb.org/qihan/ontologies/2023/6/untitled-ontology-12#NIST_Standards"/>
        <rdfs:comment>Security and Privacy Controls for Federal Information Systems and Organizations</rdfs:comment>
        <rdfs:label>NIST SP 8000-53</rdfs:label>
    </owl:Class>
    


    <!-- http://www.semanticweb.org/qihan/ontologies/2023/6/untitled-ontology-12#NIST_SP_800-61 -->

    <owl:Class rdf:about="http://www.semanticweb.org/qihan/ontologies/2023/6/untitled-ontology-12#NIST_SP_800-61">
        <rdfs:subClassOf rdf:resource="http://www.semanticweb.org/qihan/ontologies/2023/6/untitled-ontology-12#NIST_Standards"/>
        <rdfs:comment>Computer Security Incident Handling Guide</rdfs:comment>
        <rdfs:label>NIST SP 800-61</rdfs:label>
    </owl:Class>
    


    <!-- http://www.semanticweb.org/qihan/ontologies/2023/6/untitled-ontology-12#NIST_Standards -->

    <owl:Class rdf:about="http://www.semanticweb.org/qihan/ontologies/2023/6/untitled-ontology-12#NIST_Standards">
        <rdfs:subClassOf rdf:resource="http://www.semanticweb.org/qihan/ontologies/2023/6/untitled-ontology-12#Test_Standards"/>
        <rdfs:label>National Institute of Standards and Technology (NIST)</rdfs:label>
    </owl:Class>
    


    <!-- http://www.semanticweb.org/qihan/ontologies/2023/6/untitled-ontology-12#Nanocomposite -->

    <owl:Class rdf:about="http://www.semanticweb.org/qihan/ontologies/2023/6/untitled-ontology-12#Nanocomposite">
        <rdfs:subClassOf rdf:resource="http://www.semanticweb.org/qihan/ontologies/2023/6/untitled-ontology-12#Composite_Material"/>
    </owl:Class>
    


    <!-- http://www.semanticweb.org/qihan/ontologies/2023/6/untitled-ontology-12#Nanocomposite_Synthesis -->

    <owl:Class rdf:about="http://www.semanticweb.org/qihan/ontologies/2023/6/untitled-ontology-12#Nanocomposite_Synthesis">
        <rdfs:subClassOf rdf:resource="http://www.semanticweb.org/qihan/ontologies/2023/6/untitled-ontology-12#Material_Manufacturing"/>
        <rdfs:comment>Represents the process of producing nanocomposite materials, which are composites containing nanoparticles or nanofillers dispersed within the matrix material.</rdfs:comment>
        <rdfs:label>Nanocomposite Synthesis</rdfs:label>
    </owl:Class>
    


    <!-- http://www.semanticweb.org/qihan/ontologies/2023/6/untitled-ontology-12#Nanofiber_and_Nanoparticle_Coating -->

    <owl:Class rdf:about="http://www.semanticweb.org/qihan/ontologies/2023/6/untitled-ontology-12#Nanofiber_and_Nanoparticle_Coating">
        <rdfs:subClassOf rdf:resource="http://www.semanticweb.org/qihan/ontologies/2023/6/untitled-ontology-12#Material_Manufacturing"/>
        <rdfs:comment>Represents the process of applying nanofibers or nanoparticles onto the surface of a substrate or base material to create a thin and uniform coating.</rdfs:comment>
        <rdfs:label>Nanofiber and Nanoparticle Coating</rdfs:label>
    </owl:Class>
    


    <!-- http://www.semanticweb.org/qihan/ontologies/2023/6/untitled-ontology-12#Natural_Fiber_Composite -->

    <owl:Class rdf:about="http://www.semanticweb.org/qihan/ontologies/2023/6/untitled-ontology-12#Natural_Fiber_Composite">
        <rdfs:subClassOf rdf:resource="http://www.semanticweb.org/qihan/ontologies/2023/6/untitled-ontology-12#Composite_Material"/>
    </owl:Class>
    


    <!-- http://www.semanticweb.org/qihan/ontologies/2023/6/untitled-ontology-12#Natural_Fibre_Reinforces_Polymer -->

    <owl:Class rdf:about="http://www.semanticweb.org/qihan/ontologies/2023/6/untitled-ontology-12#Natural_Fibre_Reinforces_Polymer">
        <rdfs:subClassOf rdf:resource="http://www.semanticweb.org/qihan/ontologies/2023/6/untitled-ontology-12#Polymer_Matrix_Composite"/>
    </owl:Class>
    


    <!-- http://www.semanticweb.org/qihan/ontologies/2023/6/untitled-ontology-12#Nomex_Core_Composite -->

    <owl:Class rdf:about="http://www.semanticweb.org/qihan/ontologies/2023/6/untitled-ontology-12#Nomex_Core_Composite">
        <rdfs:subClassOf rdf:resource="http://www.semanticweb.org/qihan/ontologies/2023/6/untitled-ontology-12#Sandwich_Composite"/>
    </owl:Class>
    


    <!-- http://www.semanticweb.org/qihan/ontologies/2023/6/untitled-ontology-12#Non-Contact_Extensometer -->

    <owl:Class rdf:about="http://www.semanticweb.org/qihan/ontologies/2023/6/untitled-ontology-12#Non-Contact_Extensometer">
        <rdfs:subClassOf rdf:resource="http://www.semanticweb.org/qihan/ontologies/2023/6/untitled-ontology-12#Extensometer"/>
        <rdfs:comment>Represents a type of extensometer used to measure the deformation or strain of composite material specimens by making physical contact with the specimen surface.</rdfs:comment>
        <rdfs:label>Non-Contact Extensometer</rdfs:label>
    </owl:Class>
    


    <!-- http://www.semanticweb.org/qihan/ontologies/2023/6/untitled-ontology-12#Off-axis_Orientation -->

    <owl:Class rdf:about="http://www.semanticweb.org/qihan/ontologies/2023/6/untitled-ontology-12#Off-axis_Orientation">
        <rdfs:subClassOf rdf:resource="http://www.semanticweb.org/qihan/ontologies/2023/6/untitled-ontology-12#Orientation"/>
        <rdfs:comment>Represents the orientation of a material at an angle other than the primary axis or longitudinal direction.</rdfs:comment>
        <rdfs:label>Off-Axis Orientation</rdfs:label>
    </owl:Class>
    


    <!-- http://www.semanticweb.org/qihan/ontologies/2023/6/untitled-ontology-12#Open_Molding_Compression_Molding -->

    <owl:Class rdf:about="http://www.semanticweb.org/qihan/ontologies/2023/6/untitled-ontology-12#Open_Molding_Compression_Molding">
        <rdfs:subClassOf rdf:resource="http://www.semanticweb.org/qihan/ontologies/2023/6/untitled-ontology-12#Compression_Molding_Processes"/>
        <rdfs:comment>Represents a specific type of compression molding process where the composite material is placed into an open mold cavity.</rdfs:comment>
        <rdfs:label>Open Molding Compression Molding</rdfs:label>
    </owl:Class>
    


    <!-- http://www.semanticweb.org/qihan/ontologies/2023/6/untitled-ontology-12#Optical_Microscope -->

    <owl:Class rdf:about="http://www.semanticweb.org/qihan/ontologies/2023/6/untitled-ontology-12#Optical_Microscope">
        <rdfs:subClassOf rdf:resource="http://www.semanticweb.org/qihan/ontologies/2023/6/untitled-ontology-12#Microscope"/>
        <rdfs:comment>Represents a type of microscope that uses visible light to magnify and examine the surface and internal structures of composite material specimens.</rdfs:comment>
        <rdfs:label>Optical Microscope</rdfs:label>
    </owl:Class>
    


    <!-- http://www.semanticweb.org/qihan/ontologies/2023/6/untitled-ontology-12#Optical_Properties -->

    <owl:Class rdf:about="http://www.semanticweb.org/qihan/ontologies/2023/6/untitled-ontology-12#Optical_Properties">
        <rdfs:subClassOf rdf:resource="http://www.semanticweb.org/qihan/ontologies/2023/6/untitled-ontology-12#Result_Calculation"/>
    </owl:Class>
    


    <!-- http://www.semanticweb.org/qihan/ontologies/2023/6/untitled-ontology-12#Orientation -->

    <owl:Class rdf:about="http://www.semanticweb.org/qihan/ontologies/2023/6/untitled-ontology-12#Orientation">
        <rdfs:subClassOf rdf:resource="http://www.semanticweb.org/qihan/ontologies/2023/6/untitled-ontology-12#Test_Parameter"/>
        <rdfs:comment>Represents the specific direction or alignment of fibers or particles within a composite material specimen.</rdfs:comment>
        <rdfs:label>Orientation</rdfs:label>
    </owl:Class>
    


    <!-- http://www.semanticweb.org/qihan/ontologies/2023/6/untitled-ontology-12#Oscillating_Abrasion_Tester -->

    <owl:Class rdf:about="http://www.semanticweb.org/qihan/ontologies/2023/6/untitled-ontology-12#Oscillating_Abrasion_Tester">
        <rdfs:subClassOf rdf:resource="http://www.semanticweb.org/qihan/ontologies/2023/6/untitled-ontology-12#Abrasion_Testing_Machine"/>
        <rdfs:comment>Represents a specific type of test equipment used to evaluate the abrasion resistance of composite material specimens by subjecting them to oscillating or reciprocating rubbing motions against an abrasive surface.</rdfs:comment>
        <rdfs:label>Oscillating Abrasion Tester</rdfs:label>
    </owl:Class>
    


    <!-- http://www.semanticweb.org/qihan/ontologies/2023/6/untitled-ontology-12#Oscillatory_Rheometer -->

    <owl:Class rdf:about="http://www.semanticweb.org/qihan/ontologies/2023/6/untitled-ontology-12#Oscillatory_Rheometer">
        <rdfs:subClassOf rdf:resource="http://www.semanticweb.org/qihan/ontologies/2023/6/untitled-ontology-12#Rheometer"/>
        <rdfs:comment>Represents a specific type of rheometer used to characterize the viscoelastic properties of materials.</rdfs:comment>
        <rdfs:label>Oscillatory Rheometer</rdfs:label>
    </owl:Class>
    


    <!-- http://www.semanticweb.org/qihan/ontologies/2023/6/untitled-ontology-12#Out-of-Autoclave_Curing_Processes -->

    <owl:Class rdf:about="http://www.semanticweb.org/qihan/ontologies/2023/6/untitled-ontology-12#Out-of-Autoclave_Curing_Processes">
        <rdfs:subClassOf rdf:resource="http://www.semanticweb.org/qihan/ontologies/2023/6/untitled-ontology-12#Material_Manufacturing"/>
        <rdfs:comment>Represents a category of composite curing processes that do not involve the use of an autoclave.</rdfs:comment>
        <rdfs:label>Out of Autoclave Curing Processes</rdfs:label>
    </owl:Class>
    


    <!-- http://www.semanticweb.org/qihan/ontologies/2023/6/untitled-ontology-12#Parallel_Orientation -->

    <owl:Class rdf:about="http://www.semanticweb.org/qihan/ontologies/2023/6/untitled-ontology-12#Parallel_Orientation">
        <rdfs:subClassOf rdf:resource="http://www.semanticweb.org/qihan/ontologies/2023/6/untitled-ontology-12#Orientation"/>
        <rdfs:comment>Represents the orientation of a material aligned parallel to a specific reference direction or axis.</rdfs:comment>
        <rdfs:label>Parallel Orientation</rdfs:label>
    </owl:Class>
    


    <!-- http://www.semanticweb.org/qihan/ontologies/2023/6/untitled-ontology-12#Peel_Strength -->

    <owl:Class rdf:about="http://www.semanticweb.org/qihan/ontologies/2023/6/untitled-ontology-12#Peel_Strength">
        <rdfs:subClassOf rdf:resource="http://www.semanticweb.org/qihan/ontologies/2023/6/untitled-ontology-12#Adhesive_Strength"/>
    </owl:Class>
    


    <!-- http://www.semanticweb.org/qihan/ontologies/2023/6/untitled-ontology-12#Peel_Testing -->

    <owl:Class rdf:about="http://www.semanticweb.org/qihan/ontologies/2023/6/untitled-ontology-12#Peel_Testing">
        <rdfs:subClassOf rdf:resource="http://www.semanticweb.org/qihan/ontologies/2023/6/untitled-ontology-12#Testing_Method"/>
        <rdfs:comment>Represents a type of mechanical testing used to evaluate the bond strength or adhesion of materials, by measuring the force required to separate two bonded surfaces.</rdfs:comment>
        <rdfs:label>Peel Testing</rdfs:label>
    </owl:Class>
    


    <!-- http://www.semanticweb.org/qihan/ontologies/2023/6/untitled-ontology-12#Perpendicular_Orientation -->

    <owl:Class rdf:about="http://www.semanticweb.org/qihan/ontologies/2023/6/untitled-ontology-12#Perpendicular_Orientation">
        <rdfs:subClassOf rdf:resource="http://www.semanticweb.org/qihan/ontologies/2023/6/untitled-ontology-12#Orientation"/>
        <rdfs:comment>Represents the orientation of a material aligned perpendicular to a specific reference direction or axis.</rdfs:comment>
        <rdfs:label>Perpendicular Orientation</rdfs:label>
    </owl:Class>
    


    <!-- http://www.semanticweb.org/qihan/ontologies/2023/6/untitled-ontology-12#Polishing_Cloth -->

    <owl:Class rdf:about="http://www.semanticweb.org/qihan/ontologies/2023/6/untitled-ontology-12#Polishing_Cloth">
        <rdfs:subClassOf rdf:resource="http://www.semanticweb.org/qihan/ontologies/2023/6/untitled-ontology-12#Polishing_Equipment"/>
        <rdfs:comment>Represents a type of soft and absorbent cloth used for applying polishing compounds and buffing materials to the surface of a material during the polishing process.</rdfs:comment>
        <rdfs:label>Polishing Cloth</rdfs:label>
    </owl:Class>
    


    <!-- http://www.semanticweb.org/qihan/ontologies/2023/6/untitled-ontology-12#Polishing_Equipment -->

    <owl:Class rdf:about="http://www.semanticweb.org/qihan/ontologies/2023/6/untitled-ontology-12#Polishing_Equipment">
        <rdfs:subClassOf rdf:resource="http://www.semanticweb.org/qihan/ontologies/2023/6/untitled-ontology-12#Specimen_Preparation_Equipment"/>
        <rdfs:comment>Represents a general category of tools and machines used for the process of polishing, which involves smoothing and refining the surface of a material to achieve a shiny and smooth finish.</rdfs:comment>
        <rdfs:label>Polishing Equipment</rdfs:label>
    </owl:Class>
    


    <!-- http://www.semanticweb.org/qihan/ontologies/2023/6/untitled-ontology-12#Polishing_Machine -->

    <owl:Class rdf:about="http://www.semanticweb.org/qihan/ontologies/2023/6/untitled-ontology-12#Polishing_Machine">
        <rdfs:subClassOf rdf:resource="http://www.semanticweb.org/qihan/ontologies/2023/6/untitled-ontology-12#Polishing_Equipment"/>
        <rdfs:comment>Represents a type of machine designed to automate the polishing process for achieving consistent and efficient results.</rdfs:comment>
        <rdfs:label>Polishing Machine</rdfs:label>
    </owl:Class>
    


    <!-- http://www.semanticweb.org/qihan/ontologies/2023/6/untitled-ontology-12#Polishing_Wheel -->

    <owl:Class rdf:about="http://www.semanticweb.org/qihan/ontologies/2023/6/untitled-ontology-12#Polishing_Wheel">
        <rdfs:subClassOf rdf:resource="http://www.semanticweb.org/qihan/ontologies/2023/6/untitled-ontology-12#Polishing_Equipment"/>
        <rdfs:comment>Represents a type of rotating wheel made from various materials, such as cloth, felt, or sisal, coated with polishing compounds or abrasives.</rdfs:comment>
        <rdfs:label>Polishing Wheel</rdfs:label>
    </owl:Class>
    


    <!-- http://www.semanticweb.org/qihan/ontologies/2023/6/untitled-ontology-12#Polymer-Metal_Functionally_Graded_Composite -->

    <owl:Class rdf:about="http://www.semanticweb.org/qihan/ontologies/2023/6/untitled-ontology-12#Polymer-Metal_Functionally_Graded_Composite">
        <rdfs:subClassOf rdf:resource="http://www.semanticweb.org/qihan/ontologies/2023/6/untitled-ontology-12#Functionally_Graded_Composite"/>
    </owl:Class>
    


    <!-- http://www.semanticweb.org/qihan/ontologies/2023/6/untitled-ontology-12#Polymer_Matrix_Composite -->

    <owl:Class rdf:about="http://www.semanticweb.org/qihan/ontologies/2023/6/untitled-ontology-12#Polymer_Matrix_Composite">
        <rdfs:subClassOf rdf:resource="http://www.semanticweb.org/qihan/ontologies/2023/6/untitled-ontology-12#Composite_Material"/>
    </owl:Class>
    


    <!-- http://www.semanticweb.org/qihan/ontologies/2023/6/untitled-ontology-12#Polymer_Nanocomposite -->

    <owl:Class rdf:about="http://www.semanticweb.org/qihan/ontologies/2023/6/untitled-ontology-12#Polymer_Nanocomposite">
        <rdfs:subClassOf rdf:resource="http://www.semanticweb.org/qihan/ontologies/2023/6/untitled-ontology-12#Nanocomposite"/>
    </owl:Class>
    


    <!-- http://www.semanticweb.org/qihan/ontologies/2023/6/untitled-ontology-12#Post-Testing_Phase -->

    <owl:Class rdf:about="http://www.semanticweb.org/qihan/ontologies/2023/6/untitled-ontology-12#Post-Testing_Phase"/>
    


    <!-- http://www.semanticweb.org/qihan/ontologies/2023/6/untitled-ontology-12#Power -->

    <owl:Class rdf:about="http://www.semanticweb.org/qihan/ontologies/2023/6/untitled-ontology-12#Power">
        <rdfs:subClassOf rdf:resource="http://www.semanticweb.org/qihan/ontologies/2023/6/untitled-ontology-12#Test_Parameter"/>
        <rdfs:comment>Represents the rate at which work is done or energy is transferred or converted in a material or system.</rdfs:comment>
        <rdfs:label>Power</rdfs:label>
    </owl:Class>
    


    <!-- http://www.semanticweb.org/qihan/ontologies/2023/6/untitled-ontology-12#Pre-Testing_Phase -->

    <owl:Class rdf:about="http://www.semanticweb.org/qihan/ontologies/2023/6/untitled-ontology-12#Pre-Testing_Phase"/>
    


    <!-- http://www.semanticweb.org/qihan/ontologies/2023/6/untitled-ontology-12#Precision_Saw -->

    <owl:Class rdf:about="http://www.semanticweb.org/qihan/ontologies/2023/6/untitled-ontology-12#Precision_Saw">
        <rdfs:subClassOf rdf:resource="http://www.semanticweb.org/qihan/ontologies/2023/6/untitled-ontology-12#Sectioning_Equipment"/>
        <rdfs:comment>Represents a type of cutting tool designed for accurate and controlled sectioning of materials with minimal deformation or damage.</rdfs:comment>
        <rdfs:label>Precision Saw</rdfs:label>
    </owl:Class>
    


    <!-- http://www.semanticweb.org/qihan/ontologies/2023/6/untitled-ontology-12#Prepreg_Autoclave_Curing -->

    <owl:Class rdf:about="http://www.semanticweb.org/qihan/ontologies/2023/6/untitled-ontology-12#Prepreg_Autoclave_Curing">
        <rdfs:subClassOf rdf:resource="http://www.semanticweb.org/qihan/ontologies/2023/6/untitled-ontology-12#Autoclave_Curing_Process"/>
        <rdfs:comment>Represents a specific variant of autoclave curing used to process prepreg materials.</rdfs:comment>
        <rdfs:label>Prepreg Autoclave Curing</rdfs:label>
    </owl:Class>
    


    <!-- http://www.semanticweb.org/qihan/ontologies/2023/6/untitled-ontology-12#Prepreg_Curing -->

    <owl:Class rdf:about="http://www.semanticweb.org/qihan/ontologies/2023/6/untitled-ontology-12#Prepreg_Curing">
        <rdfs:subClassOf rdf:resource="http://www.semanticweb.org/qihan/ontologies/2023/6/untitled-ontology-12#Prepreg_Manufacturing"/>
        <rdfs:comment>Represents the process of fully curing prepreg materials to achieve the final properties of composite structures.</rdfs:comment>
        <rdfs:label>Prepreg Curing</rdfs:label>
    </owl:Class>
    


    <!-- http://www.semanticweb.org/qihan/ontologies/2023/6/untitled-ontology-12#Prepreg_Fabrication -->

    <owl:Class rdf:about="http://www.semanticweb.org/qihan/ontologies/2023/6/untitled-ontology-12#Prepreg_Fabrication">
        <rdfs:subClassOf rdf:resource="http://www.semanticweb.org/qihan/ontologies/2023/6/untitled-ontology-12#Prepreg_Manufacturing"/>
        <rdfs:comment>Represents the process of using prepreg materials to fabricate composite components.</rdfs:comment>
        <rdfs:label>Prepreg Fabrication</rdfs:label>
    </owl:Class>
    


    <!-- http://www.semanticweb.org/qihan/ontologies/2023/6/untitled-ontology-12#Prepreg_Manufacturing -->

    <owl:Class rdf:about="http://www.semanticweb.org/qihan/ontologies/2023/6/untitled-ontology-12#Prepreg_Manufacturing">
        <rdfs:subClassOf rdf:resource="http://www.semanticweb.org/qihan/ontologies/2023/6/untitled-ontology-12#Material_Manufacturing"/>
        <rdfs:comment>Represents the process of producing prepreg materials, which are composite reinforcements pre-impregnated with resin.</rdfs:comment>
        <rdfs:label>Prepreg Manufacturing</rdfs:label>
    </owl:Class>
    


    <!-- http://www.semanticweb.org/qihan/ontologies/2023/6/untitled-ontology-12#Pressure_Condition -->

    <owl:Class rdf:about="http://www.semanticweb.org/qihan/ontologies/2023/6/untitled-ontology-12#Pressure_Condition">
        <rdfs:subClassOf rdf:resource="http://www.semanticweb.org/qihan/ontologies/2023/6/untitled-ontology-12#Test_Environment"/>
        <rdfs:subClassOf rdf:resource="http://www.semanticweb.org/qihan/ontologies/2023/6/untitled-ontology-12#Test_Parameter"/>
        <rdfs:comment>Represents the medium of the testing environment for mechanical testing of composite material specimens. It refers to the state of pressure applied to the specimens during testing, which may include specific levels of compression or tension for particular testing methods.</rdfs:comment>
        <rdfs:label>Pressure Condition</rdfs:label>
    </owl:Class>
    


    <!-- http://www.semanticweb.org/qihan/ontologies/2023/6/untitled-ontology-12#Pultruded_Profile_Manufacturing -->

    <owl:Class rdf:about="http://www.semanticweb.org/qihan/ontologies/2023/6/untitled-ontology-12#Pultruded_Profile_Manufacturing">
        <rdfs:subClassOf rdf:resource="http://www.semanticweb.org/qihan/ontologies/2023/6/untitled-ontology-12#Pultrusion_Process"/>
        <rdfs:comment>Represents the production of composite profiles using the pultrusion process.</rdfs:comment>
        <rdfs:label>Pultruded Profile Manufacturing</rdfs:label>
    </owl:Class>
    


    <!-- http://www.semanticweb.org/qihan/ontologies/2023/6/untitled-ontology-12#Pultrusion_Process -->

    <owl:Class rdf:about="http://www.semanticweb.org/qihan/ontologies/2023/6/untitled-ontology-12#Pultrusion_Process">
        <rdfs:subClassOf rdf:resource="http://www.semanticweb.org/qihan/ontologies/2023/6/untitled-ontology-12#Material_Manufacturing"/>
        <rdfs:comment>Represents a continuous manufacturing process used to produce long and uniform composite profiles with constant cross-sections.</rdfs:comment>
        <rdfs:label>Pultrusion Process</rdfs:label>
    </owl:Class>
    


    <!-- http://www.semanticweb.org/qihan/ontologies/2023/6/untitled-ontology-12#Punch_Shear_Test_Apparatus -->

    <owl:Class rdf:about="http://www.semanticweb.org/qihan/ontologies/2023/6/untitled-ontology-12#Punch_Shear_Test_Apparatus">
        <rdfs:subClassOf rdf:resource="http://www.semanticweb.org/qihan/ontologies/2023/6/untitled-ontology-12#Shear_Testing_Apparatus"/>
        <rdfs:comment>Represents a specialized testing apparatus used to perform the punch shear test on composite material specimens.</rdfs:comment>
        <rdfs:label>Punch Shear Test Apparatus</rdfs:label>
    </owl:Class>
    


    <!-- http://www.semanticweb.org/qihan/ontologies/2023/6/untitled-ontology-12#Quality_Control_Center -->

    <owl:Class rdf:about="http://www.semanticweb.org/qihan/ontologies/2023/6/untitled-ontology-12#Quality_Control_Center">
        <rdfs:subClassOf rdf:resource="http://www.semanticweb.org/qihan/ontologies/2023/6/untitled-ontology-12#Testing_Institution"/>
        <rdfs:comment>Represents a dedicated center or department within a manufacturing company or organization that is responsible for ensuring the quality and consistency of materials and products.</rdfs:comment>
        <rdfs:label>Quality Control Center</rdfs:label>
    </owl:Class>
    


    <!-- http://www.semanticweb.org/qihan/ontologies/2023/6/untitled-ontology-12#Quarter-Bridge_Configuration -->

    <owl:Class rdf:about="http://www.semanticweb.org/qihan/ontologies/2023/6/untitled-ontology-12#Quarter-Bridge_Configuration">
        <rdfs:subClassOf rdf:resource="http://www.semanticweb.org/qihan/ontologies/2023/6/untitled-ontology-12#Strain_Gauge_Configuration"/>
        <rdfs:comment>Represents a configuration of strain gauges or sensors in which only one arm of the Wheatstone bridge circuit is active.</rdfs:comment>
        <rdfs:label>Quarter-Bridge Configuration</rdfs:label>
    </owl:Class>
    


    <!-- http://www.semanticweb.org/qihan/ontologies/2023/6/untitled-ontology-12#Ra -->

    <owl:Class rdf:about="http://www.semanticweb.org/qihan/ontologies/2023/6/untitled-ontology-12#Ra">
        <rdfs:subClassOf rdf:resource="http://www.semanticweb.org/qihan/ontologies/2023/6/untitled-ontology-12#Surface_Roughness"/>
    </owl:Class>
    


    <!-- http://www.semanticweb.org/qihan/ontologies/2023/6/untitled-ontology-12#Radial_Filament_Winding -->

    <owl:Class rdf:about="http://www.semanticweb.org/qihan/ontologies/2023/6/untitled-ontology-12#Radial_Filament_Winding">
        <rdfs:subClassOf rdf:resource="http://www.semanticweb.org/qihan/ontologies/2023/6/untitled-ontology-12#Filament_Winding_Processes"/>
        <rdfs:comment>Represents a specific filament winding process where continuous fibers are wound around a mandrel or mold in a radial direction from a central point.</rdfs:comment>
        <rdfs:label>Radial Filament Winding</rdfs:label>
    </owl:Class>
    


    <!-- http://www.semanticweb.org/qihan/ontologies/2023/6/untitled-ontology-12#Radial_Orientation -->

    <owl:Class rdf:about="http://www.semanticweb.org/qihan/ontologies/2023/6/untitled-ontology-12#Radial_Orientation">
        <rdfs:subClassOf rdf:resource="http://www.semanticweb.org/qihan/ontologies/2023/6/untitled-ontology-12#Orientation"/>
        <rdfs:label>Radial Orientation</rdfs:label>
        <rdfs:label>Represents the orientation of a material along radial lines emanating from a central point.</rdfs:label>
    </owl:Class>
    


    <!-- http://www.semanticweb.org/qihan/ontologies/2023/6/untitled-ontology-12#Random_Orbital_Sander -->

    <owl:Class rdf:about="http://www.semanticweb.org/qihan/ontologies/2023/6/untitled-ontology-12#Random_Orbital_Sander">
        <rdfs:subClassOf rdf:resource="http://www.semanticweb.org/qihan/ontologies/2023/6/untitled-ontology-12#Grinding_and_Sanding_Equipment"/>
        <rdfs:comment>Represents a type of handheld sanding tool that combines rotary and orbital movements to create a random sanding pattern.</rdfs:comment>
        <rdfs:label>Random Orbital Sander</rdfs:label>
    </owl:Class>
    


    <!-- http://www.semanticweb.org/qihan/ontologies/2023/6/untitled-ontology-12#Randomly_Oriented_Fiber_Composite -->

    <owl:Class rdf:about="http://www.semanticweb.org/qihan/ontologies/2023/6/untitled-ontology-12#Randomly_Oriented_Fiber_Composite">
        <rdfs:subClassOf rdf:resource="http://www.semanticweb.org/qihan/ontologies/2023/6/untitled-ontology-12#Discontinuous_Fiber_Composite"/>
    </owl:Class>
    


    <!-- http://www.semanticweb.org/qihan/ontologies/2023/6/untitled-ontology-12#Reduced_Temperature -->

    <owl:Class rdf:about="http://www.semanticweb.org/qihan/ontologies/2023/6/untitled-ontology-12#Reduced_Temperature">
        <rdfs:subClassOf rdf:resource="http://www.semanticweb.org/qihan/ontologies/2023/6/untitled-ontology-12#Temperature"/>
        <rdfs:comment>Represents lower-than-ambient temperatures applied to composite material specimens during mechanical testing. It involves subjecting the specimens to reduced thermal conditions for specific testing purposes.</rdfs:comment>
        <rdfs:label>Reduced Temperature</rdfs:label>
    </owl:Class>
    


    <!-- http://www.semanticweb.org/qihan/ontologies/2023/6/untitled-ontology-12#Reflectance -->

    <owl:Class rdf:about="http://www.semanticweb.org/qihan/ontologies/2023/6/untitled-ontology-12#Reflectance">
        <rdfs:subClassOf rdf:resource="http://www.semanticweb.org/qihan/ontologies/2023/6/untitled-ontology-12#Optical_Properties"/>
    </owl:Class>
    


    <!-- http://www.semanticweb.org/qihan/ontologies/2023/6/untitled-ontology-12#Refractive_Index -->

    <owl:Class rdf:about="http://www.semanticweb.org/qihan/ontologies/2023/6/untitled-ontology-12#Refractive_Index">
        <rdfs:subClassOf rdf:resource="http://www.semanticweb.org/qihan/ontologies/2023/6/untitled-ontology-12#Optical_Properties"/>
    </owl:Class>
    


    <!-- http://www.semanticweb.org/qihan/ontologies/2023/6/untitled-ontology-12#Relative_Humidity_Level -->

    <owl:Class rdf:about="http://www.semanticweb.org/qihan/ontologies/2023/6/untitled-ontology-12#Relative_Humidity_Level">
        <rdfs:subClassOf rdf:resource="http://www.semanticweb.org/qihan/ontologies/2023/6/untitled-ontology-12#Humidity"/>
        <rdfs:comment>Represents the percentage of water vapor present in the air relative to the maximum amount of water vapor the air can hold at a specific temperature and pressure.</rdfs:comment>
        <rdfs:label>Relative Humidity Level</rdfs:label>
    </owl:Class>
    


    <!-- http://www.semanticweb.org/qihan/ontologies/2023/6/untitled-ontology-12#Relaxation_Time -->

    <owl:Class rdf:about="http://www.semanticweb.org/qihan/ontologies/2023/6/untitled-ontology-12#Relaxation_Time">
        <rdfs:subClassOf rdf:resource="http://www.semanticweb.org/qihan/ontologies/2023/6/untitled-ontology-12#Time"/>
        <rdfs:comment>Represents the time duration during which a material relaxes or recovers from a previous load or stress.</rdfs:comment>
        <rdfs:label>Relaxation Time</rdfs:label>
    </owl:Class>
    


    <!-- http://www.semanticweb.org/qihan/ontologies/2023/6/untitled-ontology-12#Research_Institute -->

    <owl:Class rdf:about="http://www.semanticweb.org/qihan/ontologies/2023/6/untitled-ontology-12#Research_Institute">
        <rdfs:subClassOf rdf:resource="http://www.semanticweb.org/qihan/ontologies/2023/6/untitled-ontology-12#Testing_Institution"/>
        <rdfs:comment>Represents an organization or facility dedicated to research and development activities in various fields, including materials science and engineering.</rdfs:comment>
        <rdfs:label>Research Institute</rdfs:label>
    </owl:Class>
    


    <!-- http://www.semanticweb.org/qihan/ontologies/2023/6/untitled-ontology-12#Residual_Stress -->

    <owl:Class rdf:about="http://www.semanticweb.org/qihan/ontologies/2023/6/untitled-ontology-12#Residual_Stress">
        <rdfs:subClassOf rdf:resource="http://www.semanticweb.org/qihan/ontologies/2023/6/untitled-ontology-12#Result_Calculation"/>
    </owl:Class>
    


    <!-- http://www.semanticweb.org/qihan/ontologies/2023/6/untitled-ontology-12#Resin_Film_Infusion -->

    <owl:Class rdf:about="http://www.semanticweb.org/qihan/ontologies/2023/6/untitled-ontology-12#Resin_Film_Infusion">
        <rdfs:subClassOf rdf:resource="http://www.semanticweb.org/qihan/ontologies/2023/6/untitled-ontology-12#Resin_Infusion_Processes"/>
        <rdfs:comment>Represents a specific resin infusion process where a dry fiber reinforcement is first laid up in a mold or tool, and then a thin, pre-made resin film is placed on top of the dry fibers.</rdfs:comment>
        <rdfs:label>Resin Film Infusion</rdfs:label>
    </owl:Class>
    


    <!-- http://www.semanticweb.org/qihan/ontologies/2023/6/untitled-ontology-12#Resin_Infusion_Processes -->

    <owl:Class rdf:about="http://www.semanticweb.org/qihan/ontologies/2023/6/untitled-ontology-12#Resin_Infusion_Processes">
        <rdfs:subClassOf rdf:resource="http://www.semanticweb.org/qihan/ontologies/2023/6/untitled-ontology-12#Material_Manufacturing"/>
        <rdfs:comment>Represents a group of manufacturing processes used to introduce resin into a dry fiber reinforcement to create composite parts.</rdfs:comment>
        <rdfs:label>Resin Infusion Process</rdfs:label>
    </owl:Class>
    


    <!-- http://www.semanticweb.org/qihan/ontologies/2023/6/untitled-ontology-12#Resin_Transfer_Molding -->

    <owl:Class rdf:about="http://www.semanticweb.org/qihan/ontologies/2023/6/untitled-ontology-12#Resin_Transfer_Molding">
        <rdfs:subClassOf rdf:resource="http://www.semanticweb.org/qihan/ontologies/2023/6/untitled-ontology-12#Resin_Infusion_Processes"/>
        <rdfs:comment>Represents a specific resin infusion process in which dry fiber preforms or reinforcements are placed in a closed mold.</rdfs:comment>
        <rdfs:label>Resin Transfer Molding (RTM)</rdfs:label>
    </owl:Class>
    


    <!-- http://www.semanticweb.org/qihan/ontologies/2023/6/untitled-ontology-12#Resonance_Frequency -->

    <owl:Class rdf:about="http://www.semanticweb.org/qihan/ontologies/2023/6/untitled-ontology-12#Resonance_Frequency">
        <rdfs:subClassOf rdf:resource="http://www.semanticweb.org/qihan/ontologies/2023/6/untitled-ontology-12#Frequency"/>
        <rdfs:comment>Represents the frequency at which a material, exhibits maximum vibrational amplitude or response when subjected to external vibrations or oscillations.</rdfs:comment>
        <rdfs:label>Resonance Frequency</rdfs:label>
    </owl:Class>
    


    <!-- http://www.semanticweb.org/qihan/ontologies/2023/6/untitled-ontology-12#Result_Analysis -->

    <owl:Class rdf:about="http://www.semanticweb.org/qihan/ontologies/2023/6/untitled-ontology-12#Result_Analysis">
        <rdfs:subClassOf rdf:resource="http://www.semanticweb.org/qihan/ontologies/2023/6/untitled-ontology-12#Post-Testing_Phase"/>
    </owl:Class>
    


    <!-- http://www.semanticweb.org/qihan/ontologies/2023/6/untitled-ontology-12#Result_Calculation -->

    <owl:Class rdf:about="http://www.semanticweb.org/qihan/ontologies/2023/6/untitled-ontology-12#Result_Calculation">
        <rdfs:subClassOf rdf:resource="http://www.semanticweb.org/qihan/ontologies/2023/6/untitled-ontology-12#Result_Analysis"/>
    </owl:Class>
    


    <!-- http://www.semanticweb.org/qihan/ontologies/2023/6/untitled-ontology-12#Rheometer -->

    <owl:Class rdf:about="http://www.semanticweb.org/qihan/ontologies/2023/6/untitled-ontology-12#Rheometer">
        <rdfs:subClassOf rdf:resource="http://www.semanticweb.org/qihan/ontologies/2023/6/untitled-ontology-12#Test_Equipment"/>
        <rdfs:comment>Represents a specialized instrument used to study the rheological properties of composite material specimens, such as their viscosity, flow behavior, and deformation response under different conditions.</rdfs:comment>
        <rdfs:label>Rheometer</rdfs:label>
    </owl:Class>
    


    <!-- http://www.semanticweb.org/qihan/ontologies/2023/6/untitled-ontology-12#Rockwell_Hardness -->

    <owl:Class rdf:about="http://www.semanticweb.org/qihan/ontologies/2023/6/untitled-ontology-12#Rockwell_Hardness">
        <rdfs:subClassOf rdf:resource="http://www.semanticweb.org/qihan/ontologies/2023/6/untitled-ontology-12#Hardness"/>
    </owl:Class>
    


    <!-- http://www.semanticweb.org/qihan/ontologies/2023/6/untitled-ontology-12#Rockwell_Hardness_Tester -->

    <owl:Class rdf:about="http://www.semanticweb.org/qihan/ontologies/2023/6/untitled-ontology-12#Rockwell_Hardness_Tester">
        <rdfs:subClassOf rdf:resource="http://www.semanticweb.org/qihan/ontologies/2023/6/untitled-ontology-12#Hardness_Tester"/>
        <rdfs:comment>Represents a specific type of hardness tester used to determine the Rockwell hardness of materials, including composite material specimens.</rdfs:comment>
        <rdfs:label>Rockwell Hardness Tester</rdfs:label>
    </owl:Class>
    


    <!-- http://www.semanticweb.org/qihan/ontologies/2023/6/untitled-ontology-12#Rockwell_Hardness_Testing -->

    <owl:Class rdf:about="http://www.semanticweb.org/qihan/ontologies/2023/6/untitled-ontology-12#Rockwell_Hardness_Testing">
        <rdfs:subClassOf rdf:resource="http://www.semanticweb.org/qihan/ontologies/2023/6/untitled-ontology-12#Hardness_Testing"/>
        <rdfs:comment>Represents a type of hardness testing method used to determine the hardness of materials, by measuring the depth of penetration of an indenter into the material under two loads - minor and major loads.</rdfs:comment>
        <rdfs:label>Rockwell Hardness Testing</rdfs:label>
    </owl:Class>
    


    <!-- http://www.semanticweb.org/qihan/ontologies/2023/6/untitled-ontology-12#Rotary_Torque_Testing_Machine -->

    <owl:Class rdf:about="http://www.semanticweb.org/qihan/ontologies/2023/6/untitled-ontology-12#Rotary_Torque_Testing_Machine">
        <rdfs:subClassOf rdf:resource="http://www.semanticweb.org/qihan/ontologies/2023/6/untitled-ontology-12#Torque_Testing_Machine"/>
        <rdfs:comment>Represents a specialized testing machine used to measure the torque or rotational force applied to a material.</rdfs:comment>
        <rdfs:label>Rotary Torque Testing Machine</rdfs:label>
    </owl:Class>
    


    <!-- http://www.semanticweb.org/qihan/ontologies/2023/6/untitled-ontology-12#Rotating_Bending_Fatigue_Testing_Machine -->

    <owl:Class rdf:about="http://www.semanticweb.org/qihan/ontologies/2023/6/untitled-ontology-12#Rotating_Bending_Fatigue_Testing_Machine">
        <rdfs:subClassOf rdf:resource="http://www.semanticweb.org/qihan/ontologies/2023/6/untitled-ontology-12#Fatigue_Testing_Machine"/>
        <rdfs:comment>Represents a specific type of testing machine used for conducting fatigue tests on composite material specimens under axial loading conditions. It applies cyclic axial loads to assess the material&apos;s fatigue life and behavior under tension-compression loading.</rdfs:comment>
        <rdfs:label>Rotating Bending Fatigue Testing Machine</rdfs:label>
    </owl:Class>
    


    <!-- http://www.semanticweb.org/qihan/ontologies/2023/6/untitled-ontology-12#Rotational_Rheometer -->

    <owl:Class rdf:about="http://www.semanticweb.org/qihan/ontologies/2023/6/untitled-ontology-12#Rotational_Rheometer">
        <rdfs:subClassOf rdf:resource="http://www.semanticweb.org/qihan/ontologies/2023/6/untitled-ontology-12#Rheometer"/>
        <rdfs:comment>Represents a specific type of rheometer used to measure the flow and deformation behavior of materials.</rdfs:comment>
        <rdfs:label>Rotational Rheometer</rdfs:label>
    </owl:Class>
    


    <!-- http://www.semanticweb.org/qihan/ontologies/2023/6/untitled-ontology-12#Rz -->

    <owl:Class rdf:about="http://www.semanticweb.org/qihan/ontologies/2023/6/untitled-ontology-12#Rz">
        <rdfs:subClassOf rdf:resource="http://www.semanticweb.org/qihan/ontologies/2023/6/untitled-ontology-12#Surface_Roughness"/>
    </owl:Class>
    


    <!-- http://www.semanticweb.org/qihan/ontologies/2023/6/untitled-ontology-12#SMC_Compression_Molding -->

    <owl:Class rdf:about="http://www.semanticweb.org/qihan/ontologies/2023/6/untitled-ontology-12#SMC_Compression_Molding">
        <rdfs:subClassOf rdf:resource="http://www.semanticweb.org/qihan/ontologies/2023/6/untitled-ontology-12#Sheet_Molding_Compound__Processes"/>
        <rdfs:comment>Represents a specific sheet molding compound process where SMC sheets are placed in a compression mold.</rdfs:comment>
        <rdfs:label>SMC Compression Molding</rdfs:label>
    </owl:Class>
    


    <!-- http://www.semanticweb.org/qihan/ontologies/2023/6/untitled-ontology-12#SMC_Fabrication -->

    <owl:Class rdf:about="http://www.semanticweb.org/qihan/ontologies/2023/6/untitled-ontology-12#SMC_Fabrication">
        <rdfs:subClassOf rdf:resource="http://www.semanticweb.org/qihan/ontologies/2023/6/untitled-ontology-12#Sheet_Molding_Compound__Processes"/>
        <rdfs:comment>Represents a specific sheet molding compound process that involves the fabrication of SMC sheets.</rdfs:comment>
        <rdfs:label>SMC Fabrication</rdfs:label>
    </owl:Class>
    


    <!-- http://www.semanticweb.org/qihan/ontologies/2023/6/untitled-ontology-12#Sand_Slingers -->

    <owl:Class rdf:about="http://www.semanticweb.org/qihan/ontologies/2023/6/untitled-ontology-12#Sand_Slingers">
        <rdfs:subClassOf rdf:resource="http://www.semanticweb.org/qihan/ontologies/2023/6/untitled-ontology-12#Molding_Machine"/>
        <rdfs:comment>Represents a type of molding machine used in foundries to create sand molds by flinging sand onto a pattern.</rdfs:comment>
        <rdfs:label>Sand Slingers</rdfs:label>
    </owl:Class>
    


    <!-- http://www.semanticweb.org/qihan/ontologies/2023/6/untitled-ontology-12#Sandwich_Composite -->

    <owl:Class rdf:about="http://www.semanticweb.org/qihan/ontologies/2023/6/untitled-ontology-12#Sandwich_Composite">
        <rdfs:subClassOf rdf:resource="http://www.semanticweb.org/qihan/ontologies/2023/6/untitled-ontology-12#Composite_Material"/>
    </owl:Class>
    


    <!-- http://www.semanticweb.org/qihan/ontologies/2023/6/untitled-ontology-12#Scanning_Electron_Microscope -->

    <owl:Class rdf:about="http://www.semanticweb.org/qihan/ontologies/2023/6/untitled-ontology-12#Scanning_Electron_Microscope">
        <rdfs:subClassOf rdf:resource="http://www.semanticweb.org/qihan/ontologies/2023/6/untitled-ontology-12#Microscope"/>
        <rdfs:comment>Represents a type of electron microscope that uses focused electron beams to obtain detailed images of the surface topography and microstructure of composite material specimens.</rdfs:comment>
        <rdfs:label>Scanning Electron Microscope (SEM)</rdfs:label>
    </owl:Class>
    


    <!-- http://www.semanticweb.org/qihan/ontologies/2023/6/untitled-ontology-12#Scissors -->

    <owl:Class rdf:about="http://www.semanticweb.org/qihan/ontologies/2023/6/untitled-ontology-12#Scissors">
        <rdfs:subClassOf rdf:resource="http://www.semanticweb.org/qihan/ontologies/2023/6/untitled-ontology-12#Handheld_Cutting_Tools"/>
        <rdfs:comment>Represents a type of cutting tool.</rdfs:comment>
        <rdfs:label>Scissors</rdfs:label>
    </owl:Class>
    


    <!-- http://www.semanticweb.org/qihan/ontologies/2023/6/untitled-ontology-12#Sectioning_Equipment -->

    <owl:Class rdf:about="http://www.semanticweb.org/qihan/ontologies/2023/6/untitled-ontology-12#Sectioning_Equipment">
        <rdfs:subClassOf rdf:resource="http://www.semanticweb.org/qihan/ontologies/2023/6/untitled-ontology-12#Specimen_Preparation_Equipment"/>
        <rdfs:comment>Represents a general category of equipment used for the process of sectioning or cutting materials into smaller, representative samples or slices for further analysis and examination.</rdfs:comment>
        <rdfs:label>Sectioning Equipment</rdfs:label>
    </owl:Class>
    


    <!-- http://www.semanticweb.org/qihan/ontologies/2023/6/untitled-ontology-12#Self-healing_Composite -->

    <owl:Class rdf:about="http://www.semanticweb.org/qihan/ontologies/2023/6/untitled-ontology-12#Self-healing_Composite">
        <rdfs:subClassOf rdf:resource="http://www.semanticweb.org/qihan/ontologies/2023/6/untitled-ontology-12#Composite_Material"/>
    </owl:Class>
    


    <!-- http://www.semanticweb.org/qihan/ontologies/2023/6/untitled-ontology-12#Servo-Hydraulic_Testing_Machine -->

    <owl:Class rdf:about="http://www.semanticweb.org/qihan/ontologies/2023/6/untitled-ontology-12#Servo-Hydraulic_Testing_Machine">
        <rdfs:subClassOf rdf:resource="http://www.semanticweb.org/qihan/ontologies/2023/6/untitled-ontology-12#Universal_Testing_Machine"/>
        <rdfs:comment>Represents a type of testing machine that combines the advantages of hydraulic and servo-controlled systems to apply precise forces and deformations to materials.</rdfs:comment>
        <rdfs:label>Servo-Hydraulic Testing Machine</rdfs:label>
    </owl:Class>
    


    <!-- http://www.semanticweb.org/qihan/ontologies/2023/6/untitled-ontology-12#Shape_Memory_Polymer-based_Self-healing_Composite -->

    <owl:Class rdf:about="http://www.semanticweb.org/qihan/ontologies/2023/6/untitled-ontology-12#Shape_Memory_Polymer-based_Self-healing_Composite">
        <rdfs:subClassOf rdf:resource="http://www.semanticweb.org/qihan/ontologies/2023/6/untitled-ontology-12#Self-healing_Composite"/>
    </owl:Class>
    


    <!-- http://www.semanticweb.org/qihan/ontologies/2023/6/untitled-ontology-12#Shear-Lap_Testing -->

    <owl:Class rdf:about="http://www.semanticweb.org/qihan/ontologies/2023/6/untitled-ontology-12#Shear-Lap_Testing">
        <rdfs:subClassOf rdf:resource="http://www.semanticweb.org/qihan/ontologies/2023/6/untitled-ontology-12#Testing_Method"/>
        <rdfs:comment>Represents a type of mechanical testing used to determine the shear strength of adhesively bonded materials,  with a lap joint configuration.</rdfs:comment>
        <rdfs:label>Shear-Lap Testing</rdfs:label>
    </owl:Class>
    


    <!-- http://www.semanticweb.org/qihan/ontologies/2023/6/untitled-ontology-12#Shear_Load -->

    <owl:Class rdf:about="http://www.semanticweb.org/qihan/ontologies/2023/6/untitled-ontology-12#Shear_Load">
        <rdfs:subClassOf rdf:resource="http://www.semanticweb.org/qihan/ontologies/2023/6/untitled-ontology-12#Load"/>
        <rdfs:comment>Represents the external force or load applied to a material, in a direction that causes the material to slide or deform along parallel planes.</rdfs:comment>
        <rdfs:label>Shear Load</rdfs:label>
    </owl:Class>
    


    <!-- http://www.semanticweb.org/qihan/ontologies/2023/6/untitled-ontology-12#Shear_Modulus -->

    <owl:Class rdf:about="http://www.semanticweb.org/qihan/ontologies/2023/6/untitled-ontology-12#Shear_Modulus">
        <rdfs:subClassOf rdf:resource="http://www.semanticweb.org/qihan/ontologies/2023/6/untitled-ontology-12#Stiffness"/>
    </owl:Class>
    


    <!-- http://www.semanticweb.org/qihan/ontologies/2023/6/untitled-ontology-12#Shear_Strain -->

    <owl:Class rdf:about="http://www.semanticweb.org/qihan/ontologies/2023/6/untitled-ontology-12#Shear_Strain">
        <rdfs:subClassOf rdf:resource="http://www.semanticweb.org/qihan/ontologies/2023/6/untitled-ontology-12#Strain"/>
        <rdfs:comment>Represents the change in shape or deformation due to the applied force parallel to the cross-sectional plane of a material.</rdfs:comment>
        <rdfs:label>Shear Strain</rdfs:label>
    </owl:Class>
    


    <!-- http://www.semanticweb.org/qihan/ontologies/2023/6/untitled-ontology-12#Shear_Strain_Rate -->

    <owl:Class rdf:about="http://www.semanticweb.org/qihan/ontologies/2023/6/untitled-ontology-12#Shear_Strain_Rate">
        <rdfs:subClassOf rdf:resource="http://www.semanticweb.org/qihan/ontologies/2023/6/untitled-ontology-12#Strain_Rate"/>
        <rdfs:comment>Represents the rate at which a material undergoes shear strain or deformation over time.</rdfs:comment>
        <rdfs:label>Shear Strain Rate</rdfs:label>
    </owl:Class>
    


    <!-- http://www.semanticweb.org/qihan/ontologies/2023/6/untitled-ontology-12#Shear_Strength -->

    <owl:Class rdf:about="http://www.semanticweb.org/qihan/ontologies/2023/6/untitled-ontology-12#Shear_Strength">
        <rdfs:subClassOf rdf:resource="http://www.semanticweb.org/qihan/ontologies/2023/6/untitled-ontology-12#Strength"/>
    </owl:Class>
    


    <!-- http://www.semanticweb.org/qihan/ontologies/2023/6/untitled-ontology-12#Shear_Stress -->

    <owl:Class rdf:about="http://www.semanticweb.org/qihan/ontologies/2023/6/untitled-ontology-12#Shear_Stress">
        <rdfs:subClassOf rdf:resource="http://www.semanticweb.org/qihan/ontologies/2023/6/untitled-ontology-12#Stress"/>
        <rdfs:comment>Represents the internal resistance or force per unit area that a material experiences when subjected to shear forces.</rdfs:comment>
        <rdfs:label>Shear Stress</rdfs:label>
    </owl:Class>
    


    <!-- http://www.semanticweb.org/qihan/ontologies/2023/6/untitled-ontology-12#Shear_Testing -->

    <owl:Class rdf:about="http://www.semanticweb.org/qihan/ontologies/2023/6/untitled-ontology-12#Shear_Testing">
        <rdfs:subClassOf rdf:resource="http://www.semanticweb.org/qihan/ontologies/2023/6/untitled-ontology-12#Testing_Method"/>
        <rdfs:comment>Represents a type of mechanical testing used to determine the shear strength and deformation behavior of materials, including composites, under applied forces parallel to the plane of the material.</rdfs:comment>
        <rdfs:label>Shear Testing</rdfs:label>
    </owl:Class>
    


    <!-- http://www.semanticweb.org/qihan/ontologies/2023/6/untitled-ontology-12#Shear_Testing_Apparatus -->

    <owl:Class rdf:about="http://www.semanticweb.org/qihan/ontologies/2023/6/untitled-ontology-12#Shear_Testing_Apparatus">
        <rdfs:subClassOf rdf:resource="http://www.semanticweb.org/qihan/ontologies/2023/6/untitled-ontology-12#Test_Equipment"/>
        <rdfs:comment>Represents a specific type of test equipment used to evaluate the shear strength and behavior of material specimens.</rdfs:comment>
    </owl:Class>
    


    <!-- http://www.semanticweb.org/qihan/ontologies/2023/6/untitled-ontology-12#Shearing -->

    <owl:Class rdf:about="http://www.semanticweb.org/qihan/ontologies/2023/6/untitled-ontology-12#Shearing">
        <rdfs:subClassOf rdf:resource="http://www.semanticweb.org/qihan/ontologies/2023/6/untitled-ontology-12#Failure_Mode"/>
    </owl:Class>
    


    <!-- http://www.semanticweb.org/qihan/ontologies/2023/6/untitled-ontology-12#Sheet_Forming_Processes -->

    <owl:Class rdf:about="http://www.semanticweb.org/qihan/ontologies/2023/6/untitled-ontology-12#Sheet_Forming_Processes">
        <rdfs:subClassOf rdf:resource="http://www.semanticweb.org/qihan/ontologies/2023/6/untitled-ontology-12#Material_Manufacturing"/>
        <rdfs:comment>Represents a group of manufacturing processes used to shape and form composite sheets or panels into desired geometries.</rdfs:comment>
        <rdfs:label>Sheet Forming Processes</rdfs:label>
    </owl:Class>
    


    <!-- http://www.semanticweb.org/qihan/ontologies/2023/6/untitled-ontology-12#Sheet_Molding_Compound__Processes -->

    <owl:Class rdf:about="http://www.semanticweb.org/qihan/ontologies/2023/6/untitled-ontology-12#Sheet_Molding_Compound__Processes">
        <rdfs:subClassOf rdf:resource="http://www.semanticweb.org/qihan/ontologies/2023/6/untitled-ontology-12#Material_Manufacturing"/>
        <rdfs:comment>Represents a group of manufacturing processes that use sheet molding compounds (SMCs) to produce composite parts.</rdfs:comment>
        <rdfs:label>Sheet Molding Compound (SMC) Processes</rdfs:label>
    </owl:Class>
    


    <!-- http://www.semanticweb.org/qihan/ontologies/2023/6/untitled-ontology-12#Short_Beam_Specimen -->

    <owl:Class rdf:about="http://www.semanticweb.org/qihan/ontologies/2023/6/untitled-ontology-12#Short_Beam_Specimen">
        <rdfs:subClassOf rdf:resource="http://www.semanticweb.org/qihan/ontologies/2023/6/untitled-ontology-12#Test_Specimen_Geometry"/>
        <rdfs:comment>Represents a type of test specimen with a relatively short length compared to its width and thickness, often used in flexural and shear tests.</rdfs:comment>
        <rdfs:label>Short Beam Specimen</rdfs:label>
    </owl:Class>
    


    <!-- http://www.semanticweb.org/qihan/ontologies/2023/6/untitled-ontology-12#Short_Fiber_Reinforced_Composite -->

    <owl:Class rdf:about="http://www.semanticweb.org/qihan/ontologies/2023/6/untitled-ontology-12#Short_Fiber_Reinforced_Composite">
        <rdfs:subClassOf rdf:resource="http://www.semanticweb.org/qihan/ontologies/2023/6/untitled-ontology-12#Discontinuous_Fiber_Composite"/>
    </owl:Class>
    


    <!-- http://www.semanticweb.org/qihan/ontologies/2023/6/untitled-ontology-12#Silicon_Carbide_Matrix_Composite -->

    <owl:Class rdf:about="http://www.semanticweb.org/qihan/ontologies/2023/6/untitled-ontology-12#Silicon_Carbide_Matrix_Composite">
        <rdfs:subClassOf rdf:resource="http://www.semanticweb.org/qihan/ontologies/2023/6/untitled-ontology-12#Ceramic_Matrix_Composite"/>
    </owl:Class>
    


    <!-- http://www.semanticweb.org/qihan/ontologies/2023/6/untitled-ontology-12#Single_Cantilever_Beam_DMA -->

    <owl:Class rdf:about="http://www.semanticweb.org/qihan/ontologies/2023/6/untitled-ontology-12#Single_Cantilever_Beam_DMA">
        <rdfs:subClassOf rdf:resource="http://www.semanticweb.org/qihan/ontologies/2023/6/untitled-ontology-12#Dynamic_Mechanical_Analyzer"/>
        <rdfs:comment>Represents a specific type of DMA test configuration used for analyzing the viscoelastic properties of composite material specimens. In this setup, the specimen is fixed at one end and subjected to controlled bending motion to evaluate its dynamic behavior.</rdfs:comment>
        <rdfs:label>Single Cantilever Beam DMA</rdfs:label>
    </owl:Class>
    


    <!-- http://www.semanticweb.org/qihan/ontologies/2023/6/untitled-ontology-12#Snips -->

    <owl:Class rdf:about="http://www.semanticweb.org/qihan/ontologies/2023/6/untitled-ontology-12#Snips">
        <rdfs:subClassOf rdf:resource="http://www.semanticweb.org/qihan/ontologies/2023/6/untitled-ontology-12#Handheld_Cutting_Tools"/>
        <rdfs:comment>Represents a type of cutting tool.</rdfs:comment>
        <rdfs:label>Snips</rdfs:label>
    </owl:Class>
    


    <!-- http://www.semanticweb.org/qihan/ontologies/2023/6/untitled-ontology-12#Solvent_Cleaning_Station -->

    <owl:Class rdf:about="http://www.semanticweb.org/qihan/ontologies/2023/6/untitled-ontology-12#Solvent_Cleaning_Station">
        <rdfs:subClassOf rdf:resource="http://www.semanticweb.org/qihan/ontologies/2023/6/untitled-ontology-12#Specimen_Cleaning_Equipment"/>
        <rdfs:comment>Represents a specialized cleaning station equipped with solvents and cleaning agents to remove organic and non-organic contaminants from specimens and samples.</rdfs:comment>
        <rdfs:label>Solvent Cleaning Station</rdfs:label>
    </owl:Class>
    


    <!-- http://www.semanticweb.org/qihan/ontologies/2023/6/untitled-ontology-12#Sound_Tranmission_Loss -->

    <owl:Class rdf:about="http://www.semanticweb.org/qihan/ontologies/2023/6/untitled-ontology-12#Sound_Tranmission_Loss">
        <rdfs:subClassOf rdf:resource="http://www.semanticweb.org/qihan/ontologies/2023/6/untitled-ontology-12#Acoustic_Properties"/>
    </owl:Class>
    


    <!-- http://www.semanticweb.org/qihan/ontologies/2023/6/untitled-ontology-12#Specimen_Cleaning_Equipment -->

    <owl:Class rdf:about="http://www.semanticweb.org/qihan/ontologies/2023/6/untitled-ontology-12#Specimen_Cleaning_Equipment">
        <rdfs:subClassOf rdf:resource="http://www.semanticweb.org/qihan/ontologies/2023/6/untitled-ontology-12#Specimen_Preparation_Equipment"/>
        <rdfs:comment>Represents a category of equipment used for cleaning specimens and samples to remove contaminants, debris, or surface impurities before conducting further tests or analyses.</rdfs:comment>
        <rdfs:label>Specimen Cleaning Equipment</rdfs:label>
    </owl:Class>
    


    <!-- http://www.semanticweb.org/qihan/ontologies/2023/6/untitled-ontology-12#Specimen_Preparation_Equipment -->

    <owl:Class rdf:about="http://www.semanticweb.org/qihan/ontologies/2023/6/untitled-ontology-12#Specimen_Preparation_Equipment">
        <rdfs:subClassOf rdf:resource="http://www.semanticweb.org/qihan/ontologies/2023/6/untitled-ontology-12#Material_Preparation"/>
        <rdfs:comment>Represents a group of equipment used in the preparation of test specimens for mechanical testing of composites.</rdfs:comment>
        <rdfs:label>Specimen Preparation Equipment</rdfs:label>
    </owl:Class>
    


    <!-- http://www.semanticweb.org/qihan/ontologies/2023/6/untitled-ontology-12#Specimen_Thickness -->

    <owl:Class rdf:about="http://www.semanticweb.org/qihan/ontologies/2023/6/untitled-ontology-12#Specimen_Thickness">
        <rdfs:subClassOf rdf:resource="http://www.semanticweb.org/qihan/ontologies/2023/6/untitled-ontology-12#Thickness"/>
        <rdfs:comment>Represents the measurement of the thickness of a material specimen.</rdfs:comment>
        <rdfs:label>Specimen Thickness</rdfs:label>
    </owl:Class>
    


    <!-- http://www.semanticweb.org/qihan/ontologies/2023/6/untitled-ontology-12#Squeezers -->

    <owl:Class rdf:about="http://www.semanticweb.org/qihan/ontologies/2023/6/untitled-ontology-12#Squeezers">
        <rdfs:subClassOf rdf:resource="http://www.semanticweb.org/qihan/ontologies/2023/6/untitled-ontology-12#Molding_Machine"/>
        <rdfs:comment>Represents a type of molding machine used in foundries for molding operations.</rdfs:comment>
        <rdfs:label>Squeezers</rdfs:label>
    </owl:Class>
    


    <!-- http://www.semanticweb.org/qihan/ontologies/2023/6/untitled-ontology-12#Static_Torque_Testing_Machine -->

    <owl:Class rdf:about="http://www.semanticweb.org/qihan/ontologies/2023/6/untitled-ontology-12#Static_Torque_Testing_Machine">
        <rdfs:subClassOf rdf:resource="http://www.semanticweb.org/qihan/ontologies/2023/6/untitled-ontology-12#Torque_Testing_Machine"/>
        <rdfs:comment>Represents a specialized testing machine used to measure the static or stationary torque applied to a material, including composite material specimens.</rdfs:comment>
        <rdfs:label>Static Torque Testing Machine</rdfs:label>
    </owl:Class>
    


    <!-- http://www.semanticweb.org/qihan/ontologies/2023/6/untitled-ontology-12#Statistical_Analysis -->

    <owl:Class rdf:about="http://www.semanticweb.org/qihan/ontologies/2023/6/untitled-ontology-12#Statistical_Analysis">
        <rdfs:subClassOf rdf:resource="http://www.semanticweb.org/qihan/ontologies/2023/6/untitled-ontology-12#Result_Analysis"/>
    </owl:Class>
    


    <!-- http://www.semanticweb.org/qihan/ontologies/2023/6/untitled-ontology-12#Stereolithography -->

    <owl:Class rdf:about="http://www.semanticweb.org/qihan/ontologies/2023/6/untitled-ontology-12#Stereolithography">
        <rdfs:subClassOf rdf:resource="http://www.semanticweb.org/qihan/ontologies/2023/6/untitled-ontology-12#Additive_Manufacturing_Processes"/>
        <rdfs:comment>Represents an additive manufacturing process that uses a liquid photopolymer resin cured by a light source.</rdfs:comment>
        <rdfs:label xml:lang="en">Stereolithography (SLA)</rdfs:label>
    </owl:Class>
    


    <!-- http://www.semanticweb.org/qihan/ontologies/2023/6/untitled-ontology-12#Stiffness -->

    <owl:Class rdf:about="http://www.semanticweb.org/qihan/ontologies/2023/6/untitled-ontology-12#Stiffness">
        <rdfs:subClassOf rdf:resource="http://www.semanticweb.org/qihan/ontologies/2023/6/untitled-ontology-12#Result_Calculation"/>
    </owl:Class>
    


    <!-- http://www.semanticweb.org/qihan/ontologies/2023/6/untitled-ontology-12#Strach-based_Composite -->

    <owl:Class rdf:about="http://www.semanticweb.org/qihan/ontologies/2023/6/untitled-ontology-12#Strach-based_Composite">
        <rdfs:subClassOf rdf:resource="http://www.semanticweb.org/qihan/ontologies/2023/6/untitled-ontology-12#Bio-based_Composite"/>
    </owl:Class>
    


    <!-- http://www.semanticweb.org/qihan/ontologies/2023/6/untitled-ontology-12#Strain -->

    <owl:Class rdf:about="http://www.semanticweb.org/qihan/ontologies/2023/6/untitled-ontology-12#Strain">
        <rdfs:subClassOf rdf:resource="http://www.semanticweb.org/qihan/ontologies/2023/6/untitled-ontology-12#Test_Parameter"/>
        <rdfs:comment>Represents the amount of deformation experienced by a material.</rdfs:comment>
        <rdfs:label>Strain</rdfs:label>
    </owl:Class>
    


    <!-- http://www.semanticweb.org/qihan/ontologies/2023/6/untitled-ontology-12#Strain_Gauge_Camera -->

    <owl:Class rdf:about="http://www.semanticweb.org/qihan/ontologies/2023/6/untitled-ontology-12#Strain_Gauge_Camera">
        <rdfs:subClassOf rdf:resource="http://www.semanticweb.org/qihan/ontologies/2023/6/untitled-ontology-12#High-Speed_Camera"/>
        <rdfs:comment>Represents a camera equipped with strain gauges or sensors that are used to measure strain in composite material specimens during mechanical testing.</rdfs:comment>
        <rdfs:label>Strain Gauge Camera</rdfs:label>
    </owl:Class>
    


    <!-- http://www.semanticweb.org/qihan/ontologies/2023/6/untitled-ontology-12#Strain_Gauge_Configuration -->

    <owl:Class rdf:about="http://www.semanticweb.org/qihan/ontologies/2023/6/untitled-ontology-12#Strain_Gauge_Configuration">
        <rdfs:subClassOf rdf:resource="http://www.semanticweb.org/qihan/ontologies/2023/6/untitled-ontology-12#Test_Parameter"/>
        <rdfs:comment>Represents the arrangement or configuration of strain gauges on a material or structure.</rdfs:comment>
        <rdfs:label>Strain Gauge Configuration</rdfs:label>
    </owl:Class>
    


    <!-- http://www.semanticweb.org/qihan/ontologies/2023/6/untitled-ontology-12#Strain_Rate -->

    <owl:Class rdf:about="http://www.semanticweb.org/qihan/ontologies/2023/6/untitled-ontology-12#Strain_Rate">
        <rdfs:subClassOf rdf:resource="http://www.semanticweb.org/qihan/ontologies/2023/6/untitled-ontology-12#Test_Parameter"/>
        <rdfs:comment>Represents the rate at which strain is applied or changes over time in a material.</rdfs:comment>
        <rdfs:label>Strain Rate</rdfs:label>
    </owl:Class>
    


    <!-- http://www.semanticweb.org/qihan/ontologies/2023/6/untitled-ontology-12#Strength -->

    <owl:Class rdf:about="http://www.semanticweb.org/qihan/ontologies/2023/6/untitled-ontology-12#Strength">
        <rdfs:subClassOf rdf:resource="http://www.semanticweb.org/qihan/ontologies/2023/6/untitled-ontology-12#Result_Calculation"/>
    </owl:Class>
    


    <!-- http://www.semanticweb.org/qihan/ontologies/2023/6/untitled-ontology-12#Stress -->

    <owl:Class rdf:about="http://www.semanticweb.org/qihan/ontologies/2023/6/untitled-ontology-12#Stress">
        <rdfs:subClassOf rdf:resource="http://www.semanticweb.org/qihan/ontologies/2023/6/untitled-ontology-12#Test_Parameter"/>
        <rdfs:comment>Represents the internal force or load per unit area experienced by a material.</rdfs:comment>
        <rdfs:label>Stress</rdfs:label>
    </owl:Class>
    


    <!-- http://www.semanticweb.org/qihan/ontologies/2023/6/untitled-ontology-12#Surface_Modification_with_Nanomaterials -->

    <owl:Class rdf:about="http://www.semanticweb.org/qihan/ontologies/2023/6/untitled-ontology-12#Surface_Modification_with_Nanomaterials">
        <rdfs:subClassOf rdf:resource="http://www.semanticweb.org/qihan/ontologies/2023/6/untitled-ontology-12#Nanofiber_and_Nanoparticle_Coating"/>
        <rdfs:comment>Represents the process of altering the surface properties of a material by incorporating nanomaterials, such as nanoparticles or nanofibers, onto its surface.</rdfs:comment>
        <rdfs:label>Surface Modification with Nanomaterials</rdfs:label>
    </owl:Class>
    


    <!-- http://www.semanticweb.org/qihan/ontologies/2023/6/untitled-ontology-12#Surface_Resistivity -->

    <owl:Class rdf:about="http://www.semanticweb.org/qihan/ontologies/2023/6/untitled-ontology-12#Surface_Resistivity">
        <rdfs:subClassOf rdf:resource="http://www.semanticweb.org/qihan/ontologies/2023/6/untitled-ontology-12#Electriical_Conductivity"/>
    </owl:Class>
    


    <!-- http://www.semanticweb.org/qihan/ontologies/2023/6/untitled-ontology-12#Surface_Roughness -->

    <owl:Class rdf:about="http://www.semanticweb.org/qihan/ontologies/2023/6/untitled-ontology-12#Surface_Roughness">
        <rdfs:subClassOf rdf:resource="http://www.semanticweb.org/qihan/ontologies/2023/6/untitled-ontology-12#Result_Calculation"/>
    </owl:Class>
    


    <!-- http://www.semanticweb.org/qihan/ontologies/2023/6/untitled-ontology-12#Taber_Abrasion_Tester -->

    <owl:Class rdf:about="http://www.semanticweb.org/qihan/ontologies/2023/6/untitled-ontology-12#Taber_Abrasion_Tester">
        <rdfs:subClassOf rdf:resource="http://www.semanticweb.org/qihan/ontologies/2023/6/untitled-ontology-12#Abrasion_Testing_Machine"/>
        <rdfs:comment>Represents a specific type of test equipment used to assess the abrasion resistance of composite material specimens by rotating them against an abrasive wheel or disk.</rdfs:comment>
        <rdfs:label>Taber Abrasion Tester</rdfs:label>
    </owl:Class>
    


    <!-- http://www.semanticweb.org/qihan/ontologies/2023/6/untitled-ontology-12#Temperature -->

    <owl:Class rdf:about="http://www.semanticweb.org/qihan/ontologies/2023/6/untitled-ontology-12#Temperature">
        <rdfs:subClassOf rdf:resource="http://www.semanticweb.org/qihan/ontologies/2023/6/untitled-ontology-12#Test_Environment"/>
        <rdfs:subClassOf rdf:resource="http://www.semanticweb.org/qihan/ontologies/2023/6/untitled-ontology-12#Test_Parameter"/>
        <rdfs:comment>Represents the measurement of thermal energy in the testing environment during mechanical testing of composite material specimens.</rdfs:comment>
        <rdfs:label>Temperature</rdfs:label>
    </owl:Class>
    


    <!-- http://www.semanticweb.org/qihan/ontologies/2023/6/untitled-ontology-12#Temperature_and_Humidity_Chamber -->

    <owl:Class rdf:about="http://www.semanticweb.org/qihan/ontologies/2023/6/untitled-ontology-12#Temperature_and_Humidity_Chamber">
        <rdfs:subClassOf rdf:resource="http://www.semanticweb.org/qihan/ontologies/2023/6/untitled-ontology-12#Environmental_Chamber"/>
        <rdfs:comment>Represents a specific type of climate chamber used to regulate both temperature and humidity levels during the testing of composite material specimens.</rdfs:comment>
        <rdfs:label>Temperature and Humidity Chamber</rdfs:label>
    </owl:Class>
    


    <!-- http://www.semanticweb.org/qihan/ontologies/2023/6/untitled-ontology-12#Tensile_Instron_Machine -->

    <owl:Class rdf:about="http://www.semanticweb.org/qihan/ontologies/2023/6/untitled-ontology-12#Tensile_Instron_Machine">
        <rdfs:subClassOf rdf:resource="http://www.semanticweb.org/qihan/ontologies/2023/6/untitled-ontology-12#Instron_Machine"/>
        <rdfs:comment>Represents a specific type of Instron machine used for conducting tensile tests on materials.</rdfs:comment>
        <rdfs:label>Tensile Instron Machine</rdfs:label>
    </owl:Class>
    


    <!-- http://www.semanticweb.org/qihan/ontologies/2023/6/untitled-ontology-12#Tensile_Load -->

    <owl:Class rdf:about="http://www.semanticweb.org/qihan/ontologies/2023/6/untitled-ontology-12#Tensile_Load">
        <rdfs:subClassOf rdf:resource="http://www.semanticweb.org/qihan/ontologies/2023/6/untitled-ontology-12#Load"/>
        <rdfs:comment>Represents the external force or load applied to a material, in a direction that tends to stretch or elongate the material along its axis.</rdfs:comment>
        <rdfs:label>Tensile Load</rdfs:label>
    </owl:Class>
    


    <!-- http://www.semanticweb.org/qihan/ontologies/2023/6/untitled-ontology-12#Tensile_Residual_Stress -->

    <owl:Class rdf:about="http://www.semanticweb.org/qihan/ontologies/2023/6/untitled-ontology-12#Tensile_Residual_Stress">
        <rdfs:subClassOf rdf:resource="http://www.semanticweb.org/qihan/ontologies/2023/6/untitled-ontology-12#Residual_Stress"/>
    </owl:Class>
    


    <!-- http://www.semanticweb.org/qihan/ontologies/2023/6/untitled-ontology-12#Tensile_Strain_Rate -->

    <owl:Class rdf:about="http://www.semanticweb.org/qihan/ontologies/2023/6/untitled-ontology-12#Tensile_Strain_Rate">
        <rdfs:subClassOf rdf:resource="http://www.semanticweb.org/qihan/ontologies/2023/6/untitled-ontology-12#Strain_Rate"/>
        <rdfs:comment>Represents the rate at which a material undergoes tensile strain or deformation over time.</rdfs:comment>
        <rdfs:label>Tensile Strain Rate</rdfs:label>
    </owl:Class>
    


    <!-- http://www.semanticweb.org/qihan/ontologies/2023/6/untitled-ontology-12#Tensile_Strength -->

    <owl:Class rdf:about="http://www.semanticweb.org/qihan/ontologies/2023/6/untitled-ontology-12#Tensile_Strength">
        <rdfs:subClassOf rdf:resource="http://www.semanticweb.org/qihan/ontologies/2023/6/untitled-ontology-12#Strength"/>
    </owl:Class>
    


    <!-- http://www.semanticweb.org/qihan/ontologies/2023/6/untitled-ontology-12#Tensile_Stress -->

    <owl:Class rdf:about="http://www.semanticweb.org/qihan/ontologies/2023/6/untitled-ontology-12#Tensile_Stress">
        <rdfs:subClassOf rdf:resource="http://www.semanticweb.org/qihan/ontologies/2023/6/untitled-ontology-12#Stress"/>
        <rdfs:comment>Represents the internal resistance or force per unit area that a material experiences when subjected to tensile forces.</rdfs:comment>
        <rdfs:label>Tensile Stress</rdfs:label>
    </owl:Class>
    


    <!-- http://www.semanticweb.org/qihan/ontologies/2023/6/untitled-ontology-12#Tensile_Testing -->

    <owl:Class rdf:about="http://www.semanticweb.org/qihan/ontologies/2023/6/untitled-ontology-12#Tensile_Testing">
        <rdfs:subClassOf rdf:resource="http://www.semanticweb.org/qihan/ontologies/2023/6/untitled-ontology-12#Testing_Method"/>
        <rdfs:comment>Represents a type of mechanical testing used to determine the tensile properties of materials, by subjecting a specimen to uniaxial tensile forces.</rdfs:comment>
        <rdfs:label>Tensile Testing</rdfs:label>
    </owl:Class>
    


    <!-- http://www.semanticweb.org/qihan/ontologies/2023/6/untitled-ontology-12#Test_Duration -->

    <owl:Class rdf:about="http://www.semanticweb.org/qihan/ontologies/2023/6/untitled-ontology-12#Test_Duration">
        <rdfs:subClassOf rdf:resource="http://www.semanticweb.org/qihan/ontologies/2023/6/untitled-ontology-12#Time"/>
        <rdfs:comment>Represents the total time duration of a mechanical test performed on a material.</rdfs:comment>
        <rdfs:label>Test Duration</rdfs:label>
    </owl:Class>
    


    <!-- http://www.semanticweb.org/qihan/ontologies/2023/6/untitled-ontology-12#Test_Environment -->

    <owl:Class rdf:about="http://www.semanticweb.org/qihan/ontologies/2023/6/untitled-ontology-12#Test_Environment">
        <rdfs:subClassOf rdf:resource="http://www.semanticweb.org/qihan/ontologies/2023/6/untitled-ontology-12#In-Testing_Phase"/>
        <rdfs:comment>The test environment represents the surrounding conditions and external factors that influence the mechanical test but are not directly controlled or intentionally varied during the test. The test environment includes aspects such as temperature, humidity, pressure, and other conditions in which the test specimen is subjected to during the test.</rdfs:comment>
        <rdfs:label>Test Environment</rdfs:label>
    </owl:Class>
    


    <!-- http://www.semanticweb.org/qihan/ontologies/2023/6/untitled-ontology-12#Test_Equipment -->

    <owl:Class rdf:about="http://www.semanticweb.org/qihan/ontologies/2023/6/untitled-ontology-12#Test_Equipment">
        <rdfs:subClassOf rdf:resource="http://www.semanticweb.org/qihan/ontologies/2023/6/untitled-ontology-12#In-Testing_Phase"/>
        <rdfs:comment>Represents the various types of equipment and apparatus used for conducting mechanical testing of composite material specimens.</rdfs:comment>
        <rdfs:label>Test Equipment</rdfs:label>
    </owl:Class>
    


    <!-- http://www.semanticweb.org/qihan/ontologies/2023/6/untitled-ontology-12#Test_Parameter -->

    <owl:Class rdf:about="http://www.semanticweb.org/qihan/ontologies/2023/6/untitled-ontology-12#Test_Parameter">
        <rdfs:subClassOf rdf:resource="http://www.semanticweb.org/qihan/ontologies/2023/6/untitled-ontology-12#In-Testing_Phase"/>
        <rdfs:comment>Test parameters are specific variables or factors that directly affect the behavior and outcome of the mechanical test on composite materials. These parameters are under direct control and are intentionally set to evaluate particular material properties or behaviors during the test.</rdfs:comment>
        <rdfs:label>Test Parameter</rdfs:label>
    </owl:Class>
    


    <!-- http://www.semanticweb.org/qihan/ontologies/2023/6/untitled-ontology-12#Test_Specimen_Geometry -->

    <owl:Class rdf:about="http://www.semanticweb.org/qihan/ontologies/2023/6/untitled-ontology-12#Test_Specimen_Geometry">
        <rdfs:subClassOf rdf:resource="http://www.semanticweb.org/qihan/ontologies/2023/6/untitled-ontology-12#Material_Preparation"/>
        <rdfs:comment>Represents a category of different geometric shapes and configurations used for creating test specimens or samples for various mechanical tests.</rdfs:comment>
        <rdfs:label>Test Specimen Geometry</rdfs:label>
    </owl:Class>
    


    <!-- http://www.semanticweb.org/qihan/ontologies/2023/6/untitled-ontology-12#Test_Standards -->

    <owl:Class rdf:about="http://www.semanticweb.org/qihan/ontologies/2023/6/untitled-ontology-12#Test_Standards">
        <rdfs:subClassOf rdf:resource="http://www.semanticweb.org/qihan/ontologies/2023/6/untitled-ontology-12#In-Testing_Phase"/>
        <rdfs:comment>Represents a set of standardized guidelines, procedures, and specifications developed by various organizations and regulatory bodies to ensure consistency and reliability in conducting mechanical tests on materials, including composites.</rdfs:comment>
        <rdfs:label>Test Standards</rdfs:label>
    </owl:Class>
    


    <!-- http://www.semanticweb.org/qihan/ontologies/2023/6/untitled-ontology-12#Testing_Institution -->

    <owl:Class rdf:about="http://www.semanticweb.org/qihan/ontologies/2023/6/untitled-ontology-12#Testing_Institution">
        <rdfs:comment>Represents an organization or facility that is responsible for conducting mechanical testing on composites and other materials.</rdfs:comment>
        <rdfs:label>Testing Institution</rdfs:label>
    </owl:Class>
    


    <!-- http://www.semanticweb.org/qihan/ontologies/2023/6/untitled-ontology-12#Testing_Method -->

    <owl:Class rdf:about="http://www.semanticweb.org/qihan/ontologies/2023/6/untitled-ontology-12#Testing_Method">
        <rdfs:subClassOf rdf:resource="http://www.semanticweb.org/qihan/ontologies/2023/6/untitled-ontology-12#In-Testing_Phase"/>
        <rdfs:comment>Represents a specific procedure or technique used to perform mechanical testing on materials, including composites.</rdfs:comment>
        <rdfs:label>Testing Method</rdfs:label>
    </owl:Class>
    


    <!-- http://www.semanticweb.org/qihan/ontologies/2023/6/untitled-ontology-12#Thermal_Aging_Resistance -->

    <owl:Class rdf:about="http://www.semanticweb.org/qihan/ontologies/2023/6/untitled-ontology-12#Thermal_Aging_Resistance">
        <rdfs:subClassOf rdf:resource="http://www.semanticweb.org/qihan/ontologies/2023/6/untitled-ontology-12#Aging_Properties"/>
    </owl:Class>
    


    <!-- http://www.semanticweb.org/qihan/ontologies/2023/6/untitled-ontology-12#Thermal_Analysis_Equipment -->

    <owl:Class rdf:about="http://www.semanticweb.org/qihan/ontologies/2023/6/untitled-ontology-12#Thermal_Analysis_Equipment">
        <rdfs:subClassOf rdf:resource="http://www.semanticweb.org/qihan/ontologies/2023/6/untitled-ontology-12#Test_Equipment"/>
        <rdfs:comment>Represents a category of test equipment used to analyze the thermal properties of  material specimens.</rdfs:comment>
        <rdfs:label>Thermal Analysis Equipment</rdfs:label>
    </owl:Class>
    


    <!-- http://www.semanticweb.org/qihan/ontologies/2023/6/untitled-ontology-12#Thermal_Conductivity -->

    <owl:Class rdf:about="http://www.semanticweb.org/qihan/ontologies/2023/6/untitled-ontology-12#Thermal_Conductivity">
        <rdfs:subClassOf rdf:resource="http://www.semanticweb.org/qihan/ontologies/2023/6/untitled-ontology-12#Result_Calculation"/>
    </owl:Class>
    


    <!-- http://www.semanticweb.org/qihan/ontologies/2023/6/untitled-ontology-12#Thermal_Conductivity_Measurement_Apparatus -->

    <owl:Class rdf:about="http://www.semanticweb.org/qihan/ontologies/2023/6/untitled-ontology-12#Thermal_Conductivity_Measurement_Apparatus">
        <rdfs:subClassOf rdf:resource="http://www.semanticweb.org/qihan/ontologies/2023/6/untitled-ontology-12#Test_Equipment"/>
        <rdfs:comment>Represents a specific type of equipment used to measure the thermal conductivity of composite material specimens. It assesses the ability of the material to conduct heat.</rdfs:comment>
        <rdfs:label>Thermal Conductivity Measurement Apparatus</rdfs:label>
    </owl:Class>
    


    <!-- http://www.semanticweb.org/qihan/ontologies/2023/6/untitled-ontology-12#Thermal_Conductivity_Testing -->

    <owl:Class rdf:about="http://www.semanticweb.org/qihan/ontologies/2023/6/untitled-ontology-12#Thermal_Conductivity_Testing">
        <rdfs:subClassOf rdf:resource="http://www.semanticweb.org/qihan/ontologies/2023/6/untitled-ontology-12#Thermal_Testing"/>
        <rdfs:comment>Represents a type of thermal testing used to measure the thermal conductivity of materials.</rdfs:comment>
        <rdfs:label>Thermal Conductivity Testing</rdfs:label>
    </owl:Class>
    


    <!-- http://www.semanticweb.org/qihan/ontologies/2023/6/untitled-ontology-12#Thermal_Diffusivity -->

    <owl:Class rdf:about="http://www.semanticweb.org/qihan/ontologies/2023/6/untitled-ontology-12#Thermal_Diffusivity">
        <rdfs:subClassOf rdf:resource="http://www.semanticweb.org/qihan/ontologies/2023/6/untitled-ontology-12#Thermal_Conductivity"/>
    </owl:Class>
    


    <!-- http://www.semanticweb.org/qihan/ontologies/2023/6/untitled-ontology-12#Thermal_Expansion_Coefficient -->

    <owl:Class rdf:about="http://www.semanticweb.org/qihan/ontologies/2023/6/untitled-ontology-12#Thermal_Expansion_Coefficient">
        <rdfs:subClassOf rdf:resource="http://www.semanticweb.org/qihan/ontologies/2023/6/untitled-ontology-12#Dimensional_Changes"/>
    </owl:Class>
    


    <!-- http://www.semanticweb.org/qihan/ontologies/2023/6/untitled-ontology-12#Thermal_Expansion_Testing -->

    <owl:Class rdf:about="http://www.semanticweb.org/qihan/ontologies/2023/6/untitled-ontology-12#Thermal_Expansion_Testing">
        <rdfs:subClassOf rdf:resource="http://www.semanticweb.org/qihan/ontologies/2023/6/untitled-ontology-12#Thermal_Testing"/>
        <rdfs:comment>Represents a type of thermal testing used to determine the coefficient of thermal expansion (CTE) of materials.</rdfs:comment>
        <rdfs:label>Thermal Expansion Testing</rdfs:label>
    </owl:Class>
    


    <!-- http://www.semanticweb.org/qihan/ontologies/2023/6/untitled-ontology-12#Thermal_Resistance -->

    <owl:Class rdf:about="http://www.semanticweb.org/qihan/ontologies/2023/6/untitled-ontology-12#Thermal_Resistance">
        <rdfs:subClassOf rdf:resource="http://www.semanticweb.org/qihan/ontologies/2023/6/untitled-ontology-12#Thermal_Conductivity"/>
    </owl:Class>
    


    <!-- http://www.semanticweb.org/qihan/ontologies/2023/6/untitled-ontology-12#Thermal_Testing -->

    <owl:Class rdf:about="http://www.semanticweb.org/qihan/ontologies/2023/6/untitled-ontology-12#Thermal_Testing">
        <rdfs:subClassOf rdf:resource="http://www.semanticweb.org/qihan/ontologies/2023/6/untitled-ontology-12#Testing_Method"/>
        <rdfs:comment>Represents a type of testing used to assess the thermal properties and behavior of materials, under different temperature conditions.</rdfs:comment>
        <rdfs:label>Thermal Testing</rdfs:label>
    </owl:Class>
    


    <!-- http://www.semanticweb.org/qihan/ontologies/2023/6/untitled-ontology-12#Thermoforming -->

    <owl:Class rdf:about="http://www.semanticweb.org/qihan/ontologies/2023/6/untitled-ontology-12#Thermoforming">
        <rdfs:subClassOf rdf:resource="http://www.semanticweb.org/qihan/ontologies/2023/6/untitled-ontology-12#Sheet_Forming_Processes"/>
        <rdfs:comment>Represents a specific sheet forming process where a thermoplastic composite sheet is heated until it becomes pliable and can be stretched and formed over a mold.</rdfs:comment>
        <rdfs:label>Thermoforming</rdfs:label>
    </owl:Class>
    


    <!-- http://www.semanticweb.org/qihan/ontologies/2023/6/untitled-ontology-12#Thermoforming_Molding -->

    <owl:Class rdf:about="http://www.semanticweb.org/qihan/ontologies/2023/6/untitled-ontology-12#Thermoforming_Molding">
        <rdfs:subClassOf rdf:resource="http://www.semanticweb.org/qihan/ontologies/2023/6/untitled-ontology-12#Molding_Machine"/>
        <rdfs:comment>Represents a molding process where a thermoplastic sheet is heated and formed into a specific shape using a mold or tool.</rdfs:comment>
        <rdfs:label>Thermoforming Molding</rdfs:label>
    </owl:Class>
    


    <!-- http://www.semanticweb.org/qihan/ontologies/2023/6/untitled-ontology-12#Thermogravimetric_Analyzer -->

    <owl:Class rdf:about="http://www.semanticweb.org/qihan/ontologies/2023/6/untitled-ontology-12#Thermogravimetric_Analyzer">
        <rdfs:subClassOf rdf:resource="http://www.semanticweb.org/qihan/ontologies/2023/6/untitled-ontology-12#Thermal_Analysis_Equipment"/>
        <rdfs:comment>Represents a specific type of thermal analysis equipment used to measure the weight changes of materials.</rdfs:comment>
        <rdfs:label>Thermogravimetric Analyzer (TGA)</rdfs:label>
    </owl:Class>
    


    <!-- http://www.semanticweb.org/qihan/ontologies/2023/6/untitled-ontology-12#Thickness -->

    <owl:Class rdf:about="http://www.semanticweb.org/qihan/ontologies/2023/6/untitled-ontology-12#Thickness">
        <rdfs:subClassOf rdf:resource="http://www.semanticweb.org/qihan/ontologies/2023/6/untitled-ontology-12#Test_Parameter"/>
        <rdfs:comment>Represents the distance between the two surfaces of a material.</rdfs:comment>
        <rdfs:label>Thickness</rdfs:label>
    </owl:Class>
    


    <!-- http://www.semanticweb.org/qihan/ontologies/2023/6/untitled-ontology-12#Three-Point_Bending_DMA -->

    <owl:Class rdf:about="http://www.semanticweb.org/qihan/ontologies/2023/6/untitled-ontology-12#Three-Point_Bending_DMA">
        <rdfs:subClassOf rdf:resource="http://www.semanticweb.org/qihan/ontologies/2023/6/untitled-ontology-12#Dynamic_Mechanical_Analyzer"/>
        <rdfs:comment>Represents a specific type of DMA test configuration used to study the viscoelastic properties of composite material specimens. In this setup, the specimen is supported at two points, and a force is applied at the third point to induce bending and analyze the material&apos;s dynamic response.</rdfs:comment>
        <rdfs:label>Three-Point Bending DMA</rdfs:label>
    </owl:Class>
    


    <!-- http://www.semanticweb.org/qihan/ontologies/2023/6/untitled-ontology-12#Three-Point_Bending_Specimen -->

    <owl:Class rdf:about="http://www.semanticweb.org/qihan/ontologies/2023/6/untitled-ontology-12#Three-Point_Bending_Specimen">
        <rdfs:subClassOf rdf:resource="http://www.semanticweb.org/qihan/ontologies/2023/6/untitled-ontology-12#Test_Specimen_Geometry"/>
        <rdfs:comment>Represents a type of test specimen with one loading point and two support points, creating a three-point bending configuration.</rdfs:comment>
        <rdfs:label>Three-Point Bending Specimen</rdfs:label>
    </owl:Class>
    


    <!-- http://www.semanticweb.org/qihan/ontologies/2023/6/untitled-ontology-12#Time -->

    <owl:Class rdf:about="http://www.semanticweb.org/qihan/ontologies/2023/6/untitled-ontology-12#Time">
        <rdfs:subClassOf rdf:resource="http://www.semanticweb.org/qihan/ontologies/2023/6/untitled-ontology-12#Test_Parameter"/>
        <rdfs:comment>Represents the duration or period during which a specific process, or measurement occurs in a material.</rdfs:comment>
        <rdfs:label>Time</rdfs:label>
    </owl:Class>
    


    <!-- http://www.semanticweb.org/qihan/ontologies/2023/6/untitled-ontology-12#Time_to_Failure -->

    <owl:Class rdf:about="http://www.semanticweb.org/qihan/ontologies/2023/6/untitled-ontology-12#Time_to_Failure">
        <rdfs:subClassOf rdf:resource="http://www.semanticweb.org/qihan/ontologies/2023/6/untitled-ontology-12#Creep_Behaviour"/>
    </owl:Class>
    


    <!-- http://www.semanticweb.org/qihan/ontologies/2023/6/untitled-ontology-12#Titanium_Matrix_Composite -->

    <owl:Class rdf:about="http://www.semanticweb.org/qihan/ontologies/2023/6/untitled-ontology-12#Titanium_Matrix_Composite">
        <rdfs:subClassOf rdf:resource="http://www.semanticweb.org/qihan/ontologies/2023/6/untitled-ontology-12#Metal_Matrix_Composite"/>
    </owl:Class>
    


    <!-- http://www.semanticweb.org/qihan/ontologies/2023/6/untitled-ontology-12#Torque_Testing_Machine -->

    <owl:Class rdf:about="http://www.semanticweb.org/qihan/ontologies/2023/6/untitled-ontology-12#Torque_Testing_Machine">
        <rdfs:subClassOf rdf:resource="http://www.semanticweb.org/qihan/ontologies/2023/6/untitled-ontology-12#Test_Equipment"/>
        <rdfs:comment>Represents a specific type of test equipment used to assess the torque or rotational characteristics of composite material specimens. It measures the resistance to rotational forces applied to the material.</rdfs:comment>
        <rdfs:label>Torque Testing Machine</rdfs:label>
    </owl:Class>
    


    <!-- http://www.semanticweb.org/qihan/ontologies/2023/6/untitled-ontology-12#Torsion_DMA -->

    <owl:Class rdf:about="http://www.semanticweb.org/qihan/ontologies/2023/6/untitled-ontology-12#Torsion_DMA">
        <rdfs:subClassOf rdf:resource="http://www.semanticweb.org/qihan/ontologies/2023/6/untitled-ontology-12#Dynamic_Mechanical_Analyzer"/>
        <rdfs:comment>Represents a specific type of DMA test configuration used to study the viscoelastic properties of composite material specimens. In this setup, the specimen is supported at two points, and a force is applied at the third point to induce bending and analyze the material&apos;s dynamic response.</rdfs:comment>
        <rdfs:label>Torsion DMA</rdfs:label>
    </owl:Class>
    


    <!-- http://www.semanticweb.org/qihan/ontologies/2023/6/untitled-ontology-12#Torsional_Fatigue_Testing_Machine -->

    <owl:Class rdf:about="http://www.semanticweb.org/qihan/ontologies/2023/6/untitled-ontology-12#Torsional_Fatigue_Testing_Machine">
        <rdfs:subClassOf rdf:resource="http://www.semanticweb.org/qihan/ontologies/2023/6/untitled-ontology-12#Fatigue_Testing_Machine"/>
        <rdfs:comment>Represents a specific type of testing machine used for conducting fatigue tests on composite material specimens under axial loading conditions. It applies cyclic axial loads to assess the material&apos;s fatigue life and behavior under tension-compression loading.</rdfs:comment>
        <rdfs:label>Rotating Bending Fatigue Testing Machine</rdfs:label>
    </owl:Class>
    


    <!-- http://www.semanticweb.org/qihan/ontologies/2023/6/untitled-ontology-12#Toughness -->

    <owl:Class rdf:about="http://www.semanticweb.org/qihan/ontologies/2023/6/untitled-ontology-12#Toughness">
        <rdfs:subClassOf rdf:resource="http://www.semanticweb.org/qihan/ontologies/2023/6/untitled-ontology-12#Result_Calculation"/>
    </owl:Class>
    


    <!-- http://www.semanticweb.org/qihan/ontologies/2023/6/untitled-ontology-12#Transmission_Electron_Microscope -->

    <owl:Class rdf:about="http://www.semanticweb.org/qihan/ontologies/2023/6/untitled-ontology-12#Transmission_Electron_Microscope">
        <rdfs:subClassOf rdf:resource="http://www.semanticweb.org/qihan/ontologies/2023/6/untitled-ontology-12#Microscope"/>
        <rdfs:comment>Represents a type of electron microscope that transmits electrons through ultra-thin sections of composite material specimens to produce high-resolution images of their internal structures.</rdfs:comment>
        <rdfs:label>Transmission Electron Microscope (TEM)</rdfs:label>
    </owl:Class>
    


    <!-- http://www.semanticweb.org/qihan/ontologies/2023/6/untitled-ontology-12#Transmittance -->

    <owl:Class rdf:about="http://www.semanticweb.org/qihan/ontologies/2023/6/untitled-ontology-12#Transmittance">
        <rdfs:subClassOf rdf:resource="http://www.semanticweb.org/qihan/ontologies/2023/6/untitled-ontology-12#Optical_Properties"/>
    </owl:Class>
    


    <!-- http://www.semanticweb.org/qihan/ontologies/2023/6/untitled-ontology-12#Transverse_Displacement -->

    <owl:Class rdf:about="http://www.semanticweb.org/qihan/ontologies/2023/6/untitled-ontology-12#Transverse_Displacement">
        <rdfs:subClassOf rdf:resource="http://www.semanticweb.org/qihan/ontologies/2023/6/untitled-ontology-12#Displacement"/>
        <rdfs:comment>Represents the displacement or movement of a material, perpendicular to the axis of the applied force or load.</rdfs:comment>
        <rdfs:label>Transverse Displacement</rdfs:label>
    </owl:Class>
    


    <!-- http://www.semanticweb.org/qihan/ontologies/2023/6/untitled-ontology-12#Transverse_Orientation -->

    <owl:Class rdf:about="http://www.semanticweb.org/qihan/ontologies/2023/6/untitled-ontology-12#Transverse_Orientation">
        <rdfs:subClassOf rdf:resource="http://www.semanticweb.org/qihan/ontologies/2023/6/untitled-ontology-12#Orientation"/>
        <rdfs:comment>Represents the orientation of a material aligned perpendicular to the primary axis or longitudinal direction.</rdfs:comment>
        <rdfs:label>Transverse Orientation</rdfs:label>
    </owl:Class>
    


    <!-- http://www.semanticweb.org/qihan/ontologies/2023/6/untitled-ontology-12#Transverse_Strain -->

    <owl:Class rdf:about="http://www.semanticweb.org/qihan/ontologies/2023/6/untitled-ontology-12#Transverse_Strain">
        <rdfs:subClassOf rdf:resource="http://www.semanticweb.org/qihan/ontologies/2023/6/untitled-ontology-12#Strain"/>
        <rdfs:comment>Represents the change in size or deformation perpendicular to the applied load direction in a material.</rdfs:comment>
        <rdfs:label>Transverse Strain</rdfs:label>
    </owl:Class>
    


    <!-- http://www.semanticweb.org/qihan/ontologies/2023/6/untitled-ontology-12#Trimming_Equipment -->

    <owl:Class rdf:about="http://www.semanticweb.org/qihan/ontologies/2023/6/untitled-ontology-12#Trimming_Equipment">
        <rdfs:subClassOf rdf:resource="http://www.semanticweb.org/qihan/ontologies/2023/6/untitled-ontology-12#Specimen_Preparation_Equipment"/>
        <rdfs:label>Trimming Equipment</rdfs:label>
    </owl:Class>
    


    <!-- http://www.semanticweb.org/qihan/ontologies/2023/6/untitled-ontology-12#Trimming_Press -->

    <owl:Class rdf:about="http://www.semanticweb.org/qihan/ontologies/2023/6/untitled-ontology-12#Trimming_Press">
        <rdfs:subClassOf rdf:resource="http://www.semanticweb.org/qihan/ontologies/2023/6/untitled-ontology-12#Trimming_Equipment"/>
        <rdfs:comment>Represents a type of machine equipped with a cutting die or tool used to trim excess material from workpieces.</rdfs:comment>
        <rdfs:label>Trimming Press</rdfs:label>
    </owl:Class>
    


    <!-- http://www.semanticweb.org/qihan/ontologies/2023/6/untitled-ontology-12#Trimming_Router -->

    <owl:Class rdf:about="http://www.semanticweb.org/qihan/ontologies/2023/6/untitled-ontology-12#Trimming_Router">
        <rdfs:subClassOf rdf:resource="http://www.semanticweb.org/qihan/ontologies/2023/6/untitled-ontology-12#Trimming_Equipment"/>
        <rdfs:comment>Represents a handheld power tool equipped with a rotating cutting bit used for trimming and shaping workpieces with precision.</rdfs:comment>
        <rdfs:label>Trimming Router</rdfs:label>
    </owl:Class>
    


    <!-- http://www.semanticweb.org/qihan/ontologies/2023/6/untitled-ontology-12#Trimming_Tool -->

    <owl:Class rdf:about="http://www.semanticweb.org/qihan/ontologies/2023/6/untitled-ontology-12#Trimming_Tool">
        <rdfs:subClassOf rdf:resource="http://www.semanticweb.org/qihan/ontologies/2023/6/untitled-ontology-12#Trimming_Equipment"/>
        <rdfs:comment>Represents a handheld cutting tool designed for manual trimming and shaping of workpieces.</rdfs:comment>
        <rdfs:label>Trimming Tool</rdfs:label>
    </owl:Class>
    


    <!-- http://www.semanticweb.org/qihan/ontologies/2023/6/untitled-ontology-12#UV_Resistance -->

    <owl:Class rdf:about="http://www.semanticweb.org/qihan/ontologies/2023/6/untitled-ontology-12#UV_Resistance">
        <rdfs:subClassOf rdf:resource="http://www.semanticweb.org/qihan/ontologies/2023/6/untitled-ontology-12#Aging_Properties"/>
    </owl:Class>
    


    <!-- http://www.semanticweb.org/qihan/ontologies/2023/6/untitled-ontology-12#Ultrasonic_Cleaner -->

    <owl:Class rdf:about="http://www.semanticweb.org/qihan/ontologies/2023/6/untitled-ontology-12#Ultrasonic_Cleaner">
        <rdfs:subClassOf rdf:resource="http://www.semanticweb.org/qihan/ontologies/2023/6/untitled-ontology-12#Specimen_Cleaning_Equipment"/>
        <rdfs:comment>Represents a type of cleaning equipment that uses ultrasonic waves to create high-frequency vibrations in a cleaning liquid, producing cavitation bubbles that agitate and dislodge dirt and contaminants from specimens and surfaces.</rdfs:comment>
        <rdfs:label>Ultrasonic Cleaner</rdfs:label>
    </owl:Class>
    


    <!-- http://www.semanticweb.org/qihan/ontologies/2023/6/untitled-ontology-12#Ultrasonic_Flaw_Detector -->

    <owl:Class rdf:about="http://www.semanticweb.org/qihan/ontologies/2023/6/untitled-ontology-12#Ultrasonic_Flaw_Detector">
        <rdfs:subClassOf rdf:resource="http://www.semanticweb.org/qihan/ontologies/2023/6/untitled-ontology-12#Ultrasonic_Testing_Equipment"/>
        <rdfs:comment>Represents a specialized device used to detect and analyze internal flaws or defects in materials.</rdfs:comment>
        <rdfs:label>Ultrasonic Flaw Detector</rdfs:label>
    </owl:Class>
    


    <!-- http://www.semanticweb.org/qihan/ontologies/2023/6/untitled-ontology-12#Ultrasonic_Testing_Equipment -->

    <owl:Class rdf:about="http://www.semanticweb.org/qihan/ontologies/2023/6/untitled-ontology-12#Ultrasonic_Testing_Equipment">
        <rdfs:subClassOf rdf:resource="http://www.semanticweb.org/qihan/ontologies/2023/6/untitled-ontology-12#Test_Equipment"/>
        <rdfs:comment>Represents a category of test equipment used for non-destructive testing of composite material specimens using ultrasonic waves. It can detect internal defects and  flaws through sound wave reflections.</rdfs:comment>
        <rdfs:label>Ultrasonic Testing Equipment</rdfs:label>
    </owl:Class>
    


    <!-- http://www.semanticweb.org/qihan/ontologies/2023/6/untitled-ontology-12#Ultrasonic_Thickness_Gauge -->

    <owl:Class rdf:about="http://www.semanticweb.org/qihan/ontologies/2023/6/untitled-ontology-12#Ultrasonic_Thickness_Gauge">
        <rdfs:subClassOf rdf:resource="http://www.semanticweb.org/qihan/ontologies/2023/6/untitled-ontology-12#Ultrasonic_Testing_Equipment"/>
        <rdfs:comment>Represents a specialized device used to measure the thickness of materials by utilizing ultrasonic waves</rdfs:comment>
        <rdfs:label>Ultrasonic Thickness Gauge</rdfs:label>
    </owl:Class>
    


    <!-- http://www.semanticweb.org/qihan/ontologies/2023/6/untitled-ontology-12#Unidirectional_Composite -->

    <owl:Class rdf:about="http://www.semanticweb.org/qihan/ontologies/2023/6/untitled-ontology-12#Unidirectional_Composite">
        <rdfs:subClassOf rdf:resource="http://www.semanticweb.org/qihan/ontologies/2023/6/untitled-ontology-12#Continuous_Fiber_Composite"/>
    </owl:Class>
    


    <!-- http://www.semanticweb.org/qihan/ontologies/2023/6/untitled-ontology-12#Universal_Testing_Machine -->

    <owl:Class rdf:about="http://www.semanticweb.org/qihan/ontologies/2023/6/untitled-ontology-12#Universal_Testing_Machine">
        <rdfs:subClassOf rdf:resource="http://www.semanticweb.org/qihan/ontologies/2023/6/untitled-ontology-12#Test_Equipment"/>
        <rdfs:comment>Represents a versatile test equipment used for mechanical testing of composite material specimens. It applies various loads to assess mechanical properties.</rdfs:comment>
        <rdfs:label>Universal Testing Machine</rdfs:label>
    </owl:Class>
    


    <!-- http://www.semanticweb.org/qihan/ontologies/2023/6/untitled-ontology-12#University_Laboratory -->

    <owl:Class rdf:about="http://www.semanticweb.org/qihan/ontologies/2023/6/untitled-ontology-12#University_Laboratory">
        <rdfs:subClassOf rdf:resource="http://www.semanticweb.org/qihan/ontologies/2023/6/untitled-ontology-12#Testing_Institution"/>
        <rdfs:comment>Represents a laboratory or research facility within a university or educational institution that is engaged in scientific research and experimentation.</rdfs:comment>
        <rdfs:label>University Laboratory</rdfs:label>
    </owl:Class>
    


    <!-- http://www.semanticweb.org/qihan/ontologies/2023/6/untitled-ontology-12#Utility_Knives -->

    <owl:Class rdf:about="http://www.semanticweb.org/qihan/ontologies/2023/6/untitled-ontology-12#Utility_Knives">
        <rdfs:subClassOf rdf:resource="http://www.semanticweb.org/qihan/ontologies/2023/6/untitled-ontology-12#Handheld_Cutting_Tools"/>
        <rdfs:comment>Represents a type of cutting tool.</rdfs:comment>
        <rdfs:label>Untility Knives</rdfs:label>
    </owl:Class>
    


    <!-- http://www.semanticweb.org/qihan/ontologies/2023/6/untitled-ontology-12#V-Notched_Beam_Specimen -->

    <owl:Class rdf:about="http://www.semanticweb.org/qihan/ontologies/2023/6/untitled-ontology-12#V-Notched_Beam_Specimen">
        <rdfs:subClassOf rdf:resource="http://www.semanticweb.org/qihan/ontologies/2023/6/untitled-ontology-12#Test_Specimen_Geometry"/>
        <rdfs:comment>Represents a type of test specimen with a V-shaped notch or groove, often used in fracture mechanics tests to study crack propagation and fracture behavior under bending and tension loads.</rdfs:comment>
        <rdfs:label>V-Notched Beam Specimen</rdfs:label>
    </owl:Class>
    


    <!-- http://www.semanticweb.org/qihan/ontologies/2023/6/untitled-ontology-12#V-Notched_Rail_Shear_Apparatus -->

    <owl:Class rdf:about="http://www.semanticweb.org/qihan/ontologies/2023/6/untitled-ontology-12#V-Notched_Rail_Shear_Apparatus">
        <rdfs:subClassOf rdf:resource="http://www.semanticweb.org/qihan/ontologies/2023/6/untitled-ontology-12#Shear_Testing_Apparatus"/>
        <rdfs:label>Represents a specialized testing apparatus used to perform the v-notched rail shear test on composite material specimens.</rdfs:label>
        <rdfs:label>V-Notched Rail Shear Apparatus</rdfs:label>
    </owl:Class>
    


    <!-- http://www.semanticweb.org/qihan/ontologies/2023/6/untitled-ontology-12#Vacuum -->

    <owl:Class rdf:about="http://www.semanticweb.org/qihan/ontologies/2023/6/untitled-ontology-12#Vacuum">
        <rdfs:subClassOf rdf:resource="http://www.semanticweb.org/qihan/ontologies/2023/6/untitled-ontology-12#Medium"/>
        <rdfs:subClassOf rdf:resource="http://www.semanticweb.org/qihan/ontologies/2023/6/untitled-ontology-12#Pressure_Condition"/>
        <rdfs:comment>Represents the medium of the testing environment for mechanical testing of composite material specimens. It refers to a state of low pressure or absence of air or other gases.</rdfs:comment>
        <rdfs:label>Vacuum</rdfs:label>
    </owl:Class>
    


    <!-- http://www.semanticweb.org/qihan/ontologies/2023/6/untitled-ontology-12#Vacuum_Assisted_Resin_Infusion -->

    <owl:Class rdf:about="http://www.semanticweb.org/qihan/ontologies/2023/6/untitled-ontology-12#Vacuum_Assisted_Resin_Infusion">
        <rdfs:subClassOf rdf:resource="http://www.semanticweb.org/qihan/ontologies/2023/6/untitled-ontology-12#Resin_Infusion_Processes"/>
        <rdfs:comment>Represents a specific resin infusion process where dry fibers or a fiber reinforcement is placed in a mold or tool.</rdfs:comment>
        <rdfs:label>Vacuum Assisted Resin Infusion</rdfs:label>
    </owl:Class>
    


    <!-- http://www.semanticweb.org/qihan/ontologies/2023/6/untitled-ontology-12#Vacuum_Bag_Only -->

    <owl:Class rdf:about="http://www.semanticweb.org/qihan/ontologies/2023/6/untitled-ontology-12#Vacuum_Bag_Only">
        <rdfs:subClassOf rdf:resource="http://www.semanticweb.org/qihan/ontologies/2023/6/untitled-ontology-12#Out-of-Autoclave_Curing_Processes"/>
        <rdfs:comment>Represents a specific out of autoclave curing process where composite materials are laid up and consolidated inside a vacuum bag without additional heating.</rdfs:comment>
        <rdfs:label>Vacuum Bag Only</rdfs:label>
    </owl:Class>
    


    <!-- http://www.semanticweb.org/qihan/ontologies/2023/6/untitled-ontology-12#Vacuum_Bag_with_Oven -->

    <owl:Class rdf:about="http://www.semanticweb.org/qihan/ontologies/2023/6/untitled-ontology-12#Vacuum_Bag_with_Oven">
        <rdfs:subClassOf rdf:resource="http://www.semanticweb.org/qihan/ontologies/2023/6/untitled-ontology-12#Out-of-Autoclave_Curing_Processes"/>
        <rdfs:comment>Represents a specific out of autoclave curing process that combines the use of a vacuum bag and an oven.</rdfs:comment>
        <rdfs:label>Vacuum Bag with Oven</rdfs:label>
    </owl:Class>
    


    <!-- http://www.semanticweb.org/qihan/ontologies/2023/6/untitled-ontology-12#Vacuum_Bag_with_Resin_Infusion -->

    <owl:Class rdf:about="http://www.semanticweb.org/qihan/ontologies/2023/6/untitled-ontology-12#Vacuum_Bag_with_Resin_Infusion">
        <rdfs:subClassOf rdf:resource="http://www.semanticweb.org/qihan/ontologies/2023/6/untitled-ontology-12#Out-of-Autoclave_Curing_Processes"/>
        <rdfs:comment>Represents a specific out of autoclave curing process that involves the application of vacuum pressure and resin infusion to cure composite materials.</rdfs:comment>
        <rdfs:label>Vacuum Bag with Resin Infusion</rdfs:label>
    </owl:Class>
    


    <!-- http://www.semanticweb.org/qihan/ontologies/2023/6/untitled-ontology-12#Vacuum_Forming -->

    <owl:Class rdf:about="http://www.semanticweb.org/qihan/ontologies/2023/6/untitled-ontology-12#Vacuum_Forming">
        <rdfs:subClassOf rdf:resource="http://www.semanticweb.org/qihan/ontologies/2023/6/untitled-ontology-12#Molding_Machine"/>
        <rdfs:comment>Represents a type of thermoforming molding process where a heated thermoplastic sheet is placed over a mold and vacuum pressure is applied to shape the material to the mold contours.</rdfs:comment>
        <rdfs:label>Vacuum Forming</rdfs:label>
    </owl:Class>
    


    <!-- http://www.semanticweb.org/qihan/ontologies/2023/6/untitled-ontology-12#Vacuum_Infusion_Process -->

    <owl:Class rdf:about="http://www.semanticweb.org/qihan/ontologies/2023/6/untitled-ontology-12#Vacuum_Infusion_Process">
        <rdfs:subClassOf rdf:resource="http://www.semanticweb.org/qihan/ontologies/2023/6/untitled-ontology-12#Resin_Infusion_Processes"/>
        <rdfs:comment>Represents a specific resin infusion process where dry fibers or a fiber reinforcement is placed in a mold or layup.</rdfs:comment>
        <rdfs:label>Vacuum Infusion Process</rdfs:label>
    </owl:Class>
    


    <!-- http://www.semanticweb.org/qihan/ontologies/2023/6/untitled-ontology-12#Vacuum_casting_machine -->

    <owl:Class rdf:about="http://www.semanticweb.org/qihan/ontologies/2023/6/untitled-ontology-12#Vacuum_casting_machine">
        <rdfs:subClassOf rdf:resource="http://www.semanticweb.org/qihan/ontologies/2023/6/untitled-ontology-12#Casting_Machine"/>
        <rdfs:comment>Represents a type of casting machine used to produce high-quality castings with minimal porosity and defects.</rdfs:comment>
        <rdfs:label>Vacuum Casting Machine</rdfs:label>
    </owl:Class>
    


    <!-- http://www.semanticweb.org/qihan/ontologies/2023/6/untitled-ontology-12#Vascular_Network-based_Self-healing_Composite -->

    <owl:Class rdf:about="http://www.semanticweb.org/qihan/ontologies/2023/6/untitled-ontology-12#Vascular_Network-based_Self-healing_Composite">
        <rdfs:subClassOf rdf:resource="http://www.semanticweb.org/qihan/ontologies/2023/6/untitled-ontology-12#Self-healing_Composite"/>
    </owl:Class>
    


    <!-- http://www.semanticweb.org/qihan/ontologies/2023/6/untitled-ontology-12#Vertical_casting_machine -->

    <owl:Class rdf:about="http://www.semanticweb.org/qihan/ontologies/2023/6/untitled-ontology-12#Vertical_casting_machine">
        <rdfs:subClassOf rdf:resource="http://www.semanticweb.org/qihan/ontologies/2023/6/untitled-ontology-12#Casting_Machine"/>
        <rdfs:comment>Represents a type of casting machine that performs casting in a vertical orientation.</rdfs:comment>
        <rdfs:label>Vertical Casting Machine</rdfs:label>
    </owl:Class>
    


    <!-- http://www.semanticweb.org/qihan/ontologies/2023/6/untitled-ontology-12#Vibrational_Acceleration -->

    <owl:Class rdf:about="http://www.semanticweb.org/qihan/ontologies/2023/6/untitled-ontology-12#Vibrational_Acceleration">
        <rdfs:subClassOf rdf:resource="http://www.semanticweb.org/qihan/ontologies/2023/6/untitled-ontology-12#Acceleration"/>
        <rdfs:comment>Represents the acceleration experienced by a material due to vibrational or oscillatory motion.</rdfs:comment>
        <rdfs:label>Vibrational Acceleration</rdfs:label>
    </owl:Class>
    


    <!-- http://www.semanticweb.org/qihan/ontologies/2023/6/untitled-ontology-12#Vibrational_Frequency -->

    <owl:Class rdf:about="http://www.semanticweb.org/qihan/ontologies/2023/6/untitled-ontology-12#Vibrational_Frequency">
        <rdfs:subClassOf rdf:resource="http://www.semanticweb.org/qihan/ontologies/2023/6/untitled-ontology-12#Frequency"/>
        <rdfs:comment>Represents the frequency at which a material, exhibits vibrations or oscillations when subjected to external forces or excitations.</rdfs:comment>
        <rdfs:label>Vibrational Frequency</rdfs:label>
    </owl:Class>
    


    <!-- http://www.semanticweb.org/qihan/ontologies/2023/6/untitled-ontology-12#Vickers_Hardness -->

    <owl:Class rdf:about="http://www.semanticweb.org/qihan/ontologies/2023/6/untitled-ontology-12#Vickers_Hardness">
        <rdfs:subClassOf rdf:resource="http://www.semanticweb.org/qihan/ontologies/2023/6/untitled-ontology-12#Hardness"/>
    </owl:Class>
    


    <!-- http://www.semanticweb.org/qihan/ontologies/2023/6/untitled-ontology-12#Vickers_Hardness_Tester -->

    <owl:Class rdf:about="http://www.semanticweb.org/qihan/ontologies/2023/6/untitled-ontology-12#Vickers_Hardness_Tester">
        <rdfs:subClassOf rdf:resource="http://www.semanticweb.org/qihan/ontologies/2023/6/untitled-ontology-12#Hardness_Tester"/>
        <rdfs:comment>Represents a specific type of hardness tester used to determine the Vickers hardness of materials, including composite material specimens.</rdfs:comment>
        <rdfs:label>Vickers Hardness Tester</rdfs:label>
    </owl:Class>
    


    <!-- http://www.semanticweb.org/qihan/ontologies/2023/6/untitled-ontology-12#Vickers_Hardness_Testing -->

    <owl:Class rdf:about="http://www.semanticweb.org/qihan/ontologies/2023/6/untitled-ontology-12#Vickers_Hardness_Testing">
        <rdfs:subClassOf rdf:resource="http://www.semanticweb.org/qihan/ontologies/2023/6/untitled-ontology-12#Hardness_Testing"/>
        <rdfs:comment>Represents a type of hardness testing method used to determine the hardness of materials, by measuring the size of an indentation formed by a diamond pyramid indenter.</rdfs:comment>
        <rdfs:label>Vickers Hardness Testing</rdfs:label>
    </owl:Class>
    


    <!-- http://www.semanticweb.org/qihan/ontologies/2023/6/untitled-ontology-12#Visualization_Software -->

    <owl:Class rdf:about="http://www.semanticweb.org/qihan/ontologies/2023/6/untitled-ontology-12#Visualization_Software">
        <rdfs:subClassOf rdf:resource="http://www.semanticweb.org/qihan/ontologies/2023/6/untitled-ontology-12#Data_Visualization"/>
    </owl:Class>
    


    <!-- http://www.semanticweb.org/qihan/ontologies/2023/6/untitled-ontology-12#Visualization__Technique -->

    <owl:Class rdf:about="http://www.semanticweb.org/qihan/ontologies/2023/6/untitled-ontology-12#Visualization__Technique">
        <rdfs:subClassOf rdf:resource="http://www.semanticweb.org/qihan/ontologies/2023/6/untitled-ontology-12#Data_Visualization"/>
    </owl:Class>
    


    <!-- http://www.semanticweb.org/qihan/ontologies/2023/6/untitled-ontology-12#Volume_Resistivity -->

    <owl:Class rdf:about="http://www.semanticweb.org/qihan/ontologies/2023/6/untitled-ontology-12#Volume_Resistivity">
        <rdfs:subClassOf rdf:resource="http://www.semanticweb.org/qihan/ontologies/2023/6/untitled-ontology-12#Electriical_Conductivity"/>
    </owl:Class>
    


    <!-- http://www.semanticweb.org/qihan/ontologies/2023/6/untitled-ontology-12#Water -->

    <owl:Class rdf:about="http://www.semanticweb.org/qihan/ontologies/2023/6/untitled-ontology-12#Water">
        <rdfs:subClassOf rdf:resource="http://www.semanticweb.org/qihan/ontologies/2023/6/untitled-ontology-12#Medium"/>
        <rdfs:comment>Represents the medium of the testing environment for mechanical testing of composite material specimens. It refers to the liquid state of H2O and is used in various testing scenarios, such as submerged or wet conditions.</rdfs:comment>
        <rdfs:label>Water</rdfs:label>
    </owl:Class>
    


    <!-- http://www.semanticweb.org/qihan/ontologies/2023/6/untitled-ontology-12#Waterjet_Cutting_Machine -->

    <owl:Class rdf:about="http://www.semanticweb.org/qihan/ontologies/2023/6/untitled-ontology-12#Waterjet_Cutting_Machine">
        <rdfs:subClassOf rdf:resource="http://www.semanticweb.org/qihan/ontologies/2023/6/untitled-ontology-12#Cutting_Equipment"/>
        <rdfs:comment>Represents a type of cutting machine that utilizes a high-pressure jet of water mixed with an abrasive material to cut through materials.</rdfs:comment>
        <rdfs:label>Waterjet Cutting Machine</rdfs:label>
    </owl:Class>
    


    <!-- http://www.semanticweb.org/qihan/ontologies/2023/6/untitled-ontology-12#Wear_Rate -->

    <owl:Class rdf:about="http://www.semanticweb.org/qihan/ontologies/2023/6/untitled-ontology-12#Wear_Rate">
        <rdfs:subClassOf rdf:resource="http://www.semanticweb.org/qihan/ontologies/2023/6/untitled-ontology-12#Wear_Resistance"/>
    </owl:Class>
    


    <!-- http://www.semanticweb.org/qihan/ontologies/2023/6/untitled-ontology-12#Wear_Resistance -->

    <owl:Class rdf:about="http://www.semanticweb.org/qihan/ontologies/2023/6/untitled-ontology-12#Wear_Resistance">
        <rdfs:subClassOf rdf:resource="http://www.semanticweb.org/qihan/ontologies/2023/6/untitled-ontology-12#Result_Calculation"/>
    </owl:Class>
    


    <!-- http://www.semanticweb.org/qihan/ontologies/2023/6/untitled-ontology-12#Wet_Condition -->

    <owl:Class rdf:about="http://www.semanticweb.org/qihan/ontologies/2023/6/untitled-ontology-12#Wet_Condition">
        <rdfs:subClassOf rdf:resource="http://www.semanticweb.org/qihan/ontologies/2023/6/untitled-ontology-12#Moisture_Content"/>
        <rdfs:comment>Represents the state or condition of a material, when it is exposed to or saturated with moisture or water.</rdfs:comment>
        <rdfs:label>Wet Condition</rdfs:label>
    </owl:Class>
    


    <!-- http://www.semanticweb.org/qihan/ontologies/2023/6/untitled-ontology-12#Woven_Fabric_Composite -->

    <owl:Class rdf:about="http://www.semanticweb.org/qihan/ontologies/2023/6/untitled-ontology-12#Woven_Fabric_Composite">
        <rdfs:subClassOf rdf:resource="http://www.semanticweb.org/qihan/ontologies/2023/6/untitled-ontology-12#Continuous_Fiber_Composite"/>
    </owl:Class>
    


    <!-- http://www.semanticweb.org/qihan/ontologies/2023/6/untitled-ontology-12#Zirconia_Matrix_Composite -->

    <owl:Class rdf:about="http://www.semanticweb.org/qihan/ontologies/2023/6/untitled-ontology-12#Zirconia_Matrix_Composite">
        <rdfs:subClassOf rdf:resource="http://www.semanticweb.org/qihan/ontologies/2023/6/untitled-ontology-12#Ceramic_Matrix_Composite"/>
    </owl:Class>
    


    <!-- http://www.semanticweb.org/qihan/ontologies/2023/6/untitled-ontology-12#pH -->

    <owl:Class rdf:about="http://www.semanticweb.org/qihan/ontologies/2023/6/untitled-ontology-12#pH">
        <rdfs:subClassOf rdf:resource="http://www.semanticweb.org/qihan/ontologies/2023/6/untitled-ontology-12#Test_Parameter"/>
        <rdfs:comment>Represents the measure of acidity or alkalinity of material.</rdfs:comment>
        <rdfs:label>pH, Acidity, Potential of Hydrogen</rdfs:label>
    </owl:Class>
    


    <!-- http://www.semanticweb.org/qihan/ontologies/2023/6/untitled-ontology-12#Acidity/Alkalinity_Level -->

    <owl:Class rdf:about="http://www.semanticweb.org/qihan/ontologies/2023/6/untitled-ontology-12#Acidity/Alkalinity_Level">
        <rdfs:subClassOf rdf:resource="http://www.semanticweb.org/qihan/ontologies/2023/6/untitled-ontology-12#pH"/>
        <rdfs:comment>Represents the measure of the acidity or alkalinity of a substance, typically expressed as pH value.</rdfs:comment>
        <rdfs:label>Acidity/Alkalinity Level</rdfs:label>
    </owl:Class>
    


    <!-- http://www.semanticweb.org/qihan/ontologies/2023/6/untitled-ontology-12#Young&apos;s_Modulus -->

    <owl:Class rdf:about="http://www.semanticweb.org/qihan/ontologies/2023/6/untitled-ontology-12#Young&apos;s_Modulus">
        <rdfs:subClassOf rdf:resource="http://www.semanticweb.org/qihan/ontologies/2023/6/untitled-ontology-12#Stiffness"/>
    </owl:Class>
    


    <!-- 
    ///////////////////////////////////////////////////////////////////////////////////////
    //
    // Annotations
    //
    ///////////////////////////////////////////////////////////////////////////////////////
     -->

    <rdf:Description rdf:about="http://www.semanticweb.org/qihan/ontologies/2023/6/untitled-ontology-12#Failure_Mode">
        <rdfs:comment>Provides a more detailed description or explanation of the characteristics and behavior associated with the specific failure mode</rdfs:comment>
    </rdf:Description>
</rdf:RDF>



<!-- Generated by the OWL API (version 4.5.25.2023-02-15T19:15:49Z) https://github.com/owlcs/owlapi -->

